@prefix : <http://example.org/zilf/> .
@prefix owl: <http://www.w3.org/2002/07/owl#> .
@prefix rdf: <http://www.w3.org/1999/02/22-rdf-syntax-ns#> .
@prefix xml: <http://www.w3.org/XML/1998/namespace> .
@prefix xsd: <http://www.w3.org/2001/XMLSchema#> .
@prefix rdfs: <http://www.w3.org/2000/01/rdf-schema#> .
@prefix skos: <http://www.w3.org/2004/02/skos/core#> .
@prefix zilf: <http://example.org/zilf/> .
@base <http://example.org/zilf/> .

<http://example.org/zilf/> rdf:type owl:Ontology ;
    owl:imports <http://www.w3.org/2004/02/skos/core> .

#################################################################
#    Classes
#################################################################

zilf:LanguageConstruct rdf:type owl:Class ;
    rdfs:subClassOf skos:Concept .

#################################################################
#    Individuals (ZILF Content)
#################################################################

# The Main Scheme
zilf:ZILF_Scheme rdf:type owl:NamedIndividual , skos:ConceptScheme ;
    skos:prefLabel "ZILF Reference Scheme"@en ;
    skos:hasTopConcept zilf:CoreFunctions , zilf:ObjectSystem , zilf:ParserSystem .

# --- Parser System Category ---
zilf:ParserSystem rdf:type owl:NamedIndividual , skos:Concept ;
    skos:prefLabel "Parser System"@en ;
    skos:topConceptOf zilf:ZILF_Scheme ;
    skos:narrower zilf:VERB , zilf:SYNTAX , zilf:PREP .

zilf:VERB rdf:type owl:NamedIndividual , skos:Concept ;
    skos:prefLabel "VERB"@en ;
    skos:broader zilf:ParserSystem ;
    skos:definition "Defines action words (e.g., TAKE, DROP) and links them to syntax patterns." ;
    skos:example "<VERB TAKE T TAKE>" .

zilf:SYNTAX rdf:type owl:NamedIndividual , skos:Concept ;
    skos:prefLabel "SYNTAX"@en ;
    skos:broader zilf:ParserSystem ;
    skos:definition "Defines the grammatical structure of a command (e.g., VERB OBJECT WITH OBJECT)." .

zilf:PREP rdf:type owl:NamedIndividual , skos:Concept ;
    skos:prefLabel "PREP"@en ;
    skos:altLabel "Preposition"@en ;
    skos:broader zilf:ParserSystem ;
    skos:definition "Words like IN, ON, or WITH used to clarify object relationships in a command." .

# --- Existing Categories ---
zilf:CoreFunctions rdf:type owl:NamedIndividual , skos:Concept ;
    skos:prefLabel "Core Functions"@en ;
    skos:topConceptOf zilf:ZILF_Scheme ;
    skos:narrower zilf:SETG .

zilf:ObjectSystem rdf:type owl:NamedIndividual , skos:Concept ;
    skos:prefLabel "Object System"@en ;
    skos:topConceptOf zilf:ZILF_Scheme ;
    skos:narrower zilf:OBJECT .

zilf:SETG rdf:type owl:NamedIndividual , skos:Concept ;
    skos:prefLabel "SETG"@en ;
    skos:broader zilf:CoreFunctions .

zilf:OBJECT rdf:type owl:NamedIndividual , skos:Concept ;
    skos:prefLabel "OBJECT"@en ;
    skos:broader zilf:ObjectSystem .