@prefix : <http://example.org/zilf/> .
@prefix owl: <http://www.w3.org/2002/07/owl#> .
@prefix rdf: <http://www.w3.org/1999/02/22-rdf-syntax-ns#> .
@prefix xml: <http://www.w3.org/XML/1998/namespace> .
@prefix xsd: <http://www.w3.org/2001/XMLSchema#> .
@prefix rdfs: <http://www.w3.org/2000/01/rdf-schema#> .
@prefix skos: <http://www.w3.org/2004/02/skos/core#> .
@prefix zilf: <http://example.org/zilf/> .
@base <http://example.org/zilf/> .

<http://example.org/zilf/> rdf:type owl:Ontology ;
                            owl:imports <http://www.w3.org/2004/02/skos/core> .

#################################################################
#    Classes
#################################################################

###  http://example.org/zilf/LanguageConstruct
zilf:LanguageConstruct rdf:type owl:Class ;
                       rdfs:subClassOf skos:Concept .


#################################################################
#    Individuals
#################################################################

###  http://example.org/zilf/BitOn
zilf:BitOn rdf:type owl:NamedIndividual ,
                    skos:Concept ;
           skos:broader zilf:PropFlags ;
           skos:definition "Flag indicating that a light-source object is currently providing light." ;
           skos:prefLabel "ONBIT"@en .


###  http://example.org/zilf/BitTake
zilf:BitTake rdf:type owl:NamedIndividual ,
                      skos:Concept ;
             skos:broader zilf:PropFlags ;
             skos:definition "Flag indicating that an object can be picked up by the player." ;
             skos:prefLabel "TAKEBIT"@en .


###  http://example.org/zilf/CoreFunctions
zilf:CoreFunctions rdf:type owl:NamedIndividual ,
                            skos:Concept ;
                   skos:narrower zilf:SETG ,
                                 zilf:SETG20 ;
                   skos:topConceptOf zilf:ZILF_Scheme ;
                   skos:prefLabel "Core Functions"@en .


###  http://example.org/zilf/OBJECT
zilf:OBJECT rdf:type owl:NamedIndividual .


###  http://example.org/zilf/ObjectProperties
zilf:ObjectProperties rdf:type owl:NamedIndividual ,
                               skos:Concept ;
                      skos:broader zilf:ObjectSystem ;
                      skos:narrower zilf:PropAdjective ,
                                    zilf:PropDesc ,
                                    zilf:PropFlags ,
                                    zilf:PropSynonym ;
                      skos:prefLabel "Object Properties"@en .


###  http://example.org/zilf/ObjectSystem
zilf:ObjectSystem rdf:type owl:NamedIndividual ,
                           skos:Concept ;
                  skos:narrower zilf:OBJECT ,
                                zilf:ObjectProperties ;
                  skos:topConceptOf zilf:ZILF_Scheme ;
                  skos:prefLabel "Object System"@en .


###  http://example.org/zilf/ParserSystem
zilf:ParserSystem rdf:type owl:NamedIndividual ,
                           skos:Concept ;
                  skos:narrower zilf:SYNTAX ,
                                zilf:VERB ;
                  skos:topConceptOf zilf:ZILF_Scheme ;
                  skos:prefLabel "Parser System"@en .


###  http://example.org/zilf/PropAdjective
zilf:PropAdjective rdf:type owl:NamedIndividual ,
                            skos:Concept ;
                   skos:broader zilf:ObjectProperties ;
                   skos:definition "A list of adjectives the parser accepts to identify a specific object." ;
                   skos:example "ADJECTIVE BRASS SMALL" ;
                   skos:prefLabel "ADJECTIVE"@en .


###  http://example.org/zilf/PropDesc
zilf:PropDesc rdf:type owl:NamedIndividual ,
                       skos:Concept ;
              skos:broader zilf:ObjectProperties ;
              skos:definition "A short string used to name the object in game output." ;
              skos:prefLabel "DESC"@en .


###  http://example.org/zilf/PropFlags
zilf:PropFlags rdf:type owl:NamedIndividual ,
                        skos:Concept ;
               skos:broader zilf:ObjectProperties ;
               skos:narrower zilf:BitOn ,
                             zilf:BitTake ;
               skos:definition "A collection of boolean bits (flags) that define the state or behavior of an object." ;
               skos:prefLabel "FLAGS"@en .


###  http://example.org/zilf/PropSynonym
zilf:PropSynonym rdf:type owl:NamedIndividual ,
                          skos:Concept ;
                 skos:broader zilf:ObjectProperties ;
                 skos:definition "A list of nouns the parser accepts for this object." ;
                 skos:prefLabel "SYNONYM"@en .


###  http://example.org/zilf/SETG
zilf:SETG rdf:type owl:NamedIndividual ,
                   skos:Concept ;
          skos:broader zilf:CoreFunctions ;
          skos:definition "MDL built-in that assigns a value to the global atom. If an atom is already assigned a value, it is changed."@en ;
          skos:example "<SETG MYVAR 42> ; Store 42 in global atom MYVAR"@en ;
          skos:prefLabel "SETG"@en .


###  http://example.org/zilf/SETG20
zilf:SETG20 rdf:type owl:NamedIndividual ,
                     skos:Concept ;
            skos:broader zilf:CoreFunctions ;
            skos:inScheme zilf:ZILF_Scheme ;
            skos:definition "A member of the ZIL library, which assigs a value to the global atom. If an atom is already assigned a value, it is changed. SETG20 is an alias for SETG."@en ;
            skos:example "<SETG20 MYVAR 42> ; Store 42 in global atom MYVAR"@en ;
            skos:prefLabel "SETG20"@en .


###  http://example.org/zilf/SYNTAX
zilf:SYNTAX rdf:type owl:NamedIndividual ,
                     skos:Concept ;
            skos:broader zilf:ParserSystem ;
            skos:prefLabel "SYNTAX"@en .


###  http://example.org/zilf/VERB
zilf:VERB rdf:type owl:NamedIndividual ,
                   skos:Concept ;
          skos:broader zilf:ParserSystem ;
          skos:prefLabel "VERB"@en .


###  http://example.org/zilf/ZILF_Scheme
zilf:ZILF_Scheme rdf:type owl:NamedIndividual ,
                          skos:ConceptScheme ;
                 skos:hasTopConcept zilf:CoreFunctions ,
                                    zilf:ObjectSystem ,
                                    zilf:ParserSystem ;
                 skos:prefLabel "ZILF Reference Scheme"@en .


###  Generated by the OWL API (version 4.5.29.2024-05-13T12:11:03Z) https://github.com/owlcs/owlapi
