@prefix : <http://example.org/zilf/> .
@prefix owl: <http://www.w3.org/2002/07/owl#> .
@prefix rdf: <http://www.w3.org/1999/02/22-rdf-syntax-ns#> .
@prefix xml: <http://www.w3.org/XML/1998/namespace> .
@prefix xsd: <http://www.w3.org/2001/XMLSchema#> .
@prefix rdfs: <http://www.w3.org/2000/01/rdf-schema#> .
@prefix skos: <http://www.w3.org/2004/02/skos/core#> .
@prefix zilf: <http://example.org/zilf/> .
@base <http://example.org/zilf/> .

<http://example.org/zilf/> rdf:type owl:Ontology ;
                            owl:imports <http://www.w3.org/2004/02/skos/core> .

#################################################################
#    Annotation properties
#################################################################

###  http://www.w3.org/2004/02/skos/core#altLabel
skos:altLabel rdf:type owl:AnnotationProperty ;
              rdfs:subPropertyOf rdfs:label .


###  http://www.w3.org/2004/02/skos/core#editorialNote
skos:editorialNote rdf:type owl:AnnotationProperty ;
                   rdfs:subPropertyOf rdfs:label .


###  http://www.w3.org/2004/02/skos/core#historyNote
skos:historyNote rdf:type owl:AnnotationProperty ;
                 rdfs:subPropertyOf rdfs:label .


#################################################################
#    Classes
#################################################################

###  http://example.org/zilf/LanguageConstruct
zilf:LanguageConstruct rdf:type owl:Class ;
                       rdfs:subClassOf skos:Concept .


#################################################################
#    Individuals
#################################################################

###  http://example.org/zilf/ADJ-SYNONYM
zilf:ADJ-SYNONYM rdf:type owl:NamedIndividual ,
                          skos:Concept ;
                 skos:broader zilf:ParserSystem ;
                 skos:inScheme zilf:ZILF_Scheme ;
                 skos:definition "ZIL parser library function that creates one or more synonyms to the original adjective. ZILF treats ADJ-SYNONYM as an alias to SYNONYM."@en ;
                 skos:editorialNote "Note that due to the way words, especially adjectives and nouns, are stored in the vocabulary synonyms for adjectives only work in version 3 (ZIP) games."@en ;
                 skos:example """<ADJ-SYNONYM HAPPY JOYFUL>
<ADJ-SYNONYM INTELLIGENT SMART>
<ADJ-SYNONYM BAD AWFUL>
<ADJ-SYNONYM STRONG SOLID>"""@en ;
                 skos:prefLabel "<ADJ-SYNONYM original synonyms ...>"@en .


###  http://example.org/zilf/ASCII
zilf:ASCII rdf:type owl:NamedIndividual ,
                    skos:Concept ;
           skos:broader zilf:CoreFunctions ;
           skos:inScheme zilf:ZILF_Scheme ;
           skos:definition "MDL built-in function that converts a number to a character or a character to a number."@en ;
           skos:example """<ASCII !\\A>  ;  65
<ASCII 65>  ;  !\\A"""@en ;
           skos:prefLabel "<ASCII {number | character}>"@en .


###  http://example.org/zilf/ATOM
zilf:ATOM rdf:type owl:NamedIndividual ,
                   skos:Concept ;
          skos:broader zilf:CoreFunctions ;
          skos:inScheme zilf:ZILF_Scheme ;
          skos:definition "MDL built-in that returns a newly created ATOM with pname (string). The ATOM is not on any OBLIST and therefore has the trailer !-#FALSE () attached to it."@en ;
          skos:example """<ATOM \"FOO\">  ;  FOO!-#FALSE ()
<==? <ATOM \"FOO\"> <ATOM \"FOO\">>  ;  #FALSE"""@en ;
          skos:prefLabel "<ATOM pname>"@en .


###  http://example.org/zilf/AVALUE
zilf:AVALUE rdf:type owl:NamedIndividual ,
                     skos:Concept ;
            skos:broader zilf:CoreFunctions ;
            skos:inScheme zilf:ZILF_Scheme ;
            skos:definition "MDL built-in function that returns the value part from an asoc entry, of TYPE ASOC, in the ASSOCIATION chain."@en ;
            skos:editorialNote "See ASSOCIATIONS, GETPROP, INDICATOR, ITEM, NEXT and PUTPROP."@en ;
            skos:example """<DEFINE LAST-ASOC ()
    <REPEAT ((A <ASSOCIATIONS>))
        <COND (<=? .A <>> <RETURN <>>)
        (<=? <NEXT .A> <>> <RETURN .A>)>
    <SET A <NEXT .A>>>>
<PUTPROP NEW-ASOC TEXT \"Hello, world!\">
<SET A <LAST-ASOC>>
<AVALUE .A>  ;  \"Hello, world!\""""@en ;
            skos:prefLabel "<AVALUE asoc>"@en .


###  http://example.org/zilf/BACK
zilf:BACK rdf:type owl:NamedIndividual ,
                   skos:Concept ;
          skos:broader zilf:ZCodeBuiltIns ;
          skos:inScheme zilf:ZILF_Scheme ;
          skos:definition """Z-code built-in function that returns table with address moved bytes back. If the count moves past the start of the table no error is raised. Default value for bytes is 1. 

Note that this is not a copy of the table, it is pointing to the same table with another starting address. Also see GET, GETB, PUT, PUTB and REST."""@en ;
          skos:example """<GLOBAL TBL1 <TABLE 1 2 3 4>>  ;  TBL1 = [1 2 3 4]
<GLOBAL TBL2 <REST ,STRUCT1 4>>  ;  TBL2 = [3 4] Move 4 because WORD-table!
<SETG TBL2 <BACK ,TBL2 2>>  ;  TBL2 = [2 3 4]"""@en ;
          skos:prefLabel "<BACK table [bytes]>"@en .


###  http://example.org/zilf/BCOM
zilf:BCOM rdf:type owl:NamedIndividual ,
                   skos:Concept ;
          skos:broader zilf:ZCodeBuiltIns ;
          skos:inScheme zilf:ZILF_Scheme ;
          skos:definition "Z-code built-in function that is a bitwise NOT, reversing all bits in the WORD value (16 bits)."@en ;
          skos:editorialNote "ZILF supports BCOM in all versions."@en ;
          skos:example "<BCOM #2 000011110001111>  ;  #2 1111000011110000"@en ;
          skos:historyNote "Zapf syntax: BCOM, Inform syntax: not"@en ;
          skos:prefLabel "<BCOM value>"@en .


###  http://example.org/zilf/BEGIN-SEGMENT
zilf:BEGIN-SEGMENT rdf:type owl:NamedIndividual ,
                            skos:Concept ;
                   skos:broader zilf:CoreFunctions ;
                   skos:inScheme zilf:ZILF_Scheme ;
                   skos:definition "ZIL library function that groups code and data into segments of memory outside the main game memory. BEGIN-SEGMENT pairs with END-SEGMENT."@en ;
                   skos:editorialNote "ZILF ignores this and always returns FALSE."@en ;
                   skos:example """; From The Abyss
<BEGIN-SEGMENT 0>
; Code
<END-SEGMENT>

; From Shogun
<BEGIN-SEGMENT RECORD>
; Code
<END-SEGMENT>"""@en ;
                   skos:historyNote "Having been used in a few InfoCom projects, BEGIN-SEGMENT was notably used in The Abyss, an unreleased interactive fiction game written by Bob Bates for Infocom under historical source code for the game, entitled The Abyss Source Code Collection."@en ;
                   skos:prefLabel "<BEGIN-SEGMENT value>"@en .


###  http://example.org/zilf/BIND
zilf:BIND rdf:type owl:NamedIndividual ,
                   skos:Concept ;
          skos:broader zilf:CoreFunctions ;
          skos:inScheme zilf:ZILF_Scheme ;
          skos:definition """MDL built-in function that defines a program block with its own set of bindings. BIND is similar to PROG and REPEAT but BIND doesn't create a default activation (like PROG and REPEAT) at the start of the block and doesn't have an automatic AGAIN at the end of the block (like REPEAT). If an activation is needed it must be specified. AGAIN and RETURN without specified activation inside a BIND-block will start over or return from the closest surrounding activation within the current function.

The decl is used to specify the valid TYPE of the variables. In its simplest form decl is formatted like: #DECL ((X) FIX), meaning that X must be of the TYPE FIX. For more information on how to format the decl see GDECL. 

Also see AGAIN, PROG, REPEAT and RETURN for more details how to control program flow."""@en ;
          skos:example """<BIND ((X 1)) #DECL ((X) FIX)  
<BIND ((X 2)) <PRIN1 .X>> <PRIN1 .X>>  ;  \"21\"

<DEFINE TEST-BIND-AS-REPEAT () 
    <PRINC \"START \"> 
    <BIND ACT ((X 0)) 
        <SET X <+ .X 1>> 
        <PRIN1 .X> 
        <COND (<=? .X 3> <RETURN T .ACT>)>  ;  \"--> exit block\"
        <AGAIN .ACT>  ;  \"--> repeat\"
    >
    <PRINC \" END\">
>
<TEST-BIND-AS-REPEAT>  ;  \"START 123 END\""""@en ;
          skos:prefLabel "<BIND [activation] (bindings ...) [decl] expressions ...>"@en .


###  http://example.org/zilf/BIT-SYNONYM
zilf:BIT-SYNONYM rdf:type owl:NamedIndividual ,
                          skos:Concept ;
                 skos:broader zilf:ParserSystem ;
                 skos:inScheme zilf:ZILF_Scheme ;
                 skos:definition "ZIL parser library function that creates synonyms to flag-bits."@en ;
                 skos:example """<BIT-SYNONYM TAKEBIT GETBIT PICKBIT>
<BIT-SYNONYM LIGHTBIT DAYBIT>"""@en ;
                 skos:prefLabel "<BIT-SYNONYM first synonyms ...>"@en .


###  http://example.org/zilf/BLOAT
zilf:BLOAT rdf:type owl:NamedIndividual ,
                    skos:Concept ;
           skos:broader zilf:CoreFunctions ;
           skos:inScheme zilf:ZILF_Scheme ;
           skos:definition "MDL built-in function that is used in MDL to temporarily expand available storage space to avoid unnecessary garbage collection when loading large files."@en ;
           skos:editorialNote "ZILF ignores this and always returns FALSE."@en ;
           skos:prefLabel "<BLOAT>"@en .


###  http://example.org/zilf/BLOCK
zilf:BLOCK rdf:type owl:NamedIndividual ,
                    skos:Concept ;
           skos:broader zilf:CoreFunctions ;
           skos:inScheme zilf:ZILF_Scheme ;
           skos:definition "MDL built-in function that  pushes current binding of the local ATOM OBLIST and rebinds it with the LIST of oblist supplied as argument and returns the new <LVAL OBLIST>. Usually you want <ROOT> as the last oblist in LIST. <ENDBLOCK> then restores the local ATOM OBLIST to its previous value."@en ;
           skos:example """<SETG FOO 111>
<SET BAR 222>
<DEFINE TEST-BLOCK () <PRINT \"OUTSIDE BLOCK\">>
<BLOCK (<MOBLIST NEW-OBLIST> <ROOT>)>
<SETG FOO 333>
<SET BAR 444>
<DEFINE TEST-BLOCK () <PRINT \"INSIDE BLOCK\">>
<GVAL FOO>  ;  333
<LVAL BAR>  ;  444 
<TEST-BLOCK>  ;  \"INSIDE BLOCK\"
<ENDBLOCK>
<GVAL FOO>  ;  111
<LVAL BAR>  ;  222
<TEST-BLOCK>  ;  \"OUTSIDE BLOCK\""""@en ;
           skos:prefLabel "<BLOCK (oblist ...)>"@en .


###  http://example.org/zilf/BTST
zilf:BTST rdf:type owl:NamedIndividual ,
                   skos:Concept ;
          skos:broader zilf:ZCodeBuiltIns ;
          skos:inScheme zilf:ZILF_Scheme ;
          skos:definition "Z-code built-in predicate that performs a binary test that evaluates to true if all value2 bits are set in value1. Could be expressed as <=? <BAND value1 value2> value2>."@en ;
          skos:editorialNote "ZILF supports BTST in all versions."@en ;
          skos:example """<BTST 64 64>  ;  TRUE
<BTST 64 63>  ;  FALSE
<BTST 97 33>  ;  TRUE"""@en ;
          skos:historyNote "Zapf syntax: BTST, Inform syntax: test"@en ;
          skos:prefLabel "<BTST value1 value2>"@en .


###  http://example.org/zilf/BUFOUT
zilf:BUFOUT rdf:type owl:NamedIndividual ,
                     skos:Concept ;
            skos:broader zilf:ZCodeBuiltIns ;
            skos:inScheme zilf:ZILF_Scheme ;
            skos:definition "Z-code built-in flag that controls if output is buffered (to enable proper word-wrap). value can be true or false."@en ;
            skos:editorialNote "ZILF supports BUFOUT in versions 4-."@en ;
            skos:example """<BUFOUT <>>  ;  Turns off buffering(disables word-wrap)
<BUFOUT T>  ;  Turns on buffering"""@en ;
            skos:historyNote "Zapf syntax: BUFOUT, Inform syntax: buffer_mode"@en ;
            skos:prefLabel "<BUFOUT value>"@en .


###  http://example.org/zilf/BUZZ
zilf:BUZZ rdf:type owl:NamedIndividual ,
                   skos:Concept ;
          skos:broader zilf:ParserSystem ;
          skos:inScheme zilf:ZILF_Scheme ;
          skos:definition "ZIL parser library function that creates words in the vocabulary with the part-of-speech BUZZ."@en ;
          skos:editorialNote "These are words that can be ignored by the parser or have special handling in the parser."@en ;
          skos:example """<BUZZ A AN AND ANY ALL EVERY EVERYTHING BUT EXCEPT OF ONE
              THE THEN UNDO OOPS \\. \\, \\\">"""@en ;
          skos:prefLabel "<BUZZ atoms ...>"@en .


###  http://example.org/zilf/BYTE
zilf:BYTE rdf:type owl:NamedIndividual ,
                   skos:Concept ;
          skos:broader zilf:CoreFunctions ;
          skos:inScheme zilf:ZILF_Scheme ;
          skos:altLabel "<CHTYPE number BYTE>"@en ;
          skos:definition "ZIL library function that changes number of TYPE to #BYTE."@en ;
          skos:editorialNote "#BYTE number is alternative (MDL built-in) syntax."@en ;
          skos:example """<BYTE 42>  ;  #BYTE 42
#BYTE 42  ;  #BYTE 42
<CHTYPE 42 BYTE>  ;  #BYTE 42"""@en ;
          skos:prefLabel "<BYTE number>"@en .


###  http://example.org/zilf/BitOn
zilf:BitOn rdf:type owl:NamedIndividual ,
                    skos:Concept ;
           skos:broader zilf:PropFlags ;
           skos:definition "Flag indicating that a light-source object is currently providing light." ;
           skos:prefLabel "ONBIT"@en .


###  http://example.org/zilf/BitTake
zilf:BitTake rdf:type owl:NamedIndividual ,
                      skos:Concept ;
             skos:broader zilf:PropFlags ;
             skos:definition "Flag indicating that an object can be picked up by the player." ;
             skos:prefLabel "TAKEBIT"@en .


###  http://example.org/zilf/CATCH
zilf:CATCH rdf:type owl:NamedIndividual ,
                    skos:Concept ;
           skos:broader zilf:ZCodeBuiltIns ;
           skos:inScheme zilf:ZILF_Scheme ;
           skos:definition "Used in conjunction with THROW, this Z-code built-in function returns the current state of the stack (the \"stack frame\"). Also see THROW."@en ;
           skos:editorialNote "ZILF supports CATCH in versions 5-."@en ;
           skos:example "<SETG CATCH-POINT <CATCH>>  ;  Saves the current stack fram in global variable."@en ;
           skos:historyNote "Zapf syntax: CATCH, Inform syntax: catch"@en ;
           skos:prefLabel "<CATCH>"@en .


###  http://example.org/zilf/CHECKPOINT
zilf:CHECKPOINT rdf:type owl:NamedIndividual ,
                         skos:Concept ;
                skos:broader zilf:CoreFunctions ;
                skos:inScheme zilf:ZILF_Scheme ;
                skos:definition "ZIL library function."@en ;
                skos:editorialNote "ZILF ignores this and always returns FALSE."@en ;
                skos:prefLabel "<CHECKPOINT>"@en .


###  http://example.org/zilf/CHRSET
zilf:CHRSET rdf:type owl:NamedIndividual ,
                     skos:Concept ;
            skos:broader zilf:CoreFunctions ;
            skos:inScheme zilf:ZILF_Scheme ;
            skos:definition """ZIL library function that can be used in version 5+ to replace one or more of the standard character alphabets. The ZSCII alphabet table is divided up in three blocks of 26 characters each, totaling 78 characters.

The default layout is:

 Z-char 6789abcdef0123456789abcdef

current

A0      abcdefghijklmnopqrstuvwxyz

A1      ABCDEFGHIJKLMNOPQRSTUVWXYZ

A2       ^0123456789.,!?_#'\"/\\-:()

Text is then encoded into 2-byte words with 5-bits per character. The left-over bit is always 0 except on the last word where it is 1 to indicate that this is the last 2-byte word in the text.

--first byte-------   --second byte---

7    6 5 4 3 2  1 0   7 6 5  4 3 2 1 0

bit  --first--  --second---  --third--

Initially the A0 is the current alphabet. The characters 2, 3, 4 and 5 change alphabet according to this table:

(Z-char N)    from A0      from A1      from A2

(Z-char 2)      A1               A2               A0

(Z-char 3)      A2               A0               A1

(Z-char 4)      A1               A2               A0

(Z-char 5)      A2               A0               A1

Characters 2 and 3 change the alphabet for the next character (“shift”) and characters 4 and 5 change the alphabet permanently (“shift lock”)."""@en ;
            skos:editorialNote "CHARSET changes one character in one alphabet or changes an alphabet altogether."@en ;
            skos:example """;\"    1         2         3
67890123456789012345678901
zyxwvutsrqponmlkjihgfedcba
 z=6   i=23  l=20
1 00110 10111 10100\"

<VERSION 5>

<CHRSET 0 \"zyxwvutsrqponmlkjihgfedcba\">
<CONSTANT ENCODED-TEXT <TABLE #2 1001101011110100>>
<CONSTANT MYTEXT \"zil\">

<ROUTINE GO () <TEST-CHRSET>>

<ROUTINE TEST-CHRSET ()
    <PRINTB ,ENCODED-TEXT> <CRLF>
    <PRINT ,MYTEXT> <CRLF>
    <PRINTN <GET ,ENCODED-TEXT 0>> <CRLF>
    <PRINTN <GET <* 4 ,MYTEXT> 0>> <CRLF> ;\"Multiply by 4 to get packed address in v 5.\"
    <PRINTN <- <GET <* 4 ,MYTEXT> 0> <GET ,ENCODED-TEXT 0>>>
    <CRLF>>

;  Expected output
;  zil
;  zil
;  -25868
;  -25868
;  0"""@en ;
            skos:prefLabel "<CHRSET alphabet-number {string | character | number | byte} ...>"@en .


###  http://example.org/zilf/CLOSE
zilf:CLOSE rdf:type owl:NamedIndividual ,
                    skos:Concept ;
           skos:broader zilf:CoreFunctions ;
           skos:inScheme zilf:ZILF_Scheme ;
           skos:definition "MDL built-in function that closes the channel opened by OPEN and returns the channel."@en ;
           skos:editorialNote "See READSTRING for and example of CLOSE."@en ;
           skos:prefLabel "<CLOSE channel>"@en .


###  http://example.org/zilf/COMPILATION-FLAG
zilf:COMPILATION-FLAG rdf:type owl:NamedIndividual ,
                               skos:Concept ;
                      skos:broader zilf:CoreFunctions ;
                      skos:inScheme zilf:ZILF_Scheme ;
                      skos:definition """ZIL library function that defines a COMPILATION-FLAG named atom-or-string initialized to value. If no value is supplied it defaults to TRUE. The name of the flag can either be an ATOM or a STRING whose text becomes the ATOM. 

The flag can then be read by COMPILATION-FLAG-VALUE or used as a condition in 
IFFLAG."""@en ;
                      skos:editorialNote "A call to COMPILATION-FLAG with an already defined ATOM changes the value of the ATOM."@en ;
                      skos:example """<COMPILATION-FLAG MYFLAG>
<COMPILATION-FLAG-VALUE MYFLAG>  ;  T
<COMPILATION-FLAG “MYFLAG” 123>
<COMPILATION-FLAG-VALUE MYFLAG>  ;  123"""@en ;
                      skos:prefLabel "<COMPILATION-FLAG atom-or-string [value]>"@en .


###  http://example.org/zilf/COMPILATION-FLAG-DEFAULT
zilf:COMPILATION-FLAG-DEFAULT rdf:type owl:NamedIndividual ,
                                       skos:Concept ;
                              skos:broader zilf:CoreFunctions ;
                              skos:inScheme zilf:ZILF_Scheme ;
                              skos:definition """ZIL library function that defines a COMPILATION-FLAG named atom-or-string initialized to value. If no value is supplied it defaults to TRUE. The name of the flag can either be an ATOM or a STRING whose text becomes the ATOM. 

The flag can then be read by COMPILATION-FLAG-VALUE or used as a condition in IFFLAG."""@en ;
                              skos:editorialNote "A call to COMPILATION-FLAG-DEFAULT with an already defined ATOM doesn't change the value of the ATOM."@en ;
                              skos:example """<COMPILATION-FLAG-DEFAULT MYFLAG T>
<COMPILATION-FLAG-VALUE MYFLAG>  ;  T 
<COMPILATION-FLAG “MYFLAG” 123>
<COMPILATION-FLAG-VALUE MYFLAG>  ;  123 
<COMPILATION-FLAG-DEFAULT MYFLAG T>
<COMPILATION-FLAG-VALUE MYFLAG>  ;  123"""@en ;
                              skos:prefLabel "<COMPILATION-FLAG-DEFAULT atom-or-string value>"@en .


###  http://example.org/zilf/COMPILATION-FLAG-VALUE
zilf:COMPILATION-FLAG-VALUE rdf:type owl:NamedIndividual ,
                                     skos:Concept ;
                            skos:broader zilf:CoreFunctions ;
                            skos:inScheme zilf:ZILF_Scheme ;
                            skos:definition "ZIL library function that returns the value of the COMPILATION-FLAG atom-or-string. If no atom-or-string is defined it returns FALSE."@en ;
                            skos:example """<COMPILATION-FLAG MYFLAG 123>
<COMPILATION-FLAG-VALUE MYFLAG>  ;  123
<COMPILATION-FLAG-VALUE ASDFGHJKL>  ;  #FALSE"""@en ;
                            skos:prefLabel "<COMPILATION-FLAG-VALUE atom-or-string>"@en .


###  http://example.org/zilf/CONS
zilf:CONS rdf:type owl:NamedIndividual ,
                   skos:Concept ;
          skos:broader zilf:CoreFunctions ;
          skos:inScheme zilf:ZILF_Scheme ;
          skos:definition "MDL built-in function that adds first to the front of list, without copying list, and returns the resulting LIST. References to list are not affected."@en ;
          skos:editorialNote "CONS means \"construct\"."@en ;
          skos:example """<CONS 1 (2 3)>  ;  (1 2 3)
<SET S1 (!\\B !\\C)>
<SET S2 <CONS !\\A .S1>>
<PUT .S1 2 !\\D>
.S2  ;  (!\\A !\\B !\\D)"""@en ;
          skos:prefLabel "<CONS first list>"@en .


###  http://example.org/zilf/CONSTANT
zilf:CONSTANT rdf:type owl:NamedIndividual ,
                       skos:Concept ;
              skos:broader zilf:CoreFunctions ;
              skos:inScheme zilf:ZILF_Scheme ;
              skos:definition "ZIL library function that defines an atom with value that will never be changed. The atom can is accessed inside a ROUTINE with GVAL (or ,) just like a GLOBAL atom. Defining a CONSTANT instead of a GLOBAL when possible can be vital information the compiler can use for optimization."@en ;
              skos:editorialNote "MSETG is an alias for CONSTANT."@en ;
              skos:example """<CONSTANT MSG-CANT-DO-THAT \"You can't do that!\">
...
<TELL ,MSG-CANT-DO-THAT CR>"""@en ;
              skos:prefLabel "<CONSTANT atom value>"@en .


###  http://example.org/zilf/CRLF
zilf:CRLF rdf:type owl:NamedIndividual ,
                   skos:Concept ;
          skos:broader zilf:CoreFunctions ;
          skos:inScheme zilf:ZILF_Scheme ;
          skos:definition "MDL built-in function that prints a carriage-return and a line-feed to channel (default for channel is <LVAL OUTCHAN>; the console). CRLF returns true."@en ;
          skos:example "<CRLF>  ;  \"\\n\""@en ;
          skos:prefLabel "<CRLF [channel]>"@en .


###  http://example.org/zilf/CoreFunctions
zilf:CoreFunctions rdf:type owl:NamedIndividual ,
                            skos:Concept ;
                   skos:narrower zilf:ASCII ,
                                 zilf:ATOM ,
                                 zilf:AVALUE ,
                                 zilf:BEGIN-SEGMENT ,
                                 zilf:BIND ,
                                 zilf:BLOAT ,
                                 zilf:BLOCK ,
                                 zilf:BYTE ,
                                 zilf:CHECKPOINT ,
                                 zilf:CHRSET ,
                                 zilf:COMPILATION-FLAG ,
                                 zilf:COMPILATION-FLAG-DEFAULT ,
                                 zilf:COMPILATION-FLAG-VALUE ,
                                 zilf:CONS ,
                                 zilf:CONSTANT ,
                                 zilf:CRLF ,
                                 zilf:DECL-CHECK ,
                                 zilf:DEFAULT-DEFINITION ,
                                 zilf:DEFAULTS-DEFINED ,
                                 zilf:DEFINE ,
                                 zilf:DEFINE-GLOBALS ,
                                 zilf:DEFINE-SEGMENT ,
                                 zilf:DEFINE20 ,
                                 zilf:DEFINITIONS ,
                                 zilf:DEFMAC ,
                                 zilf:DELAY-DEFINITION ,
                                 zilf:END-DEFINITIONS ,
                                 zilf:END-SEGMENT ,
                                 zilf:ENDBLOCK ,
                                 zilf:ENDLOAD ,
                                 zilf:ENDPACKAGE ,
                                 zilf:ENDSECTION ,
                                 zilf:ENTRY ,
                                 zilf:EQVB ,
                                 zilf:ERROR ,
                                 zilf:EVAL ,
                                 zilf:EVAL-IN-SEGMENT ,
                                 zilf:EVALTYPE ,
                                 zilf:EXPAND ,
                                 zilf:FILE-LENGTH ,
                                 zilf:FLOAD ,
                                 zilf:FORM ,
                                 zilf:GC ,
                                 zilf:GC-MON ,
                                 zilf:GLOBAL ,
                                 zilf:ISTRING ,
                                 zilf:OR ,
                                 zilf:PICFILE ,
                                 zilf:PNAME ,
                                 zilf:PRIMTYPE ,
                                 zilf:PRIN1 ,
                                 zilf:PRINC ,
                                 zilf:PRINT ,
                                 zilf:PTABLE ,
                                 zilf:PUTREST ,
                                 zilf:QUIT ,
                                 zilf:QUOTE ,
                                 zilf:READSTRING ,
                                 zilf:RENTRY ,
                                 zilf:REPEAT ,
                                 zilf:REPLACE-DEFINITION ,
                                 zilf:ROOT ,
                                 zilf:ROUTINE ,
                                 zilf:SET ,
                                 zilf:SETG ,
                                 zilf:SETG20 ,
                                 zilf:SPNAME ,
                                 zilf:STRING ,
                                 zilf:TOP ,
                                 zilf:VALUE ,
                                 <http://example.org/zilf/BOUND?> ,
                                 <http://example.org/zilf/CHECK-VERSION?> ,
                                 <http://example.org/zilf/COMPILING?> ,
                                 <http://example.org/zilf/DECL?> ,
                                 <http://example.org/zilf/EMPTY?> ,
                                 <http://example.org/zilf/FREQUENT-WORDS?> ,
                                 <http://example.org/zilf/FUNNY-GLOBALS?> ,
                                 <http://example.org/zilf/G?> ,
                                 <http://example.org/zilf/GASSIGNED?> ,
                                 <http://example.org/zilf/GBOUND?> ,
                                 <http://example.org/zilf/OR?> ,
                                 <http://example.org/zilf/VALID-TYPE?> ;
                   skos:topConceptOf zilf:ZILF_Scheme ;
                   skos:prefLabel "Core Functions"@en .


###  http://example.org/zilf/DECL-CHECK
zilf:DECL-CHECK rdf:type owl:NamedIndividual ,
                         skos:Concept ;
                skos:broader zilf:CoreFunctions ;
                skos:inScheme zilf:ZILF_Scheme ;
                skos:definition "MDL built-in function that turns off or on type declaration checking. It is initially on."@en ;
                skos:example """<DECL-CHECK <>>
<GDECL (FOO) FIX>
<SETG FOO <>>  ;  Ok!
<DECL-CHECK T>
<SETG FOO <>>  ;  Error"""@en ;
                skos:prefLabel "<DECL-CHECK boolean>"@en .


###  http://example.org/zilf/DEFAULT-DEFINITION
zilf:DEFAULT-DEFINITION rdf:type owl:NamedIndividual ,
                                 skos:Concept ;
                        skos:broader zilf:CoreFunctions ;
                        skos:inScheme zilf:ZILF_Scheme ;
                        skos:definition """ZIL library function that defines a “replaceable” block with the given name.  

If neither DELAY-DEFINITION nor REPLACE-DEFINITION was previously called for the given name, then the body is evaluated, and this function returns the result of evaluating the last element of the body. 

If the block was replaced (via REPLACE-DEFINITION), the replacement body supplied earlier is used instead. 

If the block was delayed (via DELAY-DEFINITION), the body is ignored, and this function returns FALSE."""@en ;
                        skos:editorialNote """It is possible to do the same by setting REDEFINE to true. This actually makes it possible to change ALL definitions (it is the last one that becomes the one actually compiled). 

See DELAY-DEFINITION and REPLACE-DEFINITION."""@en ;
                        skos:example """<ROUTINE MY-ROUTINE ()  
    <TELL \"Original version of MY-ROUTINE\" CR> 
> 
<SET REDEFINE T> 
    <ROUTINE MY-ROUTINE ()  
        <TELL \"Replaced version of MY-ROUTINE\" CR> 
    > 
<SET REDEFINE <>> 
<MY-ROUTINE>  ;  \"Replaced version of MY-ROUTINE\""""@en ;
                        skos:prefLabel "<DEFAULT-DEFINITION name body ...>"@en .


###  http://example.org/zilf/DEFAULTS-DEFINED
zilf:DEFAULTS-DEFINED rdf:type owl:NamedIndividual ,
                               skos:Concept ;
                      skos:broader zilf:CoreFunctions ;
                      skos:inScheme zilf:ZILF_Scheme ;
                      skos:definition "ZIL library function."@en ;
                      skos:editorialNote "ZILF ignores this and always returns FALSE."@en ;
                      skos:prefLabel "<DEFAULTS-DEFINED>"@en .


###  http://example.org/zilf/DEFINE
zilf:DEFINE rdf:type owl:NamedIndividual ,
                     skos:Concept ;
            skos:broader zilf:CoreFunctions ;
            skos:inScheme zilf:ZILF_Scheme ;
            skos:definition "MDL built-in function that  assigns the global variable name with a FUNCTION. See FUNCTION for an explanation of activation, arg-list, decl and expressions."@en ;
            skos:editorialNote "<DEFINE name ...> is equivalent to <SETG name #FUNCTION ...> with the exception that DEFINE protects from overwriting a name with a new FUNCTION (this behaviour can be changed by setting REDEFINE to true, instead of false)."@en ;
            skos:example """<DEFINE MYADD (X1 X2) <+ .X1 .X2>>
<MYADD 4 5>  ;  9
<DEFINE SQUARE (X) <* .X .X>>
<SQUARE 5>  ;  25
<DEFINE POWER-TO ACT (X \"OPT\" (Y 2)) 
    <COND (<=? .Y 0> <RETURN 1 .ACT>)> 
    <REPEAT ((Z 1)(I 0)) 
        <SET Z <* .Z .X>> 
        <SET I <+ .I 1>> 
        <COND (<=? .I .Y> <RETURN .Z>)> 
    > 
> 
<POWER-TO 2 3>  ;  8
<POWER-TO 3 4>  ;  81
<POWER-TO 3 0>  ;  1"""@en ;
            skos:prefLabel "<DEFINE name [activation] arg-list [decl] expressions ...>"@en .


###  http://example.org/zilf/DEFINE-GLOBALS
zilf:DEFINE-GLOBALS rdf:type owl:NamedIndividual ,
                             skos:Concept ;
                    skos:broader zilf:CoreFunctions ;
                    skos:inScheme zilf:ZILF_Scheme ;
                    skos:definition """ZIL library function that defines a set of macros that can be used for global storage in Z-code, similar to global variables. 

Each atom-or-adecl becomes the name of a new macro which can be called with no arguments (to read the global value) or one argument (to write it). The optional initializer sets the initial value, as in GLOBAL. BYTE or WORD can be specified to set the global’s size; WORD is the default."""@en ;
                    skos:editorialNote """ZILF ignores the group-name.  

See FUNNY-GLOBALS? for a more convenient way to bypass the Z-machine’s global variable limit. (In fact, ZILF implements DEFINE-GLOBALS by turning on FUNNY-GLOBALS? and defining a global variable for each macro.)"""@en ;
                    skos:example """;  From Bureaucracy
<DEFINE-GLOBALS COMPUTER-GLOBALS
    (LAST-LINE-USED:FIX BYTE 0)
    (TIMES-THROUGH-LOOP:FIX BYTE 0)
    (FILES-ON-SCREEN? BYTE <>)
    (TELECOM? BYTE <>)
    (EXITED-ALREADY? BYTE <>)
    (COMPUTER-DEAD? BYTE <>)
    (COMP-X:FIX BYTE 0)
    (COMP-Y:FIX BYTE 0)
    (CURRENT-TARGET-NAME <>)  ;  \"String for interrupt messages\"
    (REAL-TARGET-NAME <>)  ; \"LTABLE for looking stuff up in directory\"
    (REMAINING-TARGET-TURNS:FIX BYTE 0)  ;  \"Turns left until this one's done\"
    (LINES-TO-NEXT-TARGET:FIX BYTE 0)  ;  \"Lines to output before select next target\"
    (TERMINATE-CURRENT:FIX BYTE 0)  ;  \"Lines to output before terminating this one\"
    (COMMANDS-SINCE-START:FIX BYTE 0)  ;  \"Command lines read since target started\"
    (DIE-ON-NEXT-COMMAND BYTE <>)  ;  \"To avoid hair of faking non-local return\"
    (WILL-WIN? BYTE <>)  ;  \"True if killed computer\"
    (FERROR-ACTIVE? BYTE <>)>"""@en ;
                    skos:prefLabel "<DEFINE-GLOBALS group-name (atom-or-adecl [{BYTE | WORD}] [initializer]) ...>"@en .


###  http://example.org/zilf/DEFINE-SEGMENT
zilf:DEFINE-SEGMENT rdf:type owl:NamedIndividual ,
                             skos:Concept ;
                    skos:broader zilf:CoreFunctions ;
                    skos:inScheme zilf:ZILF_Scheme ;
                    skos:definition "ZIL library function."@en ;
                    skos:editorialNote "ZILF ignores this an always returns false."@en ;
                    skos:prefLabel "<DEFINE-SEGMENT>"@en .


###  http://example.org/zilf/DEFINE20
zilf:DEFINE20 rdf:type owl:NamedIndividual ,
                       skos:Concept ;
              skos:broader zilf:CoreFunctions ;
              skos:inScheme zilf:ZILF_Scheme ;
              skos:definition "ZIL library function that  is an alias for DEFINE except that it isn’t affected by MDL-ZIL mode: it always defines an MDL function."@en ;
              skos:editorialNote "DEFINE20 (and SETG20) are used in \"MDL-ZIL\"-files, where routines are defined with DEFINE - 42 - instead of ROUTINE, global variables are created with SETG instead of GLOBAL, etc. Presumably that was a way to run the games in MDL during development to avoid recompiling them. SETG20 and DEFINE20 are aliases for the MDL versions of SETG and DEFINE."@en ;
              skos:prefLabel "<DEFINE20 name [activation] arg-list [decl] expressions ...>"@en .


###  http://example.org/zilf/DEFINITIONS
zilf:DEFINITIONS rdf:type owl:NamedIndividual ,
                          skos:Concept ;
                 skos:broader zilf:CoreFunctions ;
                 skos:inScheme zilf:ZILF_Scheme ;
                 skos:definition """MDL package system that is exactly the same as PACKAGE except that there is no internal OBLIST with DEFINITIONS, 

See END-DEFINITIONS, INCLUDE, INCLUDE-WHEN, PACKAGE and RENTRY."""@en ;
                 skos:editorialNote "To activate a package-name INCLUDE or INCLUDE-WHEN is used."@en ;
                 skos:example """;\"Define PACKAGE\" 
<REMOVE ANSWER> ;\"Secure that ATOM not on any OBLIST\"  
<DEFINITIONS \"FOO\"> 
<SETG ANSWER 42> 
<END-DEFINITIONS> 

<TYPE? <GETPROP FOO!-PACKAGE OBLIST> OBLIST>  ;  OBLIST
<GASSIGNED? ANSWER>  ;  #FALSE
<GASSIGNED? ANSWER!-FOO!-PACKAGE>  ;  T
,ANSWER!-FOO!-PACKAGE  ;  42

<REMOVE ANSWER> ;\"Secure that ATOM not on any OBLIST\"
<INCLUDE \"FOO\">
,ANSWER  ;  42"""@en ;
                 skos:prefLabel "<DEFINITIONS package-name>"@en .


###  http://example.org/zilf/DEFMAC
zilf:DEFMAC rdf:type owl:NamedIndividual ,
                     skos:Concept ;
            skos:broader zilf:CoreFunctions ;
            skos:inScheme zilf:ZILF_Scheme ;
            skos:definition "MDL built-in function that  has the same syntax as DEFINE, but defines a MACRO instead of a FUNCTION. A MACRO is evaluated two times, the first evaluation inserts the arguments in the MACRO and creates an object that is evaluated during the second evaluation. The first evaluation is done at “top-level”, in other words during compilation. EXPAND is used to perform the first evaluation."@en ;
            skos:editorialNote "Note that two identical calls to a MACRO always generate the same result from the first evaluation."@en ;
            skos:example """<DEFMAC INC (ATM \"OPTIONAL\" (N 1))
    <FORM SET .ATM 
        <FORM + <FORM LVAL .ATM> .N>>>
<SET X 1>
<INC X 2>  ;  3
<EXPAND '<INC X 2>>  ;  <SET X <+ .X 2>>"""@en ;
            skos:prefLabel "<DEFMAC name [activation] arg-list [decl] expressions ...>"@en .


###  http://example.org/zilf/DELAY-DEFINITION
zilf:DELAY-DEFINITION rdf:type owl:NamedIndividual ,
                               skos:Concept ;
                      skos:broader zilf:CoreFunctions ;
                      skos:inScheme zilf:ZILF_Scheme ;
                      skos:definition """ZIL library function that tells ZILF that a REPLACE-DEFINITION for name should be expected thus the DEFAULT-DEFINITION never is evaluated for the name. This means that REPLACE-DEFINITION can appear after the DEFAULT-DEFINITION.

DELAY-DEFINITION also means that the body of REPLACE-DEFINITION will be evaluated at the place of REPLACE-DEFINITION. 

See DEFAULT-DEFINITION and REPLACE-DEFINITION."""@en ;
                      skos:example """;\"REPLACE can be defined after DEFAULT\" 
<DELAY-DEFINITION FOO-ROUTINE> 
<DEFAULT-DEFINITION FOO-ROUTINE <DEFINE FOO () 123>> 
<REPLACE-DEFINITION FOO-ROUTINE <DEFINE FOO () 456>>
<FOO>  ;  456

;\"DELAY means that REPLACE is evaluated at right place\" 
<DELAY-DEFINITION BAR-ROUTINE> 
<SETG BAR-RESULT 789> 
<REPLACE-DEFINITION BAR-ROUTINE 
<EVAL <FORM DEFINE BAR '() ,BAR-RESULT>>> 
<SETG BAR-RESULT 123> 
<DEFAULT-DEFINITION BAR-ROUTINE 
<EVAL <FORM DEFINE BAR '() ,BAR-RESULT>>>
<BAR>  ;  789 (\"123 without DELAY\")"""@en ;
                      skos:prefLabel "<DELAY-DEFINITION name>"@en .


###  http://example.org/zilf/DIR-SYNONYM
zilf:DIR-SYNONYM rdf:type owl:NamedIndividual ,
                          skos:Concept ;
                 skos:broader zilf:ParserSystem ;
                 skos:inScheme zilf:ZILF_Scheme ;
                 skos:definition "ZIL parser library function that creates one or more synonyms to the original direction."@en ;
                 skos:editorialNote "ZILF treats DIR-SYNONYM as an alias to SYNONYM."@en ;
                 skos:example """<DIR-SYNONYM FORE F>
<DIR-SYNONYM AFT A>
<DIR-SYNONYM PORT P>
<DIR-SYNONYM STARBOARD SB>"""@en ;
                 skos:prefLabel "<DIR-SYNONYM original synonyms ...>"@en .


###  http://example.org/zilf/DIRECTIONS
zilf:DIRECTIONS rdf:type owl:NamedIndividual ,
                         skos:Concept ;
                skos:broader zilf:ParserSystem ;
                skos:inScheme zilf:ZILF_Scheme ;
                skos:definition "ZIL parser library function that creates words in the vocabulary with the part-of-speech DIRECTION."@en ;
                skos:editorialNote "DIRECTIONS are often defined in the parser and the order is usually tightly tied to the parser. Be careful if you change these. You can use DIR-SYNONYM if you, for example, want to add FORE, AFT, PORT and STARBOARD."@en ;
                skos:example "<DIRECTIONS NORTH SOUTH EAST WEST NE NW SE SW IN OUT UP DOWN>"@en ;
                skos:prefLabel "<DIRECTIONS atoms ...>"@en .


###  http://example.org/zilf/END-DEFINITIONS
zilf:END-DEFINITIONS rdf:type owl:NamedIndividual ,
                              skos:Concept ;
                     skos:broader zilf:CoreFunctions ;
                     skos:inScheme zilf:ZILF_Scheme ;
                     skos:definition "MDL package system that is an alias of ENDBLOCK."@en ;
                     skos:editorialNote "See DEFINITIONS."@en ;
                     skos:prefLabel "<END-DEFINITIONS>"@en .


###  http://example.org/zilf/END-SEGMENT
zilf:END-SEGMENT rdf:type owl:NamedIndividual ,
                          skos:Concept ;
                 skos:broader zilf:CoreFunctions ;
                 skos:inScheme zilf:ZILF_Scheme ;
                 skos:definition "ZIL library function that terminates the current code and data group, returning to main game memory. END-SEGMENT pairs with BEGIN-SEGMENT."@en ;
                 skos:editorialNote "ZILF ignores this and always returns FALSE."@en ;
                 skos:example """; From The Abyss
<BEGIN-SEGMENT 0>
; Code
<END-SEGMENT>

; From Shogun
<BEGIN-SEGMENT RECORD>
; Code
<END-SEGMENT>"""@en ;
                 skos:historyNote "Having been used in a few InfoCom projects, BEGIN-SEGMENT was notably used in The Abyss, an unreleased interactive fiction game written by Bob Bates for Infocom under historical source code for the game, entitled The Abyss Source Code Collection."@en ;
                 skos:prefLabel "<END-SEGMENT>"@en .


###  http://example.org/zilf/ENDBLOCK
zilf:ENDBLOCK rdf:type owl:NamedIndividual ,
                       skos:Concept ;
              skos:broader zilf:CoreFunctions ;
              skos:inScheme zilf:ZILF_Scheme ;
              skos:definition "MDL built-in function that  pops back, rebinds and returns the local ATOM OBLIST to the state it had before the call to BLOCK. ENDBLOCK without previous BLOCK (or PACKAGE, DEFINITIONS, etc) results in an error."@en ;
              skos:example """XYZZY!-MY-OBLIST 
<SETG FIRST!- FOO> 
<BLOCK (<GETPROP MY-OBLIST OBLIST> <ROOT>)> 
<SETG SECOND!- FOO> 
<ENDBLOCK> 
<=? ,FIRST!- ,SECOND!->  ;  #FALSE"""@en ;
              skos:prefLabel "<ENDBLOCK>"@en .


###  http://example.org/zilf/ENDLOAD
zilf:ENDLOAD rdf:type owl:NamedIndividual ,
                      skos:Concept ;
             skos:broader zilf:CoreFunctions ;
             skos:inScheme zilf:ZILF_Scheme ;
             skos:definition "ZIL library function."@en ;
             skos:editorialNote "ZILF ignores this and always returns FALSE."@en ;
             skos:prefLabel "<ENDLOAD>"@en .


###  http://example.org/zilf/ENDPACKAGE
zilf:ENDPACKAGE rdf:type owl:NamedIndividual ,
                         skos:Concept ;
                skos:broader zilf:CoreFunctions ;
                skos:inScheme zilf:ZILF_Scheme ;
                skos:definition "MDL package system that is an alias to ENDBLOCK."@en ;
                skos:editorialNote "See PACKAGE."@en ;
                skos:prefLabel "<ENDPACKAGE>"@en .


###  http://example.org/zilf/ENDSECTION
zilf:ENDSECTION rdf:type owl:NamedIndividual ,
                         skos:Concept ;
                skos:broader zilf:CoreFunctions ;
                skos:inScheme zilf:ZILF_Scheme ;
                skos:definition "MDL package system that is an alias to ENDBLOCK."@en ;
                skos:editorialNote "See DEFINITIONS."@en ;
                skos:prefLabel "<ENDSECTION>"@en .


###  http://example.org/zilf/ENTRY
zilf:ENTRY rdf:type owl:NamedIndividual ,
                    skos:Concept ;
           skos:broader zilf:CoreFunctions ;
           skos:inScheme zilf:ZILF_Scheme ;
           skos:definition "MDL package system that creates/moves one or more ATOMs to the external OBLIST in a PACKAGE. ENTRY is only valid inside a PACKAGE, if it's used outside an error is raised."@en ;
           skos:editorialNote "See PACKAGE, RENTRY, USE, USE-WHEN."@en ;
           skos:example """<REMOVE ANSWER>  ;  \"Secure that ATOM not on any OBLIST\"
<PACKAGE \"FOO\">
<SETG ANSWER 42>
<1 .OBLIST>  ;  #OBLIST ((\"ANSWER\" ANSWER)) 
<2 .OBLIST>  ;  #OBLIST ((\"IFOO\" IFOO))
<ENTRY ANSWER>
<1 .OBLIST>  ;  #OBLIST ()
<2 .OBLIST>  ;  #OBLIST ((\"IFOO\" IFOO) (\"ANSWER\" ANSWER))
<ENDPACKAGE>
,ANSWER  ;  42 (the meaning of life)"""@en ;
           skos:prefLabel "<ENTRY atoms ...>"@en .


###  http://example.org/zilf/EQVB
zilf:EQVB rdf:type owl:NamedIndividual ,
                   skos:Concept ;
          skos:broader zilf:CoreFunctions ;
          skos:inScheme zilf:ZILF_Scheme ;
          skos:definition "MDL built-in function that evaluates bitwise equivalence (inverse of exclusive “or”)."@en ;
          skos:editorialNote "EQVB uses 32-bit."@en ;
          skos:example """<XORB 250 245>  
;  00000000 00000000 00000000 11111010
;  00000000 00000000 00000000 11110101
;  -----------------------------------
;  11111111 11111111 11111111 11110000 = -16"""@en ;
          skos:prefLabel "<EQVB numbers ...>"@en .


###  http://example.org/zilf/ERASE
zilf:ERASE rdf:type owl:NamedIndividual ,
                    skos:Concept ;
           skos:broader zilf:ZCodeBuiltIns ;
           skos:inScheme zilf:ZILF_Scheme ;
           skos:definition """Z-code built-in function that erases from the current cursor position. This functions behavior is dependent on the supported version.

Versions 4 and 5: if the value is 1, erase from the current cursor position to the end of its line in the current window. If the value is anything other than 1, do nothing.  

Version 6: if the value is 1, erase from the current cursor position to the end of its line in the current window. If not, erase the given number of pixels minus one across from the cursor (clipped to stay inside the right margin). The cursor does not move."""@en ;
           skos:editorialNote "ZILF supports ERASE in versions 4-."@en ;
           skos:example "<ERASE 1>  ;  Clears from cursor to end of line"@en ;
           skos:historyNote "Zapf syntax: ERASE, Inform syntax: erase_line"@en ;
           skos:prefLabel "<ERASE value>"@en .


###  http://example.org/zilf/ERROR
zilf:ERROR rdf:type owl:NamedIndividual ,
                    skos:Concept ;
           skos:broader zilf:CoreFunctions ;
           skos:inScheme zilf:ZILF_Scheme ;
           skos:definition "MDL built-in function that raises an error ([error MDL0001]) and listing values as resources. The values are usually a text explaining the error, offending ATOM, routine where it occurred and last any other information."@en ;
           skos:example """<SET A 616>
<ERROR \"MY TYPE OF ERROR.\" .A> 
; [error MDL0001] <stdin>:1: ERROR: \"MY TYPE OF ERROR.\" 616"""@en ;
           skos:prefLabel "<ERROR values ...>"@en .


###  http://example.org/zilf/EVAL
zilf:EVAL rdf:type owl:NamedIndividual ,
                   skos:Concept ;
          skos:broader zilf:CoreFunctions ;
          skos:inScheme zilf:ZILF_Scheme ;
          skos:definition "MDL built-in function that evaluates value (usually a FORM created by FORM or QUOTE)."@en ;
          skos:editorialNote "It is possible to supply an environment for EVAL. This tells EVAL from which environment. EVAL should take variable bindings. See The MDL Programming Language, chap. 9.7 for more about the environment."@en ;
          skos:example """<SET F '<+ 1 2>> 
.F ; Sets up the stack operator and operands, + 1 2.
<EVAL .F> ; Evaluates the operands with the given operator from the stack to 3.
<SET A 0>
<DEFINE WRONG ('B \"AUX\" (A 1)) <EVAL .B>> 
<DEFINE RIGHT (\"BIND\" E 'B \"AUX\" (A 1)) <EVAL .B .E>> 
<WRONG .A> ; 1
<RIGHT .A> ; 0"""@en ;
          skos:prefLabel "<EVAL value [environment]>"@en .


###  http://example.org/zilf/EVAL-IN-SEGMENT
zilf:EVAL-IN-SEGMENT rdf:type owl:NamedIndividual ,
                              skos:Concept ;
                     skos:broader zilf:CoreFunctions ;
                     skos:inScheme zilf:ZILF_Scheme ;
                     skos:definition "ZIL library function that calls EVAL on the value and returns its result."@en ;
                     skos:editorialNote "When ZILF calls EVAL, it ignores dummy1 and the optional dummy2"@en ;
                     skos:example """<SET F '<+ 1 2>> 
.F  ;  <+ 1 2>
<EVAL-IN-SEGMENT \"HINTS\" .F (1 2 3)>  ;  3"""@en ;
                     skos:prefLabel "<EVAL-IN-SEGMENT dummy1 value[dummy2]>"@en .


###  http://example.org/zilf/EVALTYPE
zilf:EVALTYPE rdf:type owl:NamedIndividual ,
                       skos:Concept ;
              skos:broader zilf:CoreFunctions ;
              skos:inScheme zilf:ZILF_Scheme ;
              skos:definition "MDL built-in function that tells the TYPE atom how it should be evaluated by EVAL. If EVALTYPE is called without a handler then the currently active handler is returned. If there is no active handler, FALSE is returned."@en ;
              skos:editorialNote "Note that it is possible to replace the handler with a new handler, even on the predefined TYPEs. See APPLYTYPE, NEWTYPE and PRINTTYPE."@en ;
              skos:example """<NEWTYPE GRITCH LIST>
<EVALTYPE GRITCH>  ;  #FALSE
<EVALTYPE GRITCH LIST>  ;  \"Evaluate GRITCH as a LIST\"
<EVALTYPE GRITCH>  ;  LIST
#GRITCH (A <+ 1 2 3> !<SET A \"BC\">)
;\"Make it like LISP!\"  ;  (A 6 !\\B !\\C)
<EVALTYPE LIST FORM>  ;  \"Evaluate LISTs as FORMs!\"
<EVALTYPE ATOM ,LVAL>  ;  \"Evaluate bare ATOM as LVAL!\"
(+ 1 2)  ;  3
(SET 'A 5)
A  ;  5"""@en ;
              skos:prefLabel "<EVALTYPE atom [handler]>"@en .


###  http://example.org/zilf/EXPAND
zilf:EXPAND rdf:type owl:NamedIndividual ,
                     skos:Concept ;
            skos:broader zilf:CoreFunctions ;
            skos:inScheme zilf:ZILF_Scheme ;
            skos:definition "MDL built-in function that performs the first EVAL of the value. In case the value is a MACRO only the first EVAL is done."@en ;
            skos:example """<DEFMAC INC2 (ATM \"OPTIONAL\" (N 1))
    <PARSE \"<SET %.ATM <+ %.ATM %.N>>\">>
<EXPAND '<INC2 X>>   --> <SET X <+ X 1>>"""@en ;
            skos:prefLabel "<EXPAND value>"@en .


###  http://example.org/zilf/FCLEAR
zilf:FCLEAR rdf:type owl:NamedIndividual ,
                     skos:Concept ;
            skos:broader zilf:ZCodeBuiltIns ;
            skos:inScheme zilf:ZILF_Scheme ;
            skos:definition "Z-code built-in function that removes flag from object."@en ;
            skos:editorialNote "ZILF supports FCLEAR in all versions."@en ;
            skos:example "<FCLEAR ,TRAP-DOOR ,OPENBIT>  ;  Marks the trap-door as closed"@en ;
            skos:historyNote "Zapf syntax: FCLEAR, Inform syntax: clear_attr"@en ;
            skos:prefLabel "<FCLEAR object flag>"@en .


###  http://example.org/zilf/FILE-LENGTH
zilf:FILE-LENGTH rdf:type owl:NamedIndividual ,
                          skos:Concept ;
                 skos:broader zilf:CoreFunctions ;
                 skos:inScheme zilf:ZILF_Scheme ;
                 skos:definition "MDL built-in function that returns the size, in bytes, of the file on channel. FILE-LENGTH returns FALSE if the file is closed."@en ;
                 skos:example """;  \"ZILF ver 0.9\"
<SET CH <OPEN \"READ\" \"../zillib/parser.zil\">>
<FILE-LENGTH .CH>  ;  115629
<CLOSE .CH>"""@en ;
                 skos:prefLabel "<FILE-LENGTH channel>"@en .


###  http://example.org/zilf/FLOAD
zilf:FLOAD rdf:type owl:NamedIndividual ,
                    skos:Concept ;
           skos:broader zilf:CoreFunctions ;
           skos:inScheme zilf:ZILF_Scheme ;
           skos:definition "MDL built-in function."@en ;
           skos:editorialNote "ZILF ignores all but the first argument and treats FLOAD as an alias to INSERT-FILE."@en ;
           skos:prefLabel "<FLOAD filename>"@en .


###  http://example.org/zilf/FONT
zilf:FONT rdf:type owl:NamedIndividual ,
                   skos:Concept ;
          skos:broader zilf:ZCodeBuiltIns ;
          skos:inScheme zilf:ZILF_Scheme ;
          skos:definition """Z-code built-in function that Sets current font to number. Returns old fonts number. If the font number is not available 0, return false.

The following numbers map to font types.
1 := Normal font
3 := Character graphics font (see section 16 in the Z-Machine Standards Document).
4 := Monospace (fixed-pitch) font"""@en ;
          skos:editorialNote "ZILF supports FONT in versions 5-."@en ;
          skos:example "<FONT 4>  ;  Sets fixed-pitch font. In versions 3-4, this is done by setting bit 1 of Flags 2 in header <PUT 0 8 <BOR <GET 0 8> 2>>"@en ;
          skos:historyNote "Zapf syntax: FONT, Inform syntax: set_font"@en ;
          skos:prefLabel "Version 5: <FONT number>, Version 6-: <FONT number [window-number]>"@en .


###  http://example.org/zilf/FORM
zilf:FORM rdf:type owl:NamedIndividual ,
                   skos:Concept ;
          skos:broader zilf:CoreFunctions ;
          skos:inScheme zilf:ZILF_Scheme ;
          skos:definition "MDL built-in function that creates a FORM without evaluating it. This is analogous to LIST and VECTOR but with \"<>\" instead of \"()\" or \"[]\". In many cases it is possible to use QUOTE to achieve the same result."@en ;
          skos:example """<FORM + 1 2>  ;  <+ 1 2> 
<DEFINE INC-FORM (A) 
    <FORM SET .A <FORM + 1 <FORM LVAL .A>>>> 
<INC-FORM X>  ;  <SET X <+ 1 .X>"""@en ;
          skos:prefLabel "<FORM values ...>"@en .


###  http://example.org/zilf/FSET
zilf:FSET rdf:type owl:NamedIndividual ,
                   skos:Concept ;
          skos:broader zilf:ZCodeBuiltIns ;
          skos:inScheme zilf:ZILF_Scheme ;
          skos:definition "Z-code built-in function adds flag to object."@en ;
          skos:editorialNote "ZILF supports FSET in all versions."@en ;
          skos:example "<FSET ,TRAP-DOOR ,OPENBIT> --> Marks the trap-door as open"@en ;
          skos:historyNote "Zapf syntax: FSET, Inform syntax: set_attr"@en ;
          skos:prefLabel "<FSET object flag>"@en .


###  http://example.org/zilf/GC
zilf:GC rdf:type owl:NamedIndividual ,
                 skos:Concept ;
        skos:broader zilf:CoreFunctions ;
        skos:inScheme zilf:ZILF_Scheme ;
        skos:definition "MDL built-in function that causes garbage collection."@en ;
        skos:editorialNote "In ZILF, GC ignores all arguments and always returns true. ZILF relies on the garbage collection in the NET framework and only implements this for compatibility."@en ;
        skos:example """<GC>  ;  T
<GC 0 T 5>  ;  T"""@en ;
        skos:prefLabel "<GC>"@en .


###  http://example.org/zilf/GC-MON
zilf:GC-MON rdf:type owl:NamedIndividual ,
                     skos:Concept ;
            skos:broader zilf:CoreFunctions ;
            skos:inScheme zilf:ZILF_Scheme ;
            skos:definition "MDL built-in function."@en ;
            skos:editorialNote "ZILF ignores this and always returns FALSE."@en ;
            skos:prefLabel "<GC-MON>"@en .


###  http://example.org/zilf/GET
zilf:GET rdf:type owl:NamedIndividual ,
                  skos:Concept ;
         skos:broader zilf:ZCodeBuiltIns ;
         skos:inScheme zilf:ZILF_Scheme ;
         skos:definition """Z-code built-in function that returns WORD-record (2 bytes) stored at offset. Note that table is an address in memory so the WORD that is returned is at table+offset*2. It is legal to use, for example, 0 as an address to retrieve information from the header. 

Also see BACK, GETB, PUT, PUTB and REST."""@en ;
         skos:editorialNote "ZILF supports GET in all versions."@en ;
         skos:example "<GET <TABLE 0 1 2 3> 2>  ;  2"@en ;
         skos:historyNote "Zapf syntax: GET, Inform syntax: loadw"@en ;
         skos:prefLabel "<GET table offset>"@en .


###  http://example.org/zilf/GETB
zilf:GETB rdf:type owl:NamedIndividual ,
                   skos:Concept ;
          skos:broader zilf:ZCodeBuiltIns ;
          skos:inScheme zilf:ZILF_Scheme ;
          skos:definition """Z-code built-in that returns BYTE-record (1 byte) stored at offset. Note that table is an address in memory so the BYTE that is returned is at table+offset. It is legal to use, for example, 0 as an address to retrieve information from the header. 

Also see BACK, GET, PUT, PUTB and REST."""@en ;
          skos:editorialNote "ZILF supports GETB in all versions."@en ;
          skos:example "<GETB <TABLE (BYTE) !\\A !\\B !\\C !\\D> 2>  ;  !\\C"@en ;
          skos:historyNote "Zapf syntax: GETB, Inform syntax: loadb"@en ;
          skos:prefLabel "<GETB table offset>"@en .


###  http://example.org/zilf/GETP
zilf:GETP rdf:type owl:NamedIndividual ,
                   skos:Concept ;
          skos:broader zilf:ZCodeBuiltIns ;
          skos:inScheme zilf:ZILF_Scheme ;
          skos:definition "Z-code built-in function that gets property from the object. Returns default value if property is not declared in the object."@en ;
          skos:editorialNote "ZILF supports GETP in all versions."@en ;
          skos:example """<OBJECT MYOBJ (MYPROP 123)>
<GETP ,MYOBJ ,P?MYPROP>  ;  123"""@en ;
          skos:historyNote "Zapf syntax: GETP, Inform syntax: get_prop"@en ;
          skos:prefLabel "<GETP object property>"@en .


###  http://example.org/zilf/GETPT
zilf:GETPT rdf:type owl:NamedIndividual ,
                    skos:Concept ;
           skos:broader zilf:ZCodeBuiltIns ;
           skos:inScheme zilf:ZILF_Scheme ;
           skos:definition "Z-code built-in that gets property address from object. Returns 0 (false) if property is not declared in the object."@en ;
           skos:editorialNote "ZILF supports GETPT in all versions."@en ;
           skos:example """<OBJECT MYOBJ (MYPROP 123)>
<GET <GETPT ,MYOBJ ,P?MYPROP> 0>  ;  123
<GETPT ,MYOBJ ,P?MYPROP2>  ;  0"""@en ;
           skos:historyNote "Zapf syntax: GETPT, Inform syntax: get_prop_addr"@en ;
           skos:prefLabel "<GETPT object property>"@en .


###  http://example.org/zilf/GLOBAL
zilf:GLOBAL rdf:type owl:NamedIndividual ,
                     skos:Concept ;
            skos:broader zilf:CoreFunctions ;
            skos:inScheme zilf:ZILF_Scheme ;
            skos:definition "ZIL library function that declares a global variable atom, which can laater be used inside a ROUTINE. The variable is initialized with default-value."@en ;
            skos:editorialNote """ZILF ignores the DECL because DECL is checked in code that runs at compile time (i.e. MDL code); however, there is no type checking for compiled code inside routines, at runtime or compile time.

For example, the following:
<GDECL (BAR) FIX> T
<SETG BAR \"fsdf\">

Outputs this error: 
[error MDL0206] <stdin>:1: expected GVAL of BAR to match DECL FIX, but got \"fdsf\""""@en ;
            skos:example "<GLOBAL MYVAR 0>"@en ;
            skos:prefLabel "<GLOBAL atom default-value [decl] [size]>"@en .


###  http://example.org/zilf/INC
zilf:INC rdf:type owl:NamedIndividual ,
                  skos:Concept ;
         skos:broader zilf:ZCodeBuiltIns ;
         skos:inScheme zilf:ZILF_Scheme ;
         skos:definition "Z-code built-in function that increments name by 1, which is signed, such that -1 increments to 0."@en ;
         skos:editorialNote "ZILF supports INC in all versions."@en ;
         skos:example """<GLOBAL X 5>
<INC ,X>  ;  X = 6"""@en ;
         skos:historyNote "Zapf syntax: INC, Inform syntax: inc"@en ;
         skos:prefLabel "<INC name>"@en .


###  http://example.org/zilf/INPUT
zilf:INPUT rdf:type owl:NamedIndividual ,
                    skos:Concept ;
           skos:broader zilf:ZCodeBuiltIns ;
           skos:inScheme zilf:ZILF_Scheme ;
           skos:definition "Z-code built-in function that  reads a single character from the keyboard. Calls routine every time*0.1 s. If routine returns true input is aborted."@en ;
           skos:editorialNote "ZILF supports INPUT in versions 4-."@en ;
           skos:example """<INPUT 1>  ;  Wait for keypress

<ROUTINE WAIT-TWO-SECONDS ()
    <INPUT 1 20 ABORT-WAIT>
> 
 
<ROUTINE ABORT-WAIT () <RETURN T>>
 
;  Pause two seconds (if not interrupted by a keypress from the keyboard
<WAIT-TWO-SECONDS>"""@en ;
           skos:historyNote "Zapf syntax: INPUT, Inform syntax: read_char"@en ;
           skos:prefLabel "<INPUT 1 [time] [routine]>"@en .


###  http://example.org/zilf/IRESTORE
zilf:IRESTORE rdf:type owl:NamedIndividual ,
                       skos:Concept ;
              skos:broader zilf:ZCodeBuiltIns ;
              skos:inScheme zilf:ZILF_Scheme ;
              skos:definition "Z-code built-in function that restores game state saved to memory by ISAVE (undo)."@en ;
              skos:editorialNote "ZILF supports IRESTORE in versions 5-."@en ;
              skos:example "<IRESTORE>"@en ;
              skos:historyNote "Zapf syntax: IRESTORE, Inform syntax: restore_undo"@en ;
              skos:prefLabel "<IRESTORE>"@en .


###  http://example.org/zilf/ISAVE
zilf:ISAVE rdf:type owl:NamedIndividual ,
                    skos:Concept ;
           skos:broader zilf:ZCodeBuiltIns ;
           skos:inScheme zilf:ZILF_Scheme ;
           skos:definition "Z-code built-in function that saves the game state to memory that later can be restored by IRESTORE (undo). Returns 0 if ISAVE fails, returns 1 if it is successful, and returns -1 if the interpreter does not handle undo."@en ;
           skos:editorialNote "ZILF supports ISAVE in versions 5-."@en ;
           skos:example "<ISAVE>"@en ;
           skos:historyNote "Zapf syntax: ISAVE, Inform syntax: save_undo"@en ;
           skos:prefLabel "<ISAVE>"@en .


###  http://example.org/zilf/ISTRING
zilf:ISTRING rdf:type owl:NamedIndividual ,
                      skos:Concept ;
             skos:broader zilf:CoreFunctions ;
             skos:inScheme zilf:ZILF_Scheme ;
             skos:definition "MDL built-in function that returns a STRING with count items all set to init (character)."@en ;
             skos:editorialNote "ISTRING is \"implicit\" or \"iterated\"."@en ;
             skos:example """<ISTRING 4 !\\A>  ;  \"AAAA\"
<SET A 64>
<ISTRING 4 '<ASCII <SET A <+ .A 1>>>>  ;  \"ABCD\""""@en ;
             skos:prefLabel "<ISTRING count [init]>"@en .


###  http://example.org/zilf/LEX
zilf:LEX rdf:type owl:NamedIndividual ,
                  skos:Concept ;
         skos:broader zilf:ZCodeBuiltIns ;
         skos:inScheme zilf:ZILF_Scheme ;
         skos:definition "Z-code built-in function that parses the text into parse. See READ for more info about parsing. The game dictionary is used if not a dictionary table (LTABLE) is supplied. If the length of the dictionary is negative, the dictionary can be unsorted. If the flag is set (true), unrecognized words are not written to parse but their slot is left unmodified. This makes it possible to run LEX against different dictionaries serially. Also see READ."@en ;
         skos:editorialNote "ZILF supports LEX in versions 4-."@en ;
         skos:example """<GLOBAL TEXTBUF <TABLE (BYTE) !\\c !\\a !\\t>>
<GLOBAL PARSEBUF <ITABLE 1 (LEXV) 0 0>>
<OBJECT CAT (SYNONYM CAT)>
<LEX ,TEXTBUF ,PARSEBUF>
<PRINTB <GET ,PARSEBUF 1>>  ;  \"cat\""""@en ;
         skos:historyNote "Zapf syntax: LEX, Inform syntax: tokenise"@en ;
         skos:prefLabel "<LEX text parse [dictionary] [flag]>"@en .


###  http://example.org/zilf/LOC
zilf:LOC rdf:type owl:NamedIndividual ,
                  skos:Concept ;
         skos:broader zilf:ZCodeBuiltIns ;
         skos:inScheme zilf:ZILF_Scheme ;
         skos:definition "Z-code built-in function that returns parent to object."@en ;
         skos:editorialNote "ZILF supports LOC in all versions."@en ;
         skos:example """<OBJECT ANIMAL>
<OBJECT CAT (LOC ANIMAL)>

<=? <LOC ,CAT> ,ANIMAL>  ;  T
<LOC ,ANIMAL>  ;  0"""@en ;
         skos:historyNote "Zapf syntax: LOC, Inform syntax: get_parent"@en ;
         skos:prefLabel "<LOC object>"@en .


###  http://example.org/zilf/LOWCORE
zilf:LOWCORE rdf:type owl:NamedIndividual ,
                      skos:Concept ;
             skos:broader zilf:ZCodeBuiltIns ;
             skos:inScheme zilf:ZILF_Scheme ;
             skos:definition "Z-code built-in function that reads and in some cases writes to the header information fields."@en ;
             skos:editorialNote "TODO: Valid values for field-spec to be listed in a separate document to be linked from this note."@en ;
             skos:example """;  Monospace bit (bit 1) in flags 2 is set
<LOWCORE FLAGS <BOR <LOWCORE FLAGS> 2>>

;  Do the same as above
<PUT 0 8 <BOR <GET 0 8> 2>>
;  Now print the 11 lower bytes in releaseid
<PRINTN <BAND <LOWCORE RELEASEID> *3777*>>"""@en ;
             skos:prefLabel "<LOWCORE field-spec [new-value]>"@en .


###  http://example.org/zilf/LOWCORE-TABLE
zilf:LOWCORE-TABLE rdf:type owl:NamedIndividual ,
                            skos:Concept ;
                   skos:broader zilf:ZCodeBuiltIns ;
                   skos:inScheme zilf:ZILF_Scheme ;
                   skos:definition "Z-code built-in function that reads the length number of bytes from field-spec and calls routine between each byte."@en ;
                   skos:editorialNote "TODO: Valid values for field-spec to be listed in a separate document to be linked from this note."@en ;
                   skos:example """;  Reads 6 bytes from SERIAL and print each byte as character 
<LOWCORE-TABLE SERIAL 6 PRINTC>"""@en ;
                   skos:prefLabel "<LOWCORE-TABLE field-spec length routine>"@en .


###  http://example.org/zilf/LTABLE
zilf:LTABLE rdf:type owl:NamedIndividual ,
                     skos:Concept ;
            skos:broader zilf:ZCodeBuiltIns ;
            skos:inScheme zilf:ZILF_Scheme ;
            skos:definition "Z-code built-in function that Defines a table containing the specified values and with the LENGTH flag."@en ;
            skos:editorialNote "See TABLE for more information about LENGTH and other flags."@en ;
            skos:prefLabel "<LTABLE [(flags ...)] values ...>"@en .


###  http://example.org/zilf/LVAL
zilf:LVAL rdf:type owl:NamedIndividual ,
                   skos:Concept ;
          skos:broader zilf:ZCodeBuiltIns ;
          skos:inScheme zilf:ZILF_Scheme ;
          skos:altLabel ".name"@en ;
          skos:definition "Z-code built-in function that gets the value of local variable name."@en ;
          skos:editorialNote "LVAL is more often used in its short for, which is .name."@en ;
          skos:example """<SET X 5> 
<LVAL X>  ;  5
.X  ;  5"""@en ;
          skos:prefLabel "<LVAL name>"@en .


###  http://example.org/zilf/MAP-CONTENTS
zilf:MAP-CONTENTS rdf:type owl:NamedIndividual ,
                           skos:Concept ;
                  skos:broader zilf:ZCodeBuiltIns ;
                  skos:inScheme zilf:ZILF_Scheme ;
                  skos:definition """Z-code built-in function that loops over all objects that have an object as parent (all children to object). For each iteration name is assigned the current child-object and next the child-object that will be name in the next iteration (0 if the current name is the last child).

For each iteration the expressions are evaluated and, if supplied, the (END expressions...) is evaluated last after all iterations."""@en ;
                  skos:example """<OBJECT SURVIVAL-KIT
(DESC \"adventure survival kit\") (WEIGHT 10)>
<OBJECT SWORD
(IN SURVIVAL-KIT) (DESC \"sword\") (WEIGHT 10)>
<OBJECT LAMP
 (IN SURVIVAL-KIT) (DESC \"brass lamp\") (WEIGHT 5)>
<OBJECT SPOON
 (IN SURVIVAL-KIT) (DESC \"chrome spoon\") (WEIGHT 2)>

<ROUTINE TEST-MAP-CONTENTS ()
    <TELL \"Your \" D ,SURVIVAL-KIT \" contains:\" CR>
    <MAP-CONTENTS (F ,SURVIVAL-KIT)
        <TELL \"    a \" D .F CR>
    >

    <TELL \"Your \" D ,SURVIVAL-KIT \" contains:\" CR>
    <MAP-CONTENTS (F N ,SURVIVAL-KIT)
        <TELL \"    a \" D .F >
        <COND (.N <TELL \" (next item is the \" D .N \")\">)>
        <TELL CR>
    >

    <BIND ((W 0))
        <SET W <GETP ,SURVIVAL-KIT ,P?WEIGHT>>
        <MAP-CONTENTS (F ,SURVIVAL-KIT)
            (END <TELL \"Total weight is = \" N .W CR>)
            <SET W <+ .W <GETP .F ,P?WEIGHT>>>
        >
    >
>

<TEST-MAP-CONTENTS>
;  Your adventure survival kit contains: 
;      a sword
;      a chrome spoon
;      a brass lamp
;  Your adventure survival kit contains:
;          a sword (next item is the chrome spoon)
;          a chrome spoon (next item is the brass lamp)
;          a brass lamp
;  Total weight is = 27"""@en ;
                  skos:prefLabel "<MAP-CONTENTS (name [next] object) [(END expressions ...)] expressions ...>"@en .


###  http://example.org/zilf/MAP-DIRECTIONS
zilf:MAP-DIRECTIONS rdf:type owl:NamedIndividual ,
                             skos:Concept ;
                    skos:broader zilf:ZCodeBuiltIns ;
                    skos:inScheme zilf:ZILF_Scheme ;
                    skos:definition """Z-code built-in function that loops over all defined directions in a room. For each iteration name is assigned the current direction and pt is the property for this direction.

For each iteration the expressions are evaluated and, if supplied, the (END expressions...) is evaluated last after all iterations."""@en ;
                    skos:example """<DIRECTIONS NORTH SOUTH EAST WEST>
 <OBJECT CENTER (DESC \"center room\")
      (NORTH TO N-ROOM)
      (WEST TO W-ROOM)>
 <OBJECT N-ROOM (DESC \"north room\")>
 <OBJECT W-ROOM (DESC \"west room\")>

 <ROUTINE TEST-MAP-DIRECTIONS ()
      <TELL \"You're in the \" D ,CENTER>
  <TELL CR \"Obvious exits:\" CR>
      <MAP-DIRECTIONS (D P ,CENTER)
          (END <TELL \"Room description done.\" CR>)
          <COND (<EQUAL? .D ,P?NORTH> <TELL \"    North\">)
                 (<EQUAL? .D ,P?SOUTH> <TELL \"    South\">)
                 (<EQUAL? .D ,P?EAST> <TELL \"    East\">)
                 (<EQUAL? .D ,P?WEST> <TELL \"    West\">)
          >
          <VERSION?
              (ZIP <TELL \" to the \" D <GETB .P ,REXIT> CR>)
              (ELSE <TELL \" to the \" D <GET .P ,REXIT> CR>)
          >
      >
 >"""@en ;
                    skos:prefLabel "<MAP-DIRECTIONS (name pt room)  [(END expressions ...)] expressions ...>"@en .


###  http://example.org/zilf/MARGIN
zilf:MARGIN rdf:type owl:NamedIndividual ,
                     skos:Concept ;
            skos:broader zilf:ZCodeBuiltIns ;
            skos:inScheme zilf:ZILF_Scheme ;
            skos:definition "Z-code built-in function that sets the left and right margin (in pixels) of the given window-number. If no window-number is specified, MARGIN sets margins in window-number 0."@en ;
            skos:editorialNote "ZILF supports MARGIN in versions 6-."@en ;
            skos:example "<MARGIN 1 1>  ;  set 1 pixel margin in window 0"@en ;
            skos:historyNote "Zapf syntax: MARGIN, Inform syntax: set_margins"@en ;
            skos:prefLabel "<MARGIN left right [window-number]>"@en .


###  http://example.org/zilf/MENU
zilf:MENU rdf:type owl:NamedIndividual ,
                   skos:Concept ;
          skos:broader zilf:ZCodeBuiltIns ;
          skos:inScheme zilf:ZILF_Scheme ;
          skos:definition "Z-code built-in function that controls menu 3- (not menu 0-2, they are system menus). The table is a LTABLE of LTABLE. Item 1 being the menu name. Item 2- are the entries."@en ;
          skos:editorialNote "ZILF supports MENU in versions 6-."@en ;
          skos:example """;  Example from Journey
<GLOBAL MAC-SPECIAL-MENU 
    <LTABLE <TABLE (STRING LENGTH) \"Journey\"> 
        <TABLE (STRING LENGTH) \"Essences\"> 
        <TABLE (STRING LENGTH) \"No Defaults\">>> 
... 
<MENU 3 ,MAC-SPECIAL-MENU>"""@en ;
          skos:historyNote "Zapf syntax: MENU, Inform syntax: make_menu"@en ;
          skos:prefLabel "<MENU number table>"@en .


###  http://example.org/zilf/MOD
zilf:MOD rdf:type owl:NamedIndividual ,
                  skos:Concept ;
         skos:broader zilf:ZCodeBuiltIns ;
         skos:inScheme zilf:ZILF_Scheme ;
         skos:definition "Z-code built-in function that Returns remainder of 16-bit signed division. number2 is not allowed to be 0 (\"Division by zero\")."@en ;
         skos:editorialNote "ZILF supports MOD in all versions."@en ;
         skos:example """<MOD 15 4>  ;  3
<MOD -15 4>  ;  -3
<MOD -15 -4>  ;  -3
<MOD 15 -4>  ;  3"""@en ;
         skos:historyNote "Zapf syntax: MOD, Inform syntax: mod"@en ;
         skos:prefLabel "<MOD number1 number2>"@en .


###  http://example.org/zilf/NEW-ADD-WORD
zilf:NEW-ADD-WORD rdf:type owl:NamedIndividual ,
                           skos:Concept ;
                  skos:broader zilf:ParserSystem ;
                  skos:inScheme zilf:ZILF_Scheme ;
                  skos:definition "ZIL parser library function that is an alias to ADD-WORD."@en ;
                  skos:prefLabel "<NEW-ADD-WORD atom-or-string [type] [value] [flags]>"@en .


###  http://example.org/zilf/OBJECT
zilf:OBJECT rdf:type owl:NamedIndividual .


###  http://example.org/zilf/OR
zilf:OR rdf:type owl:NamedIndividual ,
                 skos:Concept ;
        skos:broader zilf:CoreFunctions ;
        skos:inScheme zilf:ZILF_Scheme ;
        skos:definition "MDL built-in function that is a boolean OR. Requires that one of the expressions evaluates to true to return true. Exits on the first expression that evaluates to true (rest of expressions are not evaluated)."@en ;
        skos:editorialNote "Because false is its own TYPE outside a routine OR returns #FALSE if all expressions are false or the value of the first true expression."@en ;
        skos:example """<OR <=? 1 2> <=? 1 1>>  ;  True 
 <OR <=? 1 1> <SET X 2>> ;  X is never set to 2 because first predicate evaluates to true 
 <SET X <OR 0 1 2 3>>  ;  X is set to 0 
 <SET X <OR <> 1 2 3>>  ;  X is set to 1"""@en ;
        skos:prefLabel "<OR expressions...>"@en .


###  http://example.org/zilf/ObjectProperties
zilf:ObjectProperties rdf:type owl:NamedIndividual ,
                               skos:Concept ;
                      skos:broader zilf:ObjectSystem ;
                      skos:narrower zilf:PropAdjective ,
                                    zilf:PropDesc ,
                                    zilf:PropFlags ,
                                    zilf:PropSynonym ;
                      skos:prefLabel "Object Properties"@en .


###  http://example.org/zilf/ObjectSystem
zilf:ObjectSystem rdf:type owl:NamedIndividual ,
                           skos:Concept ;
                  skos:narrower zilf:OBJECT ,
                                zilf:ObjectProperties ;
                  skos:topConceptOf zilf:ZILF_Scheme ;
                  skos:prefLabel "Object System"@en .


###  http://example.org/zilf/PICFILE
zilf:PICFILE rdf:type owl:NamedIndividual ,
                      skos:Concept ;
             skos:broader zilf:CoreFunctions ;
             skos:inScheme zilf:ZILF_Scheme ;
             skos:definition "ZIL library function that is a compiler directive used to associate a graphics resource file with a game, and Infocom's version of PICFILE translates to a ZAP .PICFILE directive."@en ;
             skos:editorialNote "The current version of ZILF ignores PICFILE and always returns FALSE because modern interpreters do not support Infocom's graphics format. The next release of ZILF will bundle images into Blorb files (without ZAPF)."@en ;
             skos:prefLabel "<PICFILE>"@en .


###  http://example.org/zilf/PICINF
zilf:PICINF rdf:type owl:NamedIndividual ,
                     skos:Concept ;
            skos:broader zilf:ZCodeBuiltIns ;
            skos:inScheme zilf:ZILF_Scheme ;
            skos:definition "Z-code built-in function that Writes picture data from picture-number into table. Word 0 of table holds picture width and word 1 holds picture height. Then follows the picture data. If picture-number is 0, the number of available pictures is written into word 0 of table and release number of picture file is written into word 1."@en ;
            skos:editorialNote "ZILF currently supports PICINF in versions 6-."@en ;
            skos:example """<GLOBAL MYPIC <ITABLE 2048 0>>
<PICINFO 1 ,MYPIC>  ;  Writes picture data into MYPIC"""@en ;
            skos:historyNote "Zapf syntax: PICINF, Inform syntax: picture_data"@en ;
            skos:prefLabel "<PICINF picture-number table>"@en .


###  http://example.org/zilf/PICSET
zilf:PICSET rdf:type owl:NamedIndividual ,
                     skos:Concept ;
            skos:broader zilf:ZCodeBuiltIns ;
            skos:inScheme zilf:ZILF_Scheme ;
            skos:definition "Z-code built-in function that gives the interpreter a table of picture numbers that the interpreter can then unpack from disc and cache in memory."@en ;
            skos:editorialNote "ZILF currently supports PICSET in versions 6-."@en ;
            skos:example """; From Zork Zero
<PICSET ,B-PICSET-TBL>"""@en ;
            skos:historyNote "Zapf syntax: PICSET, Inform syntax: picture_table"@en ;
            skos:prefLabel "<PICSET table>"@en .


###  http://example.org/zilf/PNAME
zilf:PNAME rdf:type owl:NamedIndividual ,
                    skos:Concept ;
           skos:broader zilf:CoreFunctions ;
           skos:inScheme zilf:ZILF_Scheme ;
           skos:definition "MDL built-in function for \"printed name\", which returns a newly created string copy of the atom's pname."@en ;
           skos:editorialNote "PNAME never prints an ATOMs trailers, unlike UNPARSE, and is therefore quicker."@en ;
           skos:example """<PNAME FOO> ; \"FOO\"
<PNAME FOO!-NEW-OBLIST> ; \"FOO\"
<UNPARSE FOO!-NEW-OBLIST> ; \"FOO!-NEW-OBLIST\""""@en ;
           skos:prefLabel "<PNAME atom>"@en .


###  http://example.org/zilf/POP
zilf:POP rdf:type owl:NamedIndividual ,
                  skos:Concept ;
         skos:broader zilf:ZCodeBuiltIns ;
         skos:inScheme zilf:ZILF_Scheme ;
         skos:definition "Z-code built-in function used inside ROUTINE that pops a value from a stack. If no stack is given, a value is popped from the game stack."@en ;
         skos:editorialNote "ZILF currently supports POP in versions 6-."@en ;
         skos:example """<PUSH .FOO>
<SET FOO some-new-value>
;code
<SET FOO <POP>>"""@en ;
         skos:historyNote "Zapf syntax: POP, Inform syntax: pull"@en ;
         skos:prefLabel "<POP [stack]>"@en .


###  http://example.org/zilf/PREP-SYNONYM
zilf:PREP-SYNONYM rdf:type owl:NamedIndividual ,
                           skos:Concept ;
                  skos:broader zilf:ParserSystem ;
                  skos:inScheme zilf:ZILF_Scheme ;
                  skos:definition "ZIL parser library function that creates one or more synonyms to the original preposition."@en ;
                  skos:editorialNote "ZILF treats PREP-SYNONYM as an alias to SYNONYM."@en ;
                  skos:example """<PREP-SYNONYM INTO IN>
<PREP-SYNONYM UPON ON>
<PREP-SYNONYM ACROSS OVER BEYOND>
<PREP-SYNONYM ABOUT REGARDING CONCERNING>"""@en ;
                  skos:prefLabel "<PREP-SYNONYM original synonyms ...>"@en .


###  http://example.org/zilf/PRIMTYPE
zilf:PRIMTYPE rdf:type owl:NamedIndividual ,
                       skos:Concept ;
              skos:broader zilf:CoreFunctions ;
              skos:inScheme zilf:ZILF_Scheme ;
              skos:definition "MDL built-in function that evaluates to the primitive type of value."@en ;
              skos:editorialNote "The primitive types are  ATOM, FIX, LIST, STRING, TABLE and VECTOR."@en ;
              skos:example """<PRIMTYPE !\\A>  ;  FIX
<PRIMTYPE <+1 2>>  ;  FIX
<PRIMTYPE \"ABC\">  ;  STRING"""@en ;
              skos:prefLabel "<PRIMTYPE value>"@en .


###  http://example.org/zilf/PRIN1
zilf:PRIN1 rdf:type owl:NamedIndividual ,
                    skos:Concept ;
           skos:broader zilf:CoreFunctions ;
           skos:inScheme zilf:ZILF_Scheme ;
           skos:definition "MDL built-in function that prints the evaluated representation of value to channel (default for channel is <LVAL OUTCHAN> - the console). PRIN1 also returns the evaluated representation of value."@en ;
           skos:example """<PRIN1 !\\A>  ;  !\\A
<PRIN1 42>  ; 42
<PRIN1 \"Hello, world!\">  ;  \"Hello, world!\"
<PRIN1 (1 2 3)>  ;  (1 2 3)
<PRIN1 <+ 1 2>>  ;  3"""@en ;
           skos:prefLabel "<PRIN1 value [channel]>"@en .


###  http://example.org/zilf/PRINC
zilf:PRINC rdf:type owl:NamedIndividual ,
                    skos:Concept ;
           skos:broader zilf:CoreFunctions ;
           skos:inScheme zilf:ZILF_Scheme ;
           skos:definition "MDL built-in function that returns the evaluated representation of value."@en ;
           skos:editorialNote "PRINC is just like PRIN1, except for STRING and CHARACTER where surrounding double quote (\") and initial !\\ is suppressed."@en ;
           skos:example """<PRINC !\\A>  ;  !\\A
<PRINC 42>  ; 42
<PRINC \"Hello, world!\">  ;  \"Hello, world!\"
<PRINC (1 2 3)>  ;  (1 2 3)
<PRINC <+ 1 2>>  ;  3"""@en ;
           skos:prefLabel "<PRINC value [channel]>"@en .


###  http://example.org/zilf/PRINT
zilf:PRINT rdf:type owl:NamedIndividual ,
                    skos:Concept ;
           skos:broader zilf:CoreFunctions ;
           skos:inScheme zilf:ZILF_Scheme ;
           rdfs:isDefinedBy """<PRINT !\\A>  ;  !\\A<space>
<PRINT 42>  ; 42<space>
<PRINT \"Hello, world!\">  ;  \"Hello, world!\"<space>
<PRINT (1 2 3)>  ;  (1 2 3)<space>
<PRINT <+ 1 2>>  ;  3<space>"""@en ;
           skos:definition "MDL built-in function that returns the evaluated representation of value."@en ;
           skos:editorialNote "PRINT is just like PRIN1, except that it first prints a CRLF, then the evaluated representation of value and lastly a space."@en ;
           skos:example """<PRINT !\\A>  ;  !\\A<space>
<PRINT 42>  ; 42<space>
<PRINT \"Hello, world!\">  ;  \"Hello, world!\"<space>
<PRINT (1 2 3)>  ;  (1 2 3)<space>
<PRINT <+ 1 2>>  ;  3<space>"""@en ;
           skos:prefLabel "<PRINT value [channel]>"@en .


###  http://example.org/zilf/PTABLE
zilf:PTABLE rdf:type owl:NamedIndividual ,
                     skos:Concept ;
            skos:broader zilf:CoreFunctions ;
            skos:inScheme zilf:ZILF_Scheme ;
            skos:definition "ZIL library function that defines a table containing the specified values and with the PURE flag (see TABLE about PURE and other flags)."@en ;
            skos:editorialNote "TABLE is a ZIL-specific structure that can be used both outside and inside ROUTINES."@en ;
            skos:example "<PTABLE 1 2 3 4>"@en ;
            skos:prefLabel "<PTABLE [(flags ...)] values ...>"@en .


###  http://example.org/zilf/PTSIZE
zilf:PTSIZE rdf:type owl:NamedIndividual ,
                     skos:Concept ;
            skos:broader zilf:ZCodeBuiltIns ;
            skos:inScheme zilf:ZILF_Scheme ;
            skos:definition "Z-code built-in function that gets the property size in bytes at property-address."@en ;
            skos:editorialNote "ZILF supports PTSIZE in all versions."@en ;
            skos:example """<OBJECT MYOBJECT (FOO 1 2 3)>
<PTSIZE <GETPT ,MYOBJECT ,P?FOO>>  ;  6"""@en ;
            skos:historyNote "Zapf syntax: PTSIZE, Inform syntax: get_prop_len"@en ;
            skos:prefLabel "<PTSIZE property-value>"@en .


###  http://example.org/zilf/PUSH
zilf:PUSH rdf:type owl:NamedIndividual ,
                   skos:Concept ;
          skos:broader zilf:ZCodeBuiltIns ;
          skos:inScheme zilf:ZILF_Scheme ;
          skos:definition "Z-code built-in function that pushes value on the game stack."@en ;
          skos:editorialNote "ZILF supports POP in all versions."@en ;
          skos:example "<PUSH 123>"@en ;
          skos:historyNote "Zapf syntax: PUT, Inform syntax: storew"@en ;
          skos:prefLabel "<PUSH value>"@en .


###  http://example.org/zilf/PUT
zilf:PUT rdf:type owl:NamedIndividual ,
                  skos:Concept ;
         skos:broader zilf:ZCodeBuiltIns ;
         skos:inScheme zilf:ZILF_Scheme ;
         skos:definition """Z-code built-in function that puts a 16-bit WORD value in the table at word position offset. Actual address is table-address+offset*2. Note that table can be a byte-address in dynamic memory. 

Also see BACK, GET, GETB, PUTB and REST."""@en ;
         skos:editorialNote "ZILF supports PUT in all versions."@en ;
         skos:example """<PUT ,MYTABLE 1 123>  ;  Stores 123 at position 1 in MYTABLE
<PUT 0 8 <BOR <GET 0 8> 2>>  ;  Sets bit 1 in Flags 2 in header (force monospace)"""@en ;
         skos:historyNote "Zapf syntax: PUT, Inform syntax: storew"@en ;
         skos:prefLabel "<PUT table offset value>"@en .


###  http://example.org/zilf/PUTB
zilf:PUTB rdf:type owl:NamedIndividual ,
                   skos:Concept ;
          skos:broader zilf:ZCodeBuiltIns ;
          skos:inScheme zilf:ZILF_Scheme ;
          skos:definition """Z-code built-in function that puts a byte value in the table at byte position offset. The actual address is table-address+offset. Note that table can be a byte-address in dynamic memory.

Also see BACK, GET, GETB, PUT and REST."""@en ;
          skos:editorialNote "ZILF supports PUTB in all versions."@en ;
          skos:example "<PUTB ,MYTABLE 1 !\\A>  ;  Stores character A at position 1 in MYTABLE"@en ;
          skos:historyNote "Zapf syntax: PUTB, Inform syntax: storeb"@en ;
          skos:prefLabel "<PUTB table offset value>"@en .


###  http://example.org/zilf/PUTP
zilf:PUTP rdf:type owl:NamedIndividual ,
                   skos:Concept ;
          skos:broader zilf:ZCodeBuiltIns ;
          skos:inScheme zilf:ZILF_Scheme ;
          skos:definition "Z-code built-in function that puts value into property on the object."@en ;
          skos:editorialNote "ZILF supports PUTP in all versions."@en ;
          skos:example """<OBJECT MYOBJ (MYPROP 123)>
<PUTP ,MYOBJ ,P?MYPROP 456>  ;  Stores 456 in property MYPROP on MYOBJ"""@en ;
          skos:historyNote "Zapf syntax: PUTP, Inform syntax: put_prop"@en ;
          skos:prefLabel "<PUTP object property value>"@en .


###  http://example.org/zilf/PUTREST
zilf:PUTREST rdf:type owl:NamedIndividual ,
                      skos:Concept ;
             skos:broader zilf:CoreFunctions ;
             skos:inScheme zilf:ZILF_Scheme ;
             skos:definition """MDL built-in function that replaces the REST of list with new-rest and returns list. In other words, list is assigned the first element of list and then all the elements from new-rest. 

Note that this actually changes the list."""@en ;
             skos:example """<PUTREST (1 2 3) (A B)>  ;  (1 A B)

<SET L1 [<SET L2 (1 2 3)>]>
<PUTREST .L2 (A B)>
.L1 ;  [(1 A B)]

<SET L1 [1 2 3]>
<SET L2 <PUTREST (!.L1) (A B)>>
.L1  ;  [1 2 3]
.L2  ;  (1 A B)

<SET L1 (1 2 3 4 5 6 7 8 9)>
<PUTREST <REST .L1 3> <REST .L1 7>>
.L1  ;  (1 2 3 4 8 9)"""@en ;
             skos:prefLabel "<PUTREST list new-rest>"@en .


###  http://example.org/zilf/ParserSystem
zilf:ParserSystem rdf:type owl:NamedIndividual ,
                           skos:Concept ;
                  skos:narrower zilf:ADJ-SYNONYM ,
                                zilf:BIT-SYNONYM ,
                                zilf:BUZZ ,
                                zilf:DIR-SYNONYM ,
                                zilf:DIRECTIONS ,
                                zilf:NEW-ADD-WORD ,
                                zilf:PREP-SYNONYM ,
                                zilf:SYNONYM ,
                                zilf:SYNTAX ,
                                zilf:VERB-SYNONYM ;
                  skos:topConceptOf zilf:ZILF_Scheme ;
                  skos:prefLabel "Parser System"@en .


###  http://example.org/zilf/PropAdjective
zilf:PropAdjective rdf:type owl:NamedIndividual ,
                            skos:Concept ;
                   skos:broader zilf:ObjectProperties ;
                   skos:definition "A list of adjectives the parser accepts to identify a specific object." ;
                   skos:example "ADJECTIVE BRASS SMALL" ;
                   skos:prefLabel "ADJECTIVE"@en .


###  http://example.org/zilf/PropDesc
zilf:PropDesc rdf:type owl:NamedIndividual ,
                       skos:Concept ;
              skos:broader zilf:ObjectProperties ;
              skos:definition "A short string used to name the object in game output." ;
              skos:prefLabel "DESC"@en .


###  http://example.org/zilf/PropFlags
zilf:PropFlags rdf:type owl:NamedIndividual ,
                        skos:Concept ;
               skos:broader zilf:ObjectProperties ;
               skos:narrower zilf:BitOn ,
                             zilf:BitTake ;
               skos:definition "A collection of boolean bits (flags) that define the state or behavior of an object." ;
               skos:prefLabel "FLAGS"@en .


###  http://example.org/zilf/PropSynonym
zilf:PropSynonym rdf:type owl:NamedIndividual ,
                          skos:Concept ;
                 skos:broader zilf:ObjectProperties ;
                 skos:definition "A list of nouns the parser accepts for this object." ;
                 skos:prefLabel "SYNONYM"@en .


###  http://example.org/zilf/QUIT
zilf:QUIT rdf:type owl:NamedIndividual ,
                   skos:Concept ;
          skos:broader zilf:CoreFunctions ,
                       zilf:ZCodeBuiltIns ;
          skos:inScheme zilf:ZILF_Scheme ;
          skos:definition "MDL built-in function that exits ZILF (interpreter mode) and returns to the operating system with exit-code."@en ;
          skos:editorialNote "ZILF supports QUIT in all versions."@en ;
          skos:example "<QUIT>"@en ;
          skos:historyNote "Zapf syntax: QUIT, Inform syntax: quit"@en ;
          skos:prefLabel "<QUIT [exit-code]>"@en .


###  http://example.org/zilf/QUOTE
zilf:QUOTE rdf:type owl:NamedIndividual ,
                    skos:Concept ;
           skos:broader zilf:CoreFunctions ;
           skos:inScheme zilf:ZILF_Scheme ;
           skos:altLabel "'value"@en ;
           skos:definition "MDL built-in function that returns unevaluated value."@en ;
           skos:example """<SET F <QUOTE <+ 1 2>> ; Or <SET F '<+ 1 2>>
.F  ;  <+ 1 2>
<EVAL .F>  ;  3
'%<+ 1 2>  ;  3"""@en ;
           skos:prefLabel "<QUOTE value>"@en .


###  http://example.org/zilf/RANDOM
zilf:RANDOM rdf:type owl:NamedIndividual ,
                     skos:Concept ;
            skos:broader zilf:ZCodeBuiltIns ;
            skos:inScheme zilf:ZILF_Scheme ;
            skos:definition "Z-code built-in function that returns a random number between 1 and range. If range is negative the randomizer is reseeded with -range (absolute value of range)."@en ;
            skos:editorialNote "ZILF supports RANDOM in all versions."@en ;
            skos:example "<- <RANDOM 101> 1>  ;  Generates random number between 0-100"@en ;
            skos:historyNote "Zapf syntax: RANDOM, Inform syntax: random"@en ;
            skos:prefLabel "<RANDOM range>"@en .


###  http://example.org/zilf/READSTRING
zilf:READSTRING rdf:type owl:NamedIndividual ,
                         skos:Concept ;
                skos:broader zilf:CoreFunctions ;
                skos:inScheme zilf:ZILF_Scheme ;
                skos:definition "MDL built-in function that reads bytes from the channel into buffer-str and returns the number of bytes read into buffer-str. The buffer-str needs to have room for the input. For each call to READSTRING it either reads bytes to fill up the buffer-str or until max-length-or-stop-chars is reached. The max-length-or-stop-chars can be a FIX number of bytes or a STRING that halts input."@en ;
                skos:editorialNote "READSTRING returns the actual number of bytes read and returns 0 when the EOF is reached."@en ;
                skos:example """;\"ZILF ver 0.9\"
<SET CH <OPEN \"READ\" \"../zillib/parser.zil\">> 
<SET BUFFER <ISTRING 10>>
<READSTRING .BUFFER .CH>  ;  10
<LVAL BUFFER>  ;  \"\\\"Library h\"
<READSTRING .BUFFER .CH 6>  ;  6
<LVAL BUFFER>  ;  \"eader\\\"ry h\"
<READSTRING .BUFFER .CH \"ZIL\">  ;  10
<LVAL BUFFER>  ;  \"\\n\\n<SETG \"
<CLOSE .CH>  ;  \"\\n = CR+LF\""""@en ;
                skos:prefLabel "<READSTRING buffer-str channel [max-length-or-stop-chars]>"@en .


###  http://example.org/zilf/REMOVE
zilf:REMOVE rdf:type owl:NamedIndividual ,
                     skos:Concept ;
            skos:broader zilf:ZCodeBuiltIns ;
            skos:inScheme zilf:ZILF_Scheme ;
            skos:definition "Z-code built-in function that removes object from parent. To reattach it to another object, see MOVE."@en ;
            skos:editorialNote "ZILF supports REMOVE in all versions."@en ;
            skos:example """<OBJECT ANIMAL>
<OBJECT CAT (LOC ANIMAL)>
<REMOVE ,CAT)  ;  Detach CAT from ANIMAL"""@en ;
            skos:historyNote "Zapf syntax: REMOVE, Inform syntax: remove_obj"@en ;
            skos:prefLabel "<REMOVE object>"@en .


###  http://example.org/zilf/RENTRY
zilf:RENTRY rdf:type owl:NamedIndividual ,
                     skos:Concept ;
            skos:broader zilf:CoreFunctions ;
            skos:inScheme zilf:ZILF_Scheme ;
            skos:definition "MDL built-in function that creates/moves one or more ATOMs to <ROOT> in a PACKAGE or DEFINITION. RENTRY is only valid inside a PACKAGE or DEFINITION, if it's used outside an error is raised."@en ;
            skos:editorialNote "See DEFINITIONS, ENTRY, INCLUDE, INCLUDE-WHEN, PACKAGE, USE, USE-WHEN."@en ;
            skos:example """<REMOVE ANSWER>  ;  \"Secure that ATOM not on any OBLIST\"
<PACKAGE \"FOO\"> 
<SETG ANSWER 42> 
<RENTRY ANSWER> 
<ENDPACKAGE> 
,ANSWER  ;  42 ;”Accessible without previous USE”"""@en ;
            skos:prefLabel "<RENTRY atoms ...>"@en .


###  http://example.org/zilf/REPEAT
zilf:REPEAT rdf:type owl:NamedIndividual ,
                     skos:Concept ;
            skos:broader zilf:CoreFunctions ;
            skos:inScheme zilf:ZILF_Scheme ;
            skos:definition """MDL built-in function that  defines a program block with its own set of bindings. REPEAT is similar to BIND and PROG but unlike BIND it creates a default activation (like PROG) at the start of the block but unlike PROG it also has an automatic AGAIN at the end of the block. It is possible to name an atom to the activation but it is not necessary. A REPEAT-block repeatedly executes expressions until it encounters a RETURN statement that will exit the block. 

The decl is used to specify the valid TYPE of the variables. In its simplest form decl is formatted like: #DECL ((X) FIX), meaning that X must be of the TYPE FIX. For more information on how to format the decl see GDECL."""@en ;
            skos:editorialNote "Also see AGAIN, BIND, PROG and RETURN for more details on how to control program flow."@en ;
            skos:example """<REPEAT ((X 1)) #DECL ((X) FIX)  
    <REPEAT ((X 2)) <PRIN1 .X> <RETURN>>  
    <PRIN1 .X> <RETURN>>  ;  \"21\"
<DEFINE TEST-REPEAT () 
    <PRINC \"START \"> 
    <REPEAT ((X 0)) 
        <SET X <+ .X 1>> 
        <PRIN1 .X> 
        <COND (<=? .X 3> <RETURN>)>  ;  \"--> exit block\" 
    > 
    <PRINC \" END\"> 
> 
    <TEST-REPEAT>  ;  \"START 123 END\""""@en ;
            skos:prefLabel "<REPEAT [activation] (bindings ...) [decl] expressions ...>"@en .


###  http://example.org/zilf/REPLACE-DEFINITION
zilf:REPLACE-DEFINITION rdf:type owl:NamedIndividual ,
                                 skos:Concept ;
                        skos:broader zilf:CoreFunctions ;
                        skos:inScheme zilf:ZILF_Scheme ;
                        skos:definition """ZIL library function that  tells the compiler this block of code defined by name should replace a later  DEFAULT-DEFINITION block of code with the same name. 

This is usually used when there is a library that is inserted (like \"parser.zil\") where some definitions are possible to override."""@en ;
                        skos:editorialNote """Note that the REPLACE-DEFINITION is required to appear before the DEFAULT-DEFINITION. It is possible to do the same by setting REDEFINE to true. This actually makes it possible to change ALL definitions (it is the last one that becomes the one actually compiled).

See DEFAULT-DEFINITION and REPLACE-DEFINITION."""@en ;
                        skos:example """<REPLACE-DEFINITION MY-ROUTINE 
     <ROUTINE MY-ROUTINE ()  
        <TELL \"Replaced version of MY-ROUTINE\" CR> 
    > 
> 
<DEFAULT-DEFINITION MY-ROUTINE 
    <ROUTINE MY-ROUTINE ()  
        <TELL \"Original version of MY-ROUTINE\" CR> 
    > 
> 
<MY-ROUTINE>  ;  \"Replaced version of MY-ROUTINE\""""@en ;
                        skos:prefLabel "<REPLACE-DEFINITION name body ...>"@en .


###  http://example.org/zilf/RFALSE
zilf:RFALSE rdf:type owl:NamedIndividual ,
                     skos:Concept ;
            skos:broader zilf:ZCodeBuiltIns ;
            skos:inScheme zilf:ZILF_Scheme ;
            skos:definition "Z-code built-in function that  always exits routine and returns false (0). Note that this differs from RETURN that can both exit program blocks and routines."@en ;
            skos:editorialNote "ZILF supports RFALSE in all versions."@en ;
            skos:example "<RFALSE>"@en ;
            skos:historyNote "Zapf syntax: RFALSE, Inform syntax: rfalse"@en ;
            skos:prefLabel "<RFALSE>"@en .


###  http://example.org/zilf/RFATAL
zilf:RFATAL rdf:type owl:NamedIndividual ,
                     skos:Concept ;
            skos:broader zilf:ZCodeBuiltIns ;
            skos:inScheme zilf:ZILF_Scheme ;
            skos:definition "Z-code built-in function that always exits routine and returns FATAL-VALUE (2). Note that this differs from RETURN that can both exit program blocks and routines."@en ;
            skos:example "<RFATAL>"@en ;
            skos:prefLabel "<RFATAL>"@en .


###  http://example.org/zilf/ROOT
zilf:ROOT rdf:type owl:NamedIndividual ,
                   skos:Concept ;
          skos:broader zilf:CoreFunctions ;
          skos:inScheme zilf:ZILF_Scheme ;
          skos:definition "MDL built-in function that returns the OBLIST containing names of primitives (the same as <2 .OBLIST>)."@en ;
          skos:editorialNote "Initially contains all predefined SUBRs or FSUBRs, as well as OBLIST, DEFAULT, T, etc."@en ;
          skos:example "<ROOT>"@en ;
          skos:prefLabel "<ROOT>"@en .


###  http://example.org/zilf/ROUTINE
zilf:ROUTINE rdf:type owl:NamedIndividual ,
                      skos:Concept ;
             skos:broader zilf:CoreFunctions ;
             skos:inScheme zilf:ZILF_Scheme ;
             skos:definition "ZIL library function that is the central building block of a ZIL-program. Inside the ROUTINE it is only possible to use the reduced instruction set that can be executed on the Z-machine. It is the instructions inside the ROUTINEs that are compiled to the actual ZIP-program."@en ;
             skos:editorialNote """ROUTINE defines a program block with its own set of bindings. It is possible to specify an activation-atom to use as an argument to control the RETURN statement inside the ROUTINE. 

The arg-list is formatted the same way as FUNCTION, but the legal tokens is reduced to these:

Arguments: The required arguments for this ROUTINE. The arguments are bound to local variables inside this ROUTINE. 

\"OPT\": The optional arguments for this ROUTINE. The arguments are bound to local variables inside this ROUTINE and can be defined with a default value. \"OPTIONAL\" is an alias for \"OPT\".

\"AUX\": Followed by any number of ATOMs that becomes local variables inside this ROUTINE and can be defined with a default value. \"EXTRA\" is a alias for \"AUX\". 

\"NAME\": Followed by an ATOM that becomes the activation-atom for this ROUTINE. This is equivalent to naming the activation-atom  before the arg-list. \"ACT\" is an alias for \"NAME\". 

Default values for \"OPT\" and \"AUX\" are defined by a two-element LIST whose first element is the ATOM and the second element it is assigned to.

<ROUTINE TEST (\"AUX\" (X 1) (Y 2)) <+ .X .Y>>  Means that the local variables X and Y are initially assigned 1 and 2. After the arg-list follows the ZIL-instructions that makes up the body of the ROUTINE."""@en ;
             skos:example """;\"Move all child objects from object src to object dst\" 
    <ROUTINE MOVE-INVENTORY (SRC DST \"AUX\" X N) 
        <SET X <FIRST? .SRC>> 
        <REPEAT () 
            <COND (.X 
                <SET N <NEXT? .X>> 
                <MOVE .X .DST> 
                <SET X .N>) 
            (T <RETURN>)>>>"""@en ;
             skos:prefLabel "<ROUTINE name [activation-atom] arg-list body ...>"@en .


###  http://example.org/zilf/RSTACK
zilf:RSTACK rdf:type owl:NamedIndividual ,
                     skos:Concept ;
            skos:broader zilf:ZCodeBuiltIns ;
            skos:inScheme zilf:ZILF_Scheme ;
            skos:definition "Z-code built-in function that pops value from the game stack and returns that value."@en ;
            skos:editorialNote "ZILF supports RSTACK in all versions."@en ;
            skos:example """<PUSH 42>
<RSTACK>  ;  Returns 42"""@en ;
            skos:historyNote "Zapf syntax: RSTACK, Inform syntax: ret_popped"@en ;
            skos:prefLabel "<RSTACK>"@en .


###  http://example.org/zilf/RTRUE
zilf:RTRUE rdf:type owl:NamedIndividual ,
                    skos:Concept ;
           skos:broader zilf:ZCodeBuiltIns ;
           skos:inScheme zilf:ZILF_Scheme ;
           skos:definition "Z-code built-in function that always exits routine and returns true (1). Note that this differs from RETURN that can both exit program blocks and routines."@en ;
           skos:editorialNote "ZILF supports RTRUE in all versions."@en ;
           skos:example "<RTRUE>"@en ;
           skos:historyNote "Zapf syntax: RTRUE, Inform syntax: rtrue"@en ;
           skos:prefLabel "<RTRUE>"@en .


###  http://example.org/zilf/SAVE
zilf:SAVE rdf:type owl:NamedIndividual ,
                   skos:Concept ;
          skos:broader zilf:ZCodeBuiltIns ;
          skos:inScheme zilf:ZILF_Scheme ;
          skos:definition """Z-code built-in function that saves a game state that later can be restored. All questions about filename and path are asked by the interpreter. 

SAVE returns 0 if SAVE fails and 1 if it is successful. 

SAVE also can return 2. That means this is a continuation from a successful RESTORE.

See RESTORE on code example on SAVE and RESTORE.

See The Inform Designer’s Manual (ch. §42, p. 319) and The Z-machine Standards Document for a description about how to SAVE and RESTORE auxiliary files."""@en ;
          skos:editorialNote "ZILF supports SAVE in all versions."@en ;
          skos:example """;  Versions 1-4
<SAVE>

;  Version 5-
;  From Zork Zero
<ROUTINE SOFT-SAVE-DEFS ()
    <CLEAR 0>
    <SCREEN 0>
    <COND (<NOT <SAVE ,FKEY-TBL
                             ,FKEYS-STRTABLE-LEN
                             ,DEFS-NAME>>
                    <TELL \"Failed.\">)>
    <CLEAR 0>
    <SCREEN ,SOFT-WINDOW>
    <RFALSE>>

<ROUTINE SOFT-RESTORE-DEFS ()
    <CLEAR 0>
    <SCREEN 0>
    <COND (<NOT <RESTORE ,FKEY-TBL ,FKEYS-STRTABLE-LEN ,DEFS-NAME>>
                    <TELL \"Failed.\">)>
    <CLEAR 0>
    <SCREEN ,SOFT-WINDOW>
    <RFALSE>>"""@en ;
          skos:historyNote "Zapf syntax: SAVE, Inform syntax: save"@en ;
          skos:prefLabel """<SAVE>  ;  Versions 1-4, 
<SAVE [table] [bytes] [filename]>  ;  Versions 5-"""@en .


###  http://example.org/zilf/SCREEN
zilf:SCREEN rdf:type owl:NamedIndividual ,
                     skos:Concept ;
            skos:broader zilf:ZCodeBuiltIns ;
            skos:inScheme zilf:ZILF_Scheme ;
            skos:definition "Z-code built-in function that selects window-number for text output. Note that in versions 3-5 only the lower screen (window-number = 0) has text-buffering and word-wrap."@en ;
            skos:editorialNote "ZILF supports SCREEN in versions 3-."@en ;
            skos:example """<SPLIT 3>
<SCREEN 1>
<TELL \"West of House\">  ;  Split screen in 2 (upper screen is 3 rows) 
                                               ;  and write \"West of House\" in upper screen"""@en ;
            skos:historyNote "Zapf syntax: SCREEN, Inform syntax: set_window"@en ;
            skos:prefLabel "<SCREEN window-number>"@en .


###  http://example.org/zilf/SCROLL
zilf:SCROLL rdf:type owl:NamedIndividual ,
                     skos:Concept ;
            skos:broader zilf:ZCodeBuiltIns ;
            skos:inScheme zilf:ZILF_Scheme ;
            skos:definition "Z-code built-in function that scrolls window-number up (pixels is positive) or down (pixels is negative) by the number of supplied pixels. New lines are empty (background color)."@en ;
            skos:editorialNote "ZILF supports SCROLL in versions 6-."@en ;
            skos:example """;  From Arthur
<SETG GL-AUTHOR-SIZE <RT-COUNT-LINES ,K-DIROUT-TBL>>
<SET AY <* ,GL-AUTHOR-SIZE ,GL-FONT-Y>>
<SCROLL 0 .AY>"""@en ;
            skos:historyNote "Zapf syntax: SCROLL, Inform syntax: scroll_window"@en ;
            skos:prefLabel "<SCROLL window-number pixels>"@en .


###  http://example.org/zilf/SET
zilf:SET rdf:type owl:NamedIndividual ,
                  skos:Concept ;
         skos:broader zilf:CoreFunctions ,
                      zilf:ZCodeBuiltIns ;
         skos:inScheme zilf:ZILF_Scheme ;
         skos:definition """MDL built-in function that asigns a value to the local atom. It is possible to supply an environment for SET. See EVAL for more about the environment.

Z-code built-in function that stores value in local variable name."""@en ;
         skos:editorialNote "ZILF supports SET in all versions."@en ;
         skos:example """MDL: <PROG (X) <SET X 5> <RETURN .X>>  ;  Returns 5 after setting X.
Zapf: <SET MYVAR 42>  ;  Store 42 in local variable MYVAR"""@en ;
         skos:historyNote "Zapf syntax: SET, Inform syntax: store"@en ;
         skos:prefLabel """MDL: <SET atom value [environment]>,
Zapf: <SET name value>"""@en .


###  http://example.org/zilf/SETG
zilf:SETG rdf:type owl:NamedIndividual ,
                   skos:Concept ;
          skos:broader zilf:CoreFunctions ,
                       zilf:ZCodeBuiltIns ;
          skos:definition """MDL built-in function that assigns a value to the global atom. If an atom is already assigned a value, it is changed.

Z-code built-in function that Store value in global variable name. The name variable must be declared with GLOBAL outside the ROUTINE."""@en ;
          skos:editorialNote "ZILF supports SETG in all versions."@en ;
          skos:example "MDL/Zapf: <SETG MYVAR 42>  ;  Store 42 in global atom MYVAR"@en ;
          skos:historyNote "Zapf syntax: SETG, Inform syntax: store"@en ;
          skos:prefLabel """MDL: <SETG atom value>,
Zapf: <SETG name value>"""@en .


###  http://example.org/zilf/SETG20
zilf:SETG20 rdf:type owl:NamedIndividual ,
                     skos:Concept ;
            skos:broader zilf:CoreFunctions ;
            skos:inScheme zilf:ZILF_Scheme ;
            skos:definition "ZIL library function that assigs a value to the global atom. If an atom is already assigned a value, it is changed. SETG20 is an alias for SETG."@en ;
            skos:example "<SETG20 MYVAR 42> ; Store 42 in global atom MYVAR"@en ;
            skos:prefLabel "<SETG20 atom value>"@en .


###  http://example.org/zilf/SOUND
zilf:SOUND rdf:type owl:NamedIndividual ,
                    skos:Concept ;
           skos:broader zilf:ZCodeBuiltIns ;
           skos:inScheme zilf:ZILF_Scheme ;
           skos:definition """Z-code built-in  that plays sound number (1 = high-pitch beep, 2 = low-pitch beep and 3- is user defined). 

Valid entries for effect are 1 = prepare, 2 = start, 3 = stop and 4 = finished with. 

The volrep is calculated as 256 * repetitions + volume. Repetitions can be 0-255 (255 = infinite) and volume 1-8, 255 (1 =  quiet, 8 = loud, 255 = loudest possible. Note that repetitions only are valid from version 5 onward. For version 5 and later a repetition equal to 0 is considered illegal but it’s suggested that interpreters should treat this as a request to play the sound once. 

If routine is supplied it is called after sound is finished. 

See The Inform Designer’s Manual (ch. §42, p. 315-316 and ch. §43) and The Z-machine Standards Document for a description about how to include sound in games."""@en ;
           skos:editorialNote "ZILF supports SOUND in versions 3-."@en ;
           skos:example """;  From Sherlock
<ROUTINE RT-S-CAB-ARRIVES ()
    <COND (<==? ,CAB-RAMP 0>
        <SOUND ,S-HORSE ,S-START 4>)
        (T
        <SETG CAB-RAMP <- ,CAB-RAMP 1>>
        <SOUND ,S-HORSE ,S-START <- 2 ,CAB-RAMP> 1 RT-S-CAB-ARRIVES>)>>"""@en ;
           skos:historyNote "Zapf syntax: SOUND, Inform syntax: sound_effect"@en ;
           skos:prefLabel """<SOUND number [effect] [volume]>  ;  \"Versions 3-4\",
<SOUND number [effect] [volrep] [routine]>  ;  \"Versions 5-\""""@en .


###  http://example.org/zilf/SPLIT
zilf:SPLIT rdf:type owl:NamedIndividual ,
                    skos:Concept ;
           skos:broader zilf:ZCodeBuiltIns ;
           skos:inScheme zilf:ZILF_Scheme ;
           skos:definition """Z-code built-in function that splits the screen  in two parts with the upper part having number rows. If number is 0 the screen is unsplit.The upper screen is window-number 1 and the lower screen is window-number 0.

See SCREEN for example on how to use SPLIT."""@en ;
           skos:editorialNote "ZILF supports SPLIT in versions 3-."@en ;
           skos:example """<SPLIT 3>
<SCREEN 1>
<TELL \"West of House\">  ;  Split screen in 2 (upper screen is 3 rows) 
                                               ;  and write \"West of House\" in upper screen"""@en ;
           skos:historyNote "Zapf syntax: SPLIT, Inform syntax: split_window"@en ;
           skos:prefLabel "<SPLIT number>"@en .


###  http://example.org/zilf/SPNAME
zilf:SPNAME rdf:type owl:NamedIndividual ,
                     skos:Concept ;
            skos:broader zilf:CoreFunctions ;
            skos:inScheme zilf:ZILF_Scheme ;
            skos:definition "MDL built-in function for \"shared printed name\", which should return the same string of the atom's pname that is in its OBLIST (i.e. pointing to the same storage and therefore not able to change or modify)."@en ;
            skos:editorialNote "ZILF treats SPNAME as an alias to PNAME and returns a string copy of the atom’s pname."@en ;
            skos:example "<SPNAME atom>"@en ;
            skos:prefLabel "<SPNAME atom>"@en .


###  http://example.org/zilf/STRING
zilf:STRING rdf:type owl:NamedIndividual ,
                     skos:Concept ;
            skos:broader zilf:CoreFunctions ;
            skos:inScheme zilf:ZILF_Scheme ;
            skos:definition "MDL built-in function that returns a concatenated string of all values. values can be character or string."@en ;
            skos:editorialNote "A string is a block of contiguous bytes where each byte holds a character. See more about STRING  structure in The MDL Programming Language, Appendix 1."@en ;
            skos:example "<STRING !\\A <ASCII 66> \"CD\"> ; \"ABCD\""@en ;
            skos:prefLabel "<STRING values ...>"@en .


###  http://example.org/zilf/SYNONYM
zilf:SYNONYM rdf:type owl:NamedIndividual ,
                      skos:Concept ;
             skos:broader zilf:ParserSystem ;
             skos:inScheme zilf:ZILF_Scheme ;
             skos:definition "ZIL parser library function that creates one or more synonyms to the original verb, adjective, preposition or direction. Instead of  SYNONYM it is also possible to use VERB-SYNONYM, ADJ-SYNONYM, PREP-SYNONYM and DIR-SYNONYM for verbs, adjectives, prepositions and directions respectively, ZILF handles them all like aliases to SYNONYM."@en ;
             skos:editorialNote "Note that due to the way words, especially adjectives and nouns,  are stored in the vocabulary synonyms for adjectives only work in version 3 (ZIP) games."@en ;
             skos:example """<SYNONYM NORTH FORE>
<SYNONYM SOUTH AFT>
<SYNONYM WEST PORT>
<SYNONYM EAST STARBOARD>

<SYNTAX PUT OBJECT = V-INSERT>
<VERB-SYNONYM PUT SLIDE DIP SOAK>"""@en ;
             skos:prefLabel "<SYNONYM original synonyms ...>"@en .


###  http://example.org/zilf/SYNTAX
zilf:SYNTAX rdf:type owl:NamedIndividual ,
                     skos:Concept ;
            skos:broader zilf:ParserSystem ;
            skos:prefLabel "SYNTAX"@en .


###  http://example.org/zilf/THROW
zilf:THROW rdf:type owl:NamedIndividual ,
                    skos:Concept ;
           skos:broader zilf:ZCodeBuiltIns ;
           skos:inScheme zilf:ZILF_Scheme ;
           skos:definition "Z-code built-in function that is used with CATCH. THROW sets the stack to stack-frame and returns value (the result is that execution returns from the routine where the stack-frame was \"caught\" with value as the routines return value. Also see CATCH."@en ;
           skos:editorialNote "ZILF supports THROW in versions 5-."@en ;
           skos:example """<ROUTINE TEST-CATCH (\"AUX\" X)
    <SET X <CATCH>>
    <THROWER .X>
    123
>

<ROUTINE THROWER (F)
    <THROW 456 .F>
>

<TEST-CATCH>  ;  456"""@en ;
           skos:historyNote "Zapf syntax: THROW, Inform syntax: throw"@en ;
           skos:prefLabel "<THROW value stack-frame>"@en .


###  http://example.org/zilf/TIME
zilf:TIME rdf:type owl:NamedIndividual ,
                   skos:Concept ;
          skos:broader zilf:CoreFunctions ;
          skos:inScheme zilf:ZILF_Scheme ;
          skos:definition "MDL built-in function that is used for measuring CPU execution time, typically used for debugging ZILCH."@en ;
          skos:editorialNote "ZILF ignores this and always returns 1, because modern IDE's offer different methods of debugging ZILCH."@en ;
          skos:example "<TIME>"@en ;
          skos:prefLabel "<TIME>"@en .


###  http://example.org/zilf/TOP
zilf:TOP rdf:type owl:NamedIndividual ,
                  skos:Concept ;
         skos:broader zilf:CoreFunctions ;
         skos:inScheme zilf:ZILF_Scheme ;
         skos:definition "MDL built-in function that returns array with all elements put back in  array. TOP only works on the structures VECTOR or STRING (arrays) and not on a LIST (a LIST is only pointing forward)."@en ;
         skos:editorialNote "The returned array is not a copy but pointing to the same array with another starting element. Also see BACK, NTH, PUT, REST and SUBSTRUC."@en ;
         skos:example """<SETG STRUCT1 [1 2 3 4 5]>  ;  STRUCT1 = [1 2 3 4 5]
<SETG STRUCT2 <REST ,STRUCT1 2>>  ;  STRUCT2 = [3 4 5]
<TOP ,STRUCT2>  ;  STRUCT2 = [1 2 3 4 5]"""@en ;
         skos:prefLabel "<TOP array>"@en .


###  http://example.org/zilf/USL
zilf:USL rdf:type owl:NamedIndividual ,
                  skos:Concept ;
         skos:broader zilf:ZCodeBuiltIns ;
         skos:inScheme zilf:ZILF_Scheme ;
         skos:definition "Z-code built-in function that updates the status line. This command is only recognized in version 3."@en ;
         skos:editorialNote "ZILF supports USL in version 3."@en ;
         skos:example "<USL>"@en ;
         skos:historyNote "Zapf syntax: USL, Inform syntax: show_status"@en ;
         skos:prefLabel "<USL>"@en .


###  http://example.org/zilf/VALUE
zilf:VALUE rdf:type owl:NamedIndividual ,
                    skos:Concept ;
           skos:broader zilf:CoreFunctions ,
                        zilf:ZCodeBuiltIns ;
           skos:inScheme zilf:ZILF_Scheme ;
           skos:definition """MDL built-in function that returns the value of an atom. If  the atom has an LVAL then the LVAL is returned, otherwise the GVAL of the atom is returned. It is possible to supply an environment for VALUE. See EVAL for more about the environment.

Z-code built-in function that loads name/number. Note that this command is mostly redundant and rarely used."""@en ;
           skos:editorialNote "ZILF supports VALUE in all versions."@en ;
           skos:example """;  MDL
<SETG X 3>
<SET X 4>
<VALUE X>  ;  4
<UNASSIGN X>
<VALUE X>  ;  3

;  Zapf
<VALUE X>  ;  Loads local or global variable X. Recommended to use LVAL or GVAL instead (.X or ,X)"""@en ;
           skos:historyNote "Zapf syntax: VALUE, Inform syntax: load"@en ;
           skos:prefLabel """MDL: <VALUE atom [environment]>, 
Zapf: <VALUE name/number>"""@en .


###  http://example.org/zilf/VERB-SYNONYM
zilf:VERB-SYNONYM rdf:type owl:NamedIndividual ,
                           skos:Concept ;
                  skos:broader zilf:ParserSystem ;
                  skos:inScheme zilf:ZILF_Scheme ;
                  skos:definition "ZIL parser library function that creates one or more synonyms to the original verb."@en ;
                  skos:editorialNote "ZILF treats VERB-SYNONYM as an alias to SYNONYM."@en ;
                  skos:example """<VERB-SYNONYM SAY TELL>
<VERB-SYNONYM GO MOVE>
<VERB-SYNONYM MAKE CREATE BUILD>
<VERB-SYNONYM GET OBTAIN ACQUIRE>"""@en ;
                  skos:prefLabel "<VERB-SYNONYM original synonyms ...>"@en .


###  http://example.org/zilf/VERIFY
zilf:VERIFY rdf:type owl:NamedIndividual ,
                     skos:Concept ;
            skos:broader zilf:ZCodeBuiltIns ;
            skos:inScheme zilf:ZILF_Scheme ;
            skos:definition "Z-code built-in function that returns true if sum($0040:PLENTH (byte 26-27 in header)) MOD $10000 = PCHKSUM (byte 28-29 in header), otherwise false."@en ;
            skos:editorialNote "ZILF supports VERIFY in all versions."@en ;
            skos:example "<VERIFY>"@en ;
            skos:historyNote "Zapf syntax: VERIFY, Inform syntax: verify"@en ;
            skos:prefLabel "<VERIFY>"@en .


###  http://example.org/zilf/WINGET
zilf:WINGET rdf:type owl:NamedIndividual ,
                     skos:Concept ;
            skos:broader zilf:ZCodeBuiltIns ;
            skos:inScheme zilf:ZILF_Scheme ;
            skos:definition "Z-code built-in function that reads property on window-number."@en ;
            skos:editorialNote "ZILF supports WINGET in versions 6-."@en ;
            skos:example """;  From Shogun
<ROUTINE GO
    <CLEAR -1>
    <SPLIT </ <WINGET 0 ,WHIGH> 4>>
    <ANIMATE ,CEL-TABLE>
    <QUIT>>"""@en ;
            skos:historyNote "Zapf syntax: WINGET, Inform syntax: get_wind_prop"@en ;
            skos:prefLabel "<WINGET window-number property>"@en .


###  http://example.org/zilf/WINPOS
zilf:WINPOS rdf:type owl:NamedIndividual ,
                     skos:Concept ;
            skos:broader zilf:ZCodeBuiltIns ;
            skos:inScheme zilf:ZILF_Scheme ;
            skos:definition "Z-code built-in function that moves window-number to position row column (pixels). (1, 1) is in the top left corner."@en ;
            skos:editorialNote "ZILF supports WINPOS in versions 6-."@en ;
            skos:example """;  From Shogun
<ROUTINE WINDEF (W TOP LEFT HIGH WIDE)
    <WINPOS .W .TOP .LEFT>
    <WINSIZE .W .HIGH .WIDE>>"""@en ;
            skos:historyNote "Zapf syntax: WINPOS, Inform syntax: move_window"@en ;
            skos:prefLabel "<WINPOS window-number row column>"@en .


###  http://example.org/zilf/WINPUT
zilf:WINPUT rdf:type owl:NamedIndividual ,
                     skos:Concept ;
            skos:broader zilf:ZCodeBuiltIns ;
            skos:inScheme zilf:ZILF_Scheme ;
            skos:definition "Z-code built-in function that writes value to property window-number."@en ;
            skos:editorialNote "ZILF supports WINPUT in versions 6-."@en ;
            skos:example """;  From Shogun
<WINPUT 0 ,WCRFUNC
    <COND (.BORD? ,RESET-MARGIN-1)
        (ELSE ,RESET-MARGIN)>>
<COND (<EQUAL? .P ,P-OAR>
    <SET Y <+ .Y 1>>)>
<WINPUT 0 ,WCRCNT .Y>)>)>"""@en ;
            skos:historyNote "Zapf syntax: WINPUT, Inform syntax: put_wind_prop"@en ;
            skos:prefLabel "<WINPUT window-number property value>"@en .


###  http://example.org/zilf/WINSIZE
zilf:WINSIZE rdf:type owl:NamedIndividual ,
                      skos:Concept ;
             skos:broader zilf:ZCodeBuiltIns ;
             skos:inScheme zilf:ZILF_Scheme ;
             skos:definition "Z-code built-in function that changes window-number size."@en ;
             skos:editorialNote "ZILF supports WINSIZE in versions 6-."@en ;
             skos:example """;  From Arthur
<SET WX <WINGET 0 ,K-W-XSIZE>>
<WINSIZE 0 .WY .WX>"""@en ;
             skos:historyNote "Zapf syntax: WINSIZE, Inform syntax: window_size"@en ;
             skos:prefLabel "<WINSIZE window-number height width>"@en .


###  http://example.org/zilf/XPUSH
zilf:XPUSH rdf:type owl:NamedIndividual ,
                    skos:Concept ;
           skos:broader zilf:ZCodeBuiltIns ;
           skos:inScheme zilf:ZILF_Scheme ;
           skos:definition "Z-code built-in function that pushes value on the stack."@en ;
           skos:editorialNote "ZILF supports XPUSH in versions 6-."@en ;
           skos:example """<GLOBAL MY-STACK <TABLE 1 0 0 0>>
<XPUSH 123 ,MY-STACK>  ;  MY-STACK <TABLE 2 0 123 0>"""@en ;
           skos:historyNote "Zapf syntax: XPUSH, Inform syntax: push_stack"@en ;
           skos:prefLabel "<XPUSH value stack>"@en .


###  http://example.org/zilf/ZCodeBuiltIns
zilf:ZCodeBuiltIns rdf:type owl:NamedIndividual ,
                            skos:Concept ;
                   skos:inScheme zilf:ZILF_Scheme ;
                   skos:narrower zilf:BACK ,
                                 zilf:BCOM ,
                                 zilf:BTST ,
                                 zilf:BUFOUT ,
                                 zilf:CATCH ,
                                 zilf:ERASE ,
                                 zilf:FCLEAR ,
                                 zilf:FONT ,
                                 zilf:FSET ,
                                 zilf:GET ,
                                 zilf:GETB ,
                                 zilf:GETP ,
                                 zilf:GETPT ,
                                 zilf:INC ,
                                 zilf:INPUT ,
                                 zilf:IRESTORE ,
                                 zilf:ISAVE ,
                                 zilf:LEX ,
                                 zilf:LOC ,
                                 zilf:LOWCORE ,
                                 zilf:LOWCORE-TABLE ,
                                 zilf:LTABLE ,
                                 zilf:LVAL ,
                                 zilf:MAP-CONTENTS ,
                                 zilf:MAP-DIRECTIONS ,
                                 zilf:MARGIN ,
                                 zilf:MENU ,
                                 zilf:MOD ,
                                 zilf:PICINF ,
                                 zilf:PICSET ,
                                 zilf:POP ,
                                 zilf:PTSIZE ,
                                 zilf:PUSH ,
                                 zilf:PUT ,
                                 zilf:PUTB ,
                                 zilf:PUTP ,
                                 zilf:QUIT ,
                                 zilf:RANDOM ,
                                 zilf:REMOVE ,
                                 zilf:RFALSE ,
                                 zilf:RFATAL ,
                                 zilf:RSTACK ,
                                 zilf:RTRUE ,
                                 zilf:SAVE ,
                                 zilf:SCREEN ,
                                 zilf:SCROLL ,
                                 zilf:SET ,
                                 zilf:SETG ,
                                 zilf:SOUND ,
                                 zilf:SPLIT ,
                                 zilf:THROW ,
                                 zilf:USL ,
                                 zilf:VALUE ,
                                 zilf:VERIFY ,
                                 zilf:WINGET ,
                                 zilf:WINPOS ,
                                 zilf:WINPUT ,
                                 zilf:WINSIZE ,
                                 zilf:XPUSH ,
                                 zilf:ZWSTR ,
                                 <http://example.org/zilf/F?> ,
                                 <http://example.org/zilf/FIRST?> ,
                                 <http://example.org/zilf/FSET?> ,
                                 <http://example.org/zilf/IN?> ,
                                 <http://example.org/zilf/INTBL?> .


###  http://example.org/zilf/ZILF_Scheme
zilf:ZILF_Scheme rdf:type owl:NamedIndividual ,
                          skos:ConceptScheme ;
                 skos:hasTopConcept zilf:CoreFunctions ,
                                    zilf:ObjectSystem ,
                                    zilf:ParserSystem ;
                 skos:prefLabel "ZILF Reference Scheme"@en .


###  http://example.org/zilf/ZWSTR
zilf:ZWSTR rdf:type owl:NamedIndividual ,
                    skos:Concept ;
           skos:broader zilf:ZCodeBuiltIns ;
           skos:inScheme zilf:ZILF_Scheme ;
           skos:definition "Z-code built-in function that encodes length characters starting at offset from ZSCII word zscii-text and stores result in 6-byte Z-encoded dest-table."@en ;
           skos:editorialNote "ZILF supports ZWSTR in versions 5-."@en ;
           skos:example """<GLOBAL SRCBUF <TABLE (STRING) \"hello\">>
<GLOBAL DSTBUF <TABLE 0 0 0>>

<ZWSTR ,SRCBUF 5 1 ,DSTBUF> 
<PRINTB ,DSTBUF>  ;  \"hello\""""@en ;
           skos:historyNote "Zapf syntax: ZWSTR, Inform syntax: encode_text"@en ;
           skos:prefLabel "<ZWSTR src-table length offset dest-table>"@en .


###  http://example.org/zilf/BOUND?
<http://example.org/zilf/BOUND?> rdf:type owl:NamedIndividual ,
                                          skos:Concept ;
                                 skos:broader zilf:CoreFunctions ;
                                 skos:inScheme zilf:ZILF_Scheme ;
                                 skos:definition """MDL bulit-in predicate that returns true if the atom ever had a local value in the environment.

If no environment is supplied, the environment defaults to current scope. See EVAL for more about the environment."""@en ;
                                 skos:example """<SET X 42>
<ASSIGNED? X>  ;  True
<GBOUND? X>  ;  True
<GUNASSIGN X>
<GASSIGNED? X>  ;  False
<GBOUND? X>  ;  True"""@en ;
                                 skos:prefLabel "<BOUND? atom [environment]>"@en .


###  http://example.org/zilf/CHECK-VERSION?
<http://example.org/zilf/CHECK-VERSION?> rdf:type owl:NamedIndividual ,
                                                  skos:Concept ;
                                         skos:broader zilf:CoreFunctions ;
                                         skos:inScheme zilf:ZILF_Scheme ;
                                         skos:definition "ZIL library predicate that  returns TRUE if current setting of VERSION is version-spec. Valid values for version-spec are ZIP, EZIP, XZIP, YZIP and the values 3-8."@en ;
                                         skos:example """<VERSION XZIP>
<CHECK-VERSION? ZIP>  ;  #FALSE
<CHECK-VERSION? 5>  ;  T"""@en ;
                                         skos:prefLabel "<CHECK-VERSION? version-spec>"@en .


###  http://example.org/zilf/COMPILING?
<http://example.org/zilf/COMPILING?> rdf:type owl:NamedIndividual ,
                                              skos:Concept ;
                                     skos:broader zilf:CoreFunctions ;
                                     skos:inScheme zilf:ZILF_Scheme ;
                                     skos:definition "ZIL library function that is presumably  used in the MDL environment to determine if the game is compiled with ZILCH or running in the interpreter."@en ;
                                     skos:editorialNote "ZILF ignores this and always returns TRUE."@en ;
                                     skos:prefLabel "<COMPILING?>"@en .


###  http://example.org/zilf/DECL?
<http://example.org/zilf/DECL?> rdf:type owl:NamedIndividual ,
                                         skos:Concept ;
                                skos:broader zilf:CoreFunctions ;
                                skos:inScheme zilf:ZILF_Scheme ;
                                skos:definition "MDL built-in predicate that returns TRUE if value checks against pattern, otherwise FALSE. For the format of the pattern, see GDECL."@en ;
                                skos:example """;  Simple DECL
<DECL? 1 FIX>  ;  T
<DECL? \"hi\" STRING>  ;  T
<DECL? FOO STRING>  ;  #FALSE

;  OR DECL
<DECL? 1 '<OR FIX FALSE>>  ;  T
<DECL? \"hi\" '<OR VECTOR STRING>>  ;  T
<DECL? FOO '<OR STRING FIX>>  ;  #FALSE

;  Structure DECL
<DECL? '(1) '<LIST FIX>  ;  T
<DECL? '(1) '<LIST ATOM>>  ;  #FALSE
<DECL? '<1> '<LIST FIX>>  ;  #FALSE
<DECL? '<1> '<<OR FORM LIST> FIX>>  ;  T
<DECL? '<1> '<<OR <PRIMTYPE LIST> <PRIMTYPE STRING>> FIX>>  ;  T
<DECL? '(1) '<<PRIMTYPE LIST> FIX>>  ;  T
<DECL? '<1> '<<PRIMTYPE LIST> FIX>>  ;  T

;  NTH DECL
<DECL? '[\"hi\" 456 789 1011] '<VECTOR STRING [4 FIX]>>  ;  #FALSE
<DECL? '[\"hi\" 456 789 1011] '<VECTOR STRING [3 FIX]>>  ;  T
<DECL? '[\"hi\" 456 789 1011] '<VECTOR [3 FIX]>>  ;  #FALSE
<DECL? '[\"hi\" 456 789 1011] '<VECTOR STRING [2 FIX]>>  ;  T
<DECL? '[\"hi\" 456 789 1011] '<VECTOR STRING [2 FIX] FIX>>  ;  T
<DECL? '[\"hi\" 456 789 1011] '<VECTOR STRING [2 FIX] ATOM>>  ;  #FALSE
<DECL? '(1 MONEY 2 SHOW 3 READY 4 GO) '<LIST [4 FIX ATOM]>>  ;  T
<DECL? '(1 MONEY 2 SHOW 3 READY 4 GO) '<LIST [4 FIX]>>  ;  #FALSE
<DECL? '(1 MONEY 2 SHOW 3 READY 4 GO)
    '<LIST [3 FIX ATOM] FIX ATOM>>  ;  T
<DECL? '(1 MONEY 2 SHOW 3 READY 4 GO) '<LIST [3 FIX ATOM]>>  ;  T

;  REST DECL
<DECL? '[\"hi\" 456 789 1011] '<VECTOR STRING FIX [REST FIX]>>  ;  T
<DECL? '(FOO BAR) '<LIST STRING [REST FIX]>>  ;  #FALSE
<DECL? '(FOO BAR) '<LIST ATOM [REST FIX]>>  ;  #FALSE
<DECL? '(FOO BAR) '<LIST ATOM ATOM [REST FIX]>>  ;  T

;  OPT DECL
<DECL? '(FOO BAR) '<LIST [OPT FIX FIX] [REST ATOM]>>  ;  T
<DECL? '(1 FOO BAR) '<LIST [OPT FIX FIX] [REST ATOM]>>  ;  T
<DECL? '(1 2 FOO BAR) '<LIST [OPT FIX] [REST ATOM]>>  ;  #FALSE
<DECL? '(1 2 FOO BAR) '<LIST [OPT FIX FIX] [REST ATOM]>>  ;  T
<DECL? '(1 2) '<LIST [OPT FIX FIX] [REST ATOM]>>  ;  T
 
;  QUOTE DECL
<DECL? FOO ''FOO>  ;  T
<DECL? FOO ''BAR>  ;  #FALSE
<DECL? '<OR FIX FALSE> ''<OR FIX FALSE>>  ;  T
<DECL? 123 ''<OR FIX FALSE>>  ;  #FALSE

;  Segment DECL
<DECL? '(1 2 3) '<LIST FIX FIX>>  ;  T
<DECL? '(1 2 3) '!<LIST FIX FIX>>  ;  #FALSE
<DECL? '(1 2) '!<LIST FIX FIX>>  ;  T
<DECL? '(1 2) '!<LIST [REST FIX FIX]>>  ;  T
<DECL? '(1 2 3) '!<LIST [REST FIX FIX]>>  ;  #FALSE
<DECL? '(1 2 3 4) '!<LIST [REST FIX FIX]>>  ;  T

;  LVAL/GVAL DECL
<DECL? '.X LVAL>  ;  T
<DECL? '.X GVAL>  ;  #FALSE
<DECL? ',X GVAL>  ;  T
<DECL? ',X LVAL>  ;  #FALSE
<DECL? '.X '<PRIMTYPE ATOM>>  ;  T
<DECL? ',X '<PRIMTYPE ATOM>>  ;  T"""@en ;
                                skos:prefLabel "<DECL? value pattern>"@en .


###  http://example.org/zilf/EMPTY?
<http://example.org/zilf/EMPTY?> rdf:type owl:NamedIndividual ,
                                          skos:Concept ;
                                 skos:broader zilf:CoreFunctions ;
                                 skos:inScheme zilf:ZILF_Scheme ;
                                 skos:definition "MDL built-in predicate that returns true if structure contains no elements, otherwise false."@en ;
                                 skos:editorialNote "structure must be an object that STRUCTURED? evaluates to true."@en ;
                                 skos:example """<EMPTY? [1 2 3]>  ;  False
<EMPTY? []>  ;  True"""@en ;
                                 skos:prefLabel "<EMPTY? structure>"@en .


###  http://example.org/zilf/F?
<http://example.org/zilf/F?> rdf:type owl:NamedIndividual ,
                                      skos:Concept ;
                             skos:broader zilf:ZCodeBuiltIns ;
                             skos:inScheme zilf:ZILF_Scheme ;
                             skos:definition "Z-code built-in predicate that tests is expression evaluates to false."@en ;
                             skos:editorialNote "ZILF supports FONT in all versions."@en ;
                             skos:example """<F? <=? 1 1>>  ;  False
<F? <=? 1 2>>  ;  True"""@en ;
                             skos:prefLabel "<F? expression>"@en .


###  http://example.org/zilf/FIRST?
<http://example.org/zilf/FIRST?> rdf:type owl:NamedIndividual ,
                                          skos:Concept ;
                                 skos:broader zilf:ZCodeBuiltIns ;
                                 skos:inScheme zilf:ZILF_Scheme ;
                                 skos:definition "Z-code built-in function that returns the first object inside (contained) in the object. Returns 0 (false) if no object exists."@en ;
                                 skos:editorialNote "ZILF supports FIRST? in all versions."@en ;
                                 skos:example "<SET RM <FIRST? ,ROOMS>>  ;  Sets RM to first object in ROOMS. Also evaluates to true (all values not 0 is true)"@en ;
                                 skos:historyNote "Zapf syntax: FIRST?, Inform syntax: get_child"@en ;
                                 skos:prefLabel "<FIRST? object>"@en .


###  http://example.org/zilf/FREQUENT-WORDS?
<http://example.org/zilf/FREQUENT-WORDS?> rdf:type owl:NamedIndividual ,
                                                   skos:Concept ;
                                          skos:broader zilf:CoreFunctions ;
                                          skos:inScheme zilf:ZILF_Scheme ;
                                          skos:definition "ZIL library predicate."@en ;
                                          skos:editorialNote "ZILF ignores this and always returns FALSE. Frequent words table is built by ZAPF instead."@en ;
                                          skos:prefLabel "<FREQUENT-WORDS?>"@en .


###  http://example.org/zilf/FSET?
<http://example.org/zilf/FSET?> rdf:type owl:NamedIndividual ,
                                         skos:Concept ;
                                skos:broader zilf:ZCodeBuiltIns ;
                                skos:inScheme zilf:ZILF_Scheme ;
                                skos:definition "Z-code built-in predicate that tests if the flag is set on the object."@en ;
                                skos:editorialNote "ZILF supports FSET? in all versions."@en ;
                                skos:example "<FSET? ,TRAP-DOOR ,OPENBIT>  ;  True if OPENBIT is set"@en ;
                                skos:historyNote "Zapf syntax: FSET?, Inform syntax: test_attr"@en ;
                                skos:prefLabel "<FSET? object flag>"@en .


###  http://example.org/zilf/FUNNY-GLOBALS?
<http://example.org/zilf/FUNNY-GLOBALS?> rdf:type owl:NamedIndividual ,
                                                  skos:Concept ;
                                         skos:broader zilf:CoreFunctions ;
                                         skos:inScheme zilf:ZILF_Scheme ;
                                         skos:definition """When enabled, this ZIL library predicate lets the game define more than the usual 240 global variables.

If needed, ZILF will move the extra variables into a table (GLOBAL-VARS-TABLE) and generate table instructions to access them (PUT and GET, or in the case of BYTE globals created with DEFINE-GLOBALS, PUTB and GETB)."""@en ;
                                         skos:editorialNote "This translation is mostly transparent to game source code, but it can’t be used for global variables that are ever referenced indirectly by number. ZILF uses a simple heuristic to try to identify those variables and reserve “real” global variable slots for them."@en ;
                                         skos:prefLabel "<FUNNY-GLOBALS? [boolean]>"@en .


###  http://example.org/zilf/G?
<http://example.org/zilf/G?> rdf:type owl:NamedIndividual ,
                                      skos:Concept ;
                             skos:broader zilf:CoreFunctions ;
                             skos:inScheme zilf:ZILF_Scheme ;
                             skos:definition "MDL built-in predicate that returns true if value1 is greater than value2, otherwise the predicate returns false."@en ;
                             skos:editorialNote "'G' means \"is greater than.\""@en ;
                             skos:prefLabel "<G? value1 value2>"@en .


###  http://example.org/zilf/GASSIGNED?
<http://example.org/zilf/GASSIGNED?> rdf:type owl:NamedIndividual ,
                                              skos:Concept ;
                                     skos:broader zilf:CoreFunctions ;
                                     skos:inScheme zilf:ZILF_Scheme ;
                                     skos:definition "MDL built-in predicate that returns true if atom has a GVAL (global value)."@en ;
                                     skos:example """<GASSIGNED? X>  ;  False 
<SETG X 1> 
<GASSIGNED? X>  ;  True"""@en ;
                                     skos:prefLabel "<GASSIGNED? Atom>"@en .


###  http://example.org/zilf/GBOUND?
<http://example.org/zilf/GBOUND?> rdf:type owl:NamedIndividual ,
                                           skos:Concept ;
                                  skos:broader zilf:CoreFunctions ;
                                  skos:inScheme zilf:ZILF_Scheme ;
                                  skos:definition "MDL built-in predicate that returns true if the atom ever had a global value."@en ;
                                  skos:example """<SETG X 42> 
<GASSIGNED? X>  ;  True 
<GBOUND? X>  ;  True 
<GUNASSIGN X>
<GASSIGNED? X>  ;  False 
<GBOUND? X>  ;  True"""@en ;
                                  skos:prefLabel "<GBOUND? atom>"@en .


###  http://example.org/zilf/IN?
<http://example.org/zilf/IN?> rdf:type owl:NamedIndividual ,
                                       skos:Concept ;
                              skos:broader zilf:ZCodeBuiltIns ;
                              skos:inScheme zilf:ZILF_Scheme ;
                              skos:definition "Z-code built-in predicate that returns true if object1 is in object2 (object1 has object2 as parent),otherwise false."@en ;
                              skos:editorialNote "ZILF supports IN? in all versions."@en ;
                              skos:example """<OBJECT ANIMAL>
<OBJECT CAT (LOC ANIMAL)>
<IN? ,CAT ,ANIMAL>  ;  T
<IN? ,ANIMAL ,CAT>  ;  <>"""@en ;
                              skos:historyNote "Zapf syntax: IN?, Inform syntax: jin"@en ;
                              skos:prefLabel "<IN? object1 object2>"@en .


###  http://example.org/zilf/INTBL?
<http://example.org/zilf/INTBL?> rdf:type owl:NamedIndividual ,
                                          skos:Concept ;
                                 skos:broader zilf:ZCodeBuiltIns ;
                                 skos:inScheme zilf:ZILF_Scheme ;
                                 skos:definition """Z-code built-in predicate that that returns the address of value if value is in the table table of the length length, otherwise 0. 

In version 5, 7 and 8 the rec-spec describes the field where bit 7 is set for words and clear for bytes, rest defines the length of the field."""@en ;
                                 skos:editorialNote "ZILF supports INTBL? in versions 4-."@en ;
                                 skos:example """<T <INTBL? 3 <TABLE 1 2 3 4> 4>>  ;  T
<T <INTBL? 6 <TABLE 1 2 3 4> 4>>  ;  #FALSE

;  \"Search byte-table with record length 3 (ver 5, 7-)\"
<T <INTBL? 8 <TABLE (BYTE) 2 0 1 4 0 1 8 0 1> 9 3>>  ;  T
<T <INTBL? 1 <TABLE (BYTE) 2 0 1 4 0 1 8 0 1> 9 3>>  ;  <>

;  \"Search word-table with record length 3 (ver 5, 7-)\"
<T <INTBL? 8 <TABLE 2 0 1 4 0 1 8 0 1> 9 131>>  ;  T
<T <INTBL? 1 <TABLE 2 0 1 4 0 1 8 0 1> 9 131>>  ;  <>"""@en ;
                                 skos:historyNote "Zapf syntax: INTBL?, Inform syntax: scan_table"@en ;
                                 skos:prefLabel """<INTBL? value table length [rec-spec]>  ;  \"Version 5, 7-\"
<INTBL? value table length>   ;  \"Version 4, 6\""""@en .


###  http://example.org/zilf/OR?
<http://example.org/zilf/OR?> rdf:type owl:NamedIndividual ,
                                       skos:Concept ;
                              skos:broader zilf:CoreFunctions ;
                              skos:inScheme zilf:ZILF_Scheme ;
                              skos:definition "MDL built-in function that returns the same result as OR with the difference that all exressions are evaluated."@en ;
                              skos:editorialNote """<OR? <=? 1 2> <=? 1 1>>  ; True 
 <OR? <=? 1 1> <SET X 2>> ;  X is set to 2 because all expressions are evaluated"""@en ;
                              skos:prefLabel "<OR? Expressions ...>"@en .


###  http://example.org/zilf/VALID-TYPE?
<http://example.org/zilf/VALID-TYPE?> rdf:type owl:NamedIndividual ,
                                               skos:Concept ;
                                      skos:broader zilf:CoreFunctions ;
                                      skos:inScheme zilf:ZILF_Scheme ;
                                      skos:definition "MDL build-in function that returns the TYPE if the atom is a valid name of a TYPE (the atom name is in ALLTYPES), otherwise FALSE."@en ;
                                      skos:example """<VALID-TYPE? VECTOR>  ;  VECTOR
<VALID-TYPE? FOO>  ;  #FALSE
<NEWTYPE FOO FIX> 
<VALID-TYPE? FOO>  ;  FOO"""@en ;
                                      skos:prefLabel "<VALID-TYPE? atom>"@en .


###  Generated by the OWL API (version 4.5.29.2024-05-13T12:11:03Z) https://github.com/owlcs/owlapi
