@prefix : <http://example.org/zilf/> .
@prefix owl: <http://www.w3.org/2002/07/owl#> .
@prefix rdf: <http://www.w3.org/1999/02/22-rdf-syntax-ns#> .
@prefix xml: <http://www.w3.org/XML/1998/namespace> .
@prefix xsd: <http://www.w3.org/2001/XMLSchema#> .
@prefix rdfs: <http://www.w3.org/2000/01/rdf-schema#> .
@prefix skos: <http://www.w3.org/2004/02/skos/core#> .
@prefix zilf: <http://example.org/zilf/> .
@base <http://example.org/zilf/> .

<http://example.org/zilf/> rdf:type owl:Ontology ;
                            owl:imports <http://www.w3.org/2004/02/skos/core> .

#################################################################
#    Annotation properties
#################################################################

###  http://www.w3.org/2004/02/skos/core#altLabel
skos:altLabel rdf:type owl:AnnotationProperty ;
              rdfs:subPropertyOf rdfs:label .


###  http://www.w3.org/2004/02/skos/core#editorialNote
skos:editorialNote rdf:type owl:AnnotationProperty ;
                   rdfs:subPropertyOf rdfs:label .


###  http://www.w3.org/2004/02/skos/core#historyNote
skos:historyNote rdf:type owl:AnnotationProperty ;
                 rdfs:subPropertyOf rdfs:label .


#################################################################
#    Classes
#################################################################

###  http://example.org/zilf/LanguageConstruct
zilf:LanguageConstruct rdf:type owl:Class ;
                       rdfs:subClassOf skos:Concept .


#################################################################
#    Individuals
#################################################################

###  http://example.org/zilf/ADJ-SYNONYM
zilf:ADJ-SYNONYM rdf:type owl:NamedIndividual ,
                          skos:Concept ;
                 skos:broader zilf:ParserSystem ;
                 skos:inScheme zilf:ZILF_Scheme ;
                 skos:definition "ZIL parser library function that creates one or more synonyms to the original adjective. ZILF treats ADJ-SYNONYM as an alias to SYNONYM."@en ;
                 skos:editorialNote "Note that due to the way words, especially adjectives and nouns, are stored in the vocabulary synonyms for adjectives only work in version 3 (ZIP) games."@en ;
                 skos:example """<ADJ-SYNONYM HAPPY JOYFUL>
<ADJ-SYNONYM INTELLIGENT SMART>
<ADJ-SYNONYM BAD AWFUL>
<ADJ-SYNONYM STRONG SOLID>"""@en ;
                 skos:prefLabel "<ADJ-SYNONYM original synonyms ...>"@en .


###  http://example.org/zilf/ASCII
zilf:ASCII rdf:type owl:NamedIndividual ,
                    skos:Concept ;
           skos:broader zilf:CoreFunctions ;
           skos:inScheme zilf:ZILF_Scheme ;
           skos:definition "MDL built-in function that converts a number to a character or a character to a number."@en ;
           skos:example """<ASCII !\\A>  ;  65
<ASCII 65>  ;  !\\A"""@en ;
           skos:prefLabel "<ASCII {number | character}>"@en .


###  http://example.org/zilf/ATOM
zilf:ATOM rdf:type owl:NamedIndividual ,
                   skos:Concept ;
          skos:broader zilf:CoreFunctions ;
          skos:inScheme zilf:ZILF_Scheme ;
          skos:definition "MDL built-in that returns a newly created ATOM with pname (string). The ATOM is not on any OBLIST and therefore has the trailer !-#FALSE () attached to it."@en ;
          skos:example """<ATOM \"FOO\">  ;  FOO!-#FALSE ()
<==? <ATOM \"FOO\"> <ATOM \"FOO\">>  ;  #FALSE"""@en ;
          skos:prefLabel "<ATOM pname>"@en .


###  http://example.org/zilf/AVALUE
zilf:AVALUE rdf:type owl:NamedIndividual ,
                     skos:Concept ;
            skos:broader zilf:CoreFunctions ;
            skos:inScheme zilf:ZILF_Scheme ;
            skos:definition "MDL built-in function that returns the value part from an asoc entry, of TYPE ASOC, in the ASSOCIATION chain."@en ;
            skos:editorialNote "See ASSOCIATIONS, GETPROP, INDICATOR, ITEM, NEXT and PUTPROP."@en ;
            skos:example """<DEFINE LAST-ASOC ()
    <REPEAT ((A <ASSOCIATIONS>))
        <COND (<=? .A <>> <RETURN <>>)
        (<=? <NEXT .A> <>> <RETURN .A>)>
    <SET A <NEXT .A>>>>
<PUTPROP NEW-ASOC TEXT \"Hello, world!\">
<SET A <LAST-ASOC>>
<AVALUE .A>  ;  \"Hello, world!\""""@en ;
            skos:prefLabel "<AVALUE asoc>"@en .


###  http://example.org/zilf/BEGIN-SEGMENT
zilf:BEGIN-SEGMENT rdf:type owl:NamedIndividual ,
                            skos:Concept ;
                   skos:broader zilf:CoreFunctions ;
                   skos:inScheme zilf:ZILF_Scheme ;
                   skos:definition "ZIL library function that groups code and data into segments of memory outside the main game memory. BEGIN-SEGMENT pairs with END-SEGMENT."@en ;
                   skos:editorialNote "ZILF ignores this and always returns FALSE."@en ;
                   skos:example """; From The Abyss
<BEGIN-SEGMENT 0>
; Code
<END-SEGMENT>

; From Shogun
<BEGIN-SEGMENT RECORD>
; Code
<END-SEGMENT>"""@en ;
                   skos:historyNote "Having been used in a few InfoCom projects, BEGIN-SEGMENT was notably used in The Abyss, an unreleased interactive fiction game written by Bob Bates for Infocom under historical source code for the game, entitled The Abyss Source Code Collection."@en ;
                   skos:prefLabel "<BEGIN-SEGMENT value>"@en .


###  http://example.org/zilf/BIT-SYNONYM
zilf:BIT-SYNONYM rdf:type owl:NamedIndividual ,
                          skos:Concept ;
                 skos:broader zilf:ParserSystem ;
                 skos:inScheme zilf:ZILF_Scheme ;
                 skos:definition "ZIL parser library function that creates synonyms to flag-bits."@en ;
                 skos:example """<BIT-SYNONYM TAKEBIT GETBIT PICKBIT>
<BIT-SYNONYM LIGHTBIT DAYBIT>"""@en ;
                 skos:prefLabel "<BIT-SYNONYM first synonyms ...>"@en .


###  http://example.org/zilf/BUZZ
zilf:BUZZ rdf:type owl:NamedIndividual ,
                   skos:Concept ;
          skos:broader zilf:ParserSystem ;
          skos:inScheme zilf:ZILF_Scheme ;
          skos:definition "ZIL parser library function that creates words in the vocabulary with the part-of-speech BUZZ."@en ;
          skos:editorialNote "These are words that can be ignored by the parser or have special handling in the parser."@en ;
          skos:example """<BUZZ A AN AND ANY ALL EVERY EVERYTHING BUT EXCEPT OF ONE
              THE THEN UNDO OOPS \\. \\, \\\">"""@en ;
          skos:prefLabel "<BUZZ atoms ...>"@en .


###  http://example.org/zilf/BitOn
zilf:BitOn rdf:type owl:NamedIndividual ,
                    skos:Concept ;
           skos:broader zilf:PropFlags ;
           skos:definition "Flag indicating that a light-source object is currently providing light." ;
           skos:prefLabel "ONBIT"@en .


###  http://example.org/zilf/BitTake
zilf:BitTake rdf:type owl:NamedIndividual ,
                      skos:Concept ;
             skos:broader zilf:PropFlags ;
             skos:definition "Flag indicating that an object can be picked up by the player." ;
             skos:prefLabel "TAKEBIT"@en .


###  http://example.org/zilf/CoreFunctions
zilf:CoreFunctions rdf:type owl:NamedIndividual ,
                            skos:Concept ;
                   skos:narrower zilf:ASCII ,
                                 zilf:ATOM ,
                                 zilf:AVALUE ,
                                 zilf:BEGIN-SEGMENT ,
                                 zilf:END-SEGMENT ,
                                 zilf:EVAL ,
                                 zilf:GLOBAL ,
                                 zilf:OR ,
                                 zilf:PICFILE ,
                                 zilf:PNAME ,
                                 zilf:PRIMTYPE ,
                                 zilf:PRIN1 ,
                                 zilf:PRINC ,
                                 zilf:PRINT ,
                                 zilf:PTABLE ,
                                 zilf:PUTREST ,
                                 zilf:QUIT ,
                                 zilf:QUOTE ,
                                 zilf:ROOT ,
                                 zilf:ROUTINE ,
                                 zilf:SET ,
                                 zilf:SETG ,
                                 zilf:SETG20 ,
                                 zilf:SPNAME ,
                                 zilf:STRING ,
                                 zilf:TOP ,
                                 zilf:VALUE ,
                                 <http://example.org/zilf/OR?> ,
                                 <http://example.org/zilf/VALID-TYPE?> ;
                   skos:topConceptOf zilf:ZILF_Scheme ;
                   skos:prefLabel "Core Functions"@en .


###  http://example.org/zilf/DIR-SYNONYM
zilf:DIR-SYNONYM rdf:type owl:NamedIndividual ,
                          skos:Concept ;
                 skos:broader zilf:ParserSystem ;
                 skos:inScheme zilf:ZILF_Scheme ;
                 skos:definition "ZIL parser library function that creates one or more synonyms to the original direction."@en ;
                 skos:editorialNote "ZILF treats DIR-SYNONYM as an alias to SYNONYM."@en ;
                 skos:example """<DIR-SYNONYM FORE F>
<DIR-SYNONYM AFT A>
<DIR-SYNONYM PORT P>
<DIR-SYNONYM STARBOARD SB>"""@en ;
                 skos:prefLabel "<DIR-SYNONYM original synonyms ...>"@en .


###  http://example.org/zilf/END-SEGMENT
zilf:END-SEGMENT rdf:type owl:NamedIndividual ,
                          skos:Concept ;
                 skos:broader zilf:CoreFunctions ;
                 skos:inScheme zilf:ZILF_Scheme ;
                 skos:definition "ZIL library function that terminates the current code and data group, returning to main game memory. END-SEGMENT pairs with BEGIN-SEGMENT."@en ;
                 skos:editorialNote "ZILF ignores this and always returns FALSE."@en ;
                 skos:example """; From The Abyss
<BEGIN-SEGMENT 0>
; Code
<END-SEGMENT>

; From Shogun
<BEGIN-SEGMENT RECORD>
; Code
<END-SEGMENT>"""@en ;
                 skos:historyNote "Having been used in a few InfoCom projects, BEGIN-SEGMENT was notably used in The Abyss, an unreleased interactive fiction game written by Bob Bates for Infocom under historical source code for the game, entitled The Abyss Source Code Collection."@en ;
                 skos:prefLabel "<END-SEGMENT>"@en .


###  http://example.org/zilf/ERASE
zilf:ERASE rdf:type owl:NamedIndividual ,
                    skos:Concept ;
           skos:broader zilf:ZCodeBuiltIns ;
           skos:inScheme zilf:ZILF_Scheme ;
           skos:definition """Z-code built-in function that erases from the current cursor position. This functions behavior is dependent on the supported version.

Versions 4 and 5: if the value is 1, erase from the current cursor position to the end of its line in the current window. If the value is anything other than 1, do nothing.  

Version 6: if the value is 1, erase from the current cursor position to the end of its line in the current window. If not, erase the given number of pixels minus one across from the cursor (clipped to stay inside the right margin). The cursor does not move."""@en ;
           skos:editorialNote "ZILF supports ERASE in versions 4-."@en ;
           skos:example "<ERASE 1>  ;  Clears from cursor to end of line"@en ;
           skos:historyNote "Zapf syntax: ERASE, Inform syntax: erase_line"@en ;
           skos:prefLabel "<ERASE value>"@en .


###  http://example.org/zilf/EVAL
zilf:EVAL rdf:type owl:NamedIndividual ,
                   skos:Concept ;
          skos:broader zilf:CoreFunctions ;
          skos:inScheme zilf:ZILF_Scheme ;
          skos:definition "MDL built-in function that evaluates value (usually a FORM created by FORM or QUOTE)."@en ;
          skos:editorialNote "It is possible to supply an environment for EVAL. This tells EVAL from which environment. EVAL should take variable bindings. See The MDL Programming Language, chap. 9.7 for more about the environment."@en ;
          skos:example """<SET F '<+ 1 2>> 
.F ; Sets up the stack operator and operands, + 1 2.
<EVAL .F> ; Evaluates the operands with the given operator from the stack to 3.
<SET A 0>
<DEFINE WRONG ('B \"AUX\" (A 1)) <EVAL .B>> 
<DEFINE RIGHT (\"BIND\" E 'B \"AUX\" (A 1)) <EVAL .B .E>> 
<WRONG .A> ; 1
<RIGHT .A> ; 0"""@en ;
          skos:prefLabel "<EVAL value [environment]>"@en .


###  http://example.org/zilf/FCLEAR
zilf:FCLEAR rdf:type owl:NamedIndividual ,
                     skos:Concept ;
            skos:broader zilf:ZCodeBuiltIns ;
            skos:inScheme zilf:ZILF_Scheme ;
            skos:definition "Z-code built-in function that removes flag from object."@en ;
            skos:editorialNote "ZILF supports FCLEAR in all versions."@en ;
            skos:example "<FCLEAR ,TRAP-DOOR ,OPENBIT>  ;  Marks the trap-door as closed"@en ;
            skos:historyNote "Zapf syntax: FCLEAR, Inform syntax: clear_attr"@en ;
            skos:prefLabel "<FCLEAR object flag>"@en .


###  http://example.org/zilf/FONT
zilf:FONT rdf:type owl:NamedIndividual ,
                   skos:Concept ;
          skos:broader zilf:ZCodeBuiltIns ;
          skos:inScheme zilf:ZILF_Scheme ;
          skos:definition """Z-code built-in function that Sets current font to number. Returns old fonts number. If the font number is not available 0, return false.

The following numbers map to font types.
1 := Normal font
3 := Character graphics font (see section 16 in the Z-Machine Standards Document).
4 := Monospace (fixed-pitch) font"""@en ;
          skos:editorialNote "ZILF supports FONT in versions 5-."@en ;
          skos:example "<FONT 4>  ;  Sets fixed-pitch font. In versions 3-4, this is done by setting bit 1 of Flags 2 in header <PUT 0 8 <BOR <GET 0 8> 2>>"@en ;
          skos:historyNote "Zapf syntax: FONT, Inform syntax: set_font"@en ;
          skos:prefLabel "Version 5: <FONT number>, Version 6-: <FONT number [window-number]>"@en .


###  http://example.org/zilf/FSET
zilf:FSET rdf:type owl:NamedIndividual ,
                   skos:Concept ;
          skos:broader zilf:ZCodeBuiltIns ;
          skos:inScheme zilf:ZILF_Scheme ;
          skos:definition "Z-code built-in function adds flag to object."@en ;
          skos:editorialNote "ZILF supports FSET in all versions."@en ;
          skos:example "<FSET ,TRAP-DOOR ,OPENBIT> --> Marks the trap-door as open"@en ;
          skos:historyNote "Zapf syntax: FSET, Inform syntax: set_attr"@en ;
          skos:prefLabel "<FSET object flag>"@en .


###  http://example.org/zilf/GET
zilf:GET rdf:type owl:NamedIndividual ,
                  skos:Concept ;
         skos:broader zilf:ZCodeBuiltIns ;
         skos:inScheme zilf:ZILF_Scheme ;
         skos:definition """Z-code built-in function that returns WORD-record (2 bytes) stored at offset. Note that table is an address in memory so the WORD that is returned is at table+offset*2. It is legal to use, for example, 0 as an address to retrieve information from the header. 

Also see BACK, GETB, PUT, PUTB and REST."""@en ;
         skos:editorialNote "ZILF supports GET in all versions."@en ;
         skos:example "<GET <TABLE 0 1 2 3> 2>  ;  2"@en ;
         skos:historyNote "Zapf syntax: GET, Inform syntax: loadw"@en ;
         skos:prefLabel "<GET table offset>"@en .


###  http://example.org/zilf/GETB
zilf:GETB rdf:type owl:NamedIndividual ,
                   skos:Concept ;
          skos:broader zilf:ZCodeBuiltIns ;
          skos:inScheme zilf:ZILF_Scheme ;
          skos:definition """Z-code built-in that returns BYTE-record (1 byte) stored at offset. Note that table is an address in memory so the BYTE that is returned is at table+offset. It is legal to use, for example, 0 as an address to retrieve information from the header. 

Also see BACK, GET, PUT, PUTB and REST."""@en ;
          skos:editorialNote "ZILF supports GETB in all versions."@en ;
          skos:example "<GETB <TABLE (BYTE) !\\A !\\B !\\C !\\D> 2>  ;  !\\C"@en ;
          skos:historyNote "Zapf syntax: GETB, Inform syntax: loadb"@en ;
          skos:prefLabel "<GETB table offset>"@en .


###  http://example.org/zilf/GETP
zilf:GETP rdf:type owl:NamedIndividual ,
                   skos:Concept ;
          skos:broader zilf:ZCodeBuiltIns ;
          skos:inScheme zilf:ZILF_Scheme ;
          skos:definition "Z-code built-in function that gets property from the object. Returns default value if property is not declared in the object."@en ;
          skos:editorialNote "ZILF supports GETP in all versions."@en ;
          skos:example """<OBJECT MYOBJ (MYPROP 123)>
<GETP ,MYOBJ ,P?MYPROP>  ;  123"""@en ;
          skos:historyNote "Zapf syntax: GETP, Inform syntax: get_prop"@en ;
          skos:prefLabel "<GETP object property>"@en .


###  http://example.org/zilf/GETPT
zilf:GETPT rdf:type owl:NamedIndividual ,
                    skos:Concept ;
           skos:broader zilf:ZCodeBuiltIns ;
           skos:inScheme zilf:ZILF_Scheme ;
           skos:definition "Z-code built-in that gets property address from object. Returns 0 (false) if property is not declared in the object."@en ;
           skos:editorialNote "ZILF supports GETPT in all versions."@en ;
           skos:example """<OBJECT MYOBJ (MYPROP 123)>
<GET <GETPT ,MYOBJ ,P?MYPROP> 0>  ;  123
<GETPT ,MYOBJ ,P?MYPROP2>  ;  0"""@en ;
           skos:historyNote "Zapf syntax: GETPT, Inform syntax: get_prop_addr"@en ;
           skos:prefLabel "<GETPT object property>"@en .


###  http://example.org/zilf/GLOBAL
zilf:GLOBAL rdf:type owl:NamedIndividual ,
                     skos:Concept ;
            skos:broader zilf:CoreFunctions ;
            skos:inScheme zilf:ZILF_Scheme ;
            skos:definition "ZIL library function that declares a global variable atom, which can laater be used inside a ROUTINE. The variable is initialized with default-value."@en ;
            skos:editorialNote """ZILF ignores the DECL because DECL is checked in code that runs at compile time (i.e. MDL code); however, there is no type checking for compiled code inside routines, at runtime or compile time.

For example, the following:
<GDECL (BAR) FIX> T
<SETG BAR \"fsdf\">

Outputs this error: 
[error MDL0206] <stdin>:1: expected GVAL of BAR to match DECL FIX, but got \"fdsf\""""@en ;
            skos:example "<GLOBAL MYVAR 0>"@en ;
            skos:prefLabel "<GLOBAL atom default-value [decl] [size]>"@en .


###  http://example.org/zilf/OBJECT
zilf:OBJECT rdf:type owl:NamedIndividual .


###  http://example.org/zilf/OR
zilf:OR rdf:type owl:NamedIndividual ,
                 skos:Concept ;
        skos:broader zilf:CoreFunctions ;
        skos:inScheme zilf:ZILF_Scheme ;
        skos:definition "MDL built-in function that is a boolean OR. Requires that one of the expressions evaluates to true to return true. Exits on the first expression that evaluates to true (rest of expressions are not evaluated)."@en ;
        skos:editorialNote "Because false is its own TYPE outside a routine OR returns #FALSE if all expressions are false or the value of the first true expression."@en ;
        skos:example """<OR <=? 1 2> <=? 1 1>>  ;  True 
 <OR <=? 1 1> <SET X 2>> ;  X is never set to 2 because first predicate evaluates to true 
 <SET X <OR 0 1 2 3>>  ;  X is set to 0 
 <SET X <OR <> 1 2 3>>  ;  X is set to 1"""@en ;
        skos:prefLabel "<OR expressions...>"@en .


###  http://example.org/zilf/ObjectProperties
zilf:ObjectProperties rdf:type owl:NamedIndividual ,
                               skos:Concept ;
                      skos:broader zilf:ObjectSystem ;
                      skos:narrower zilf:PropAdjective ,
                                    zilf:PropDesc ,
                                    zilf:PropFlags ,
                                    zilf:PropSynonym ;
                      skos:prefLabel "Object Properties"@en .


###  http://example.org/zilf/ObjectSystem
zilf:ObjectSystem rdf:type owl:NamedIndividual ,
                           skos:Concept ;
                  skos:narrower zilf:OBJECT ,
                                zilf:ObjectProperties ;
                  skos:topConceptOf zilf:ZILF_Scheme ;
                  skos:prefLabel "Object System"@en .


###  http://example.org/zilf/PICFILE
zilf:PICFILE rdf:type owl:NamedIndividual ,
                      skos:Concept ;
             skos:broader zilf:CoreFunctions ;
             skos:inScheme zilf:ZILF_Scheme ;
             skos:definition "ZIL library function that is a compiler directive used to associate a graphics resource file with a game, and Infocom's version of PICFILE translates to a ZAP .PICFILE directive."@en ;
             skos:editorialNote "The current version of ZILF ignores PICFILE and always returns FALSE because modern interpreters do not support Infocom's graphics format. The next release of ZILF will bundle images into Blorb files (without ZAPF)."@en ;
             skos:prefLabel "<PICFILE>"@en .


###  http://example.org/zilf/PICINF
zilf:PICINF rdf:type owl:NamedIndividual ,
                     skos:Concept ;
            skos:broader zilf:ZCodeBuiltIns ;
            skos:inScheme zilf:ZILF_Scheme ;
            skos:definition "Z-code built-in function that Writes picture data from picture-number into table. Word 0 of table holds picture width and word 1 holds picture height. Then follows the picture data. If picture-number is 0, the number of available pictures is written into word 0 of table and release number of picture file is written into word 1."@en ;
            skos:editorialNote "ZILF currently supports PICINF in versions 6-."@en ;
            skos:example """<GLOBAL MYPIC <ITABLE 2048 0>>
<PICINFO 1 ,MYPIC>  ;  Writes picture data into MYPIC"""@en ;
            skos:historyNote "Zapf syntax: PICINF, Inform syntax: picture_data"@en ;
            skos:prefLabel "<PICINF picture-number table>"@en .


###  http://example.org/zilf/PICSET
zilf:PICSET rdf:type owl:NamedIndividual ,
                     skos:Concept ;
            skos:broader zilf:ZCodeBuiltIns ;
            skos:inScheme zilf:ZILF_Scheme ;
            skos:definition "Z-code built-in function that gives the interpreter a table of picture numbers that the interpreter can then unpack from disc and cache in memory."@en ;
            skos:editorialNote "ZILF currently supports PICSET in versions 6-."@en ;
            skos:example """; From Zork Zero
<PICSET ,B-PICSET-TBL>"""@en ;
            skos:historyNote "Zapf syntax: PICSET, Inform syntax: picture_table"@en ;
            skos:prefLabel "<PICSET table>"@en .


###  http://example.org/zilf/PNAME
zilf:PNAME rdf:type owl:NamedIndividual ,
                    skos:Concept ;
           skos:broader zilf:CoreFunctions ;
           skos:inScheme zilf:ZILF_Scheme ;
           skos:definition "MDL built-in function for \"printed name\", which returns a newly created string copy of the atom's pname."@en ;
           skos:editorialNote "PNAME never prints an ATOMs trailers, unlike UNPARSE, and is therefore quicker."@en ;
           skos:example """<PNAME FOO> ; \"FOO\"
<PNAME FOO!-NEW-OBLIST> ; \"FOO\"
<UNPARSE FOO!-NEW-OBLIST> ; \"FOO!-NEW-OBLIST\""""@en ;
           skos:prefLabel "<PNAME atom>"@en .


###  http://example.org/zilf/POP
zilf:POP rdf:type owl:NamedIndividual ,
                  skos:Concept ;
         skos:broader zilf:ZCodeBuiltIns ;
         skos:inScheme zilf:ZILF_Scheme ;
         skos:definition "Z-code built-in function used inside ROUTINE that pops a value from a stack. If no stack is given, a value is popped from the game stack."@en ;
         skos:editorialNote "ZILF currently supports POP in versions 6-."@en ;
         skos:example """<PUSH .FOO>
<SET FOO some-new-value>
;code
<SET FOO <POP>>"""@en ;
         skos:historyNote "Zapf syntax: POP, Inform syntax: pull"@en ;
         skos:prefLabel "<POP [stack]>"@en .


###  http://example.org/zilf/PREP-SYNONYM
zilf:PREP-SYNONYM rdf:type owl:NamedIndividual ,
                           skos:Concept ;
                  skos:broader zilf:ParserSystem ;
                  skos:inScheme zilf:ZILF_Scheme ;
                  skos:definition "ZIL parser library function that creates one or more synonyms to the original preposition."@en ;
                  skos:editorialNote "ZILF treats PREP-SYNONYM as an alias to SYNONYM."@en ;
                  skos:example """<PREP-SYNONYM INTO IN>
<PREP-SYNONYM UPON ON>
<PREP-SYNONYM ACROSS OVER BEYOND>
<PREP-SYNONYM ABOUT REGARDING CONCERNING>"""@en ;
                  skos:prefLabel "<PREP-SYNONYM original synonyms ...>"@en .


###  http://example.org/zilf/PRIMTYPE
zilf:PRIMTYPE rdf:type owl:NamedIndividual ,
                       skos:Concept ;
              skos:broader zilf:CoreFunctions ;
              skos:inScheme zilf:ZILF_Scheme ;
              skos:definition "MDL built-in function that evaluates to the primitive type of value."@en ;
              skos:editorialNote "The primitive types are  ATOM, FIX, LIST, STRING, TABLE and VECTOR."@en ;
              skos:example """<PRIMTYPE !\\A>  ;  FIX
<PRIMTYPE <+1 2>>  ;  FIX
<PRIMTYPE \"ABC\">  ;  STRING"""@en ;
              skos:prefLabel "<PRIMTYPE value>"@en .


###  http://example.org/zilf/PRIN1
zilf:PRIN1 rdf:type owl:NamedIndividual ,
                    skos:Concept ;
           skos:broader zilf:CoreFunctions ;
           skos:inScheme zilf:ZILF_Scheme ;
           skos:definition "MDL built-in function that prints the evaluated representation of value to channel (default for channel is <LVAL OUTCHAN> - the console). PRIN1 also returns the evaluated representation of value."@en ;
           skos:example """<PRIN1 !\\A>  ;  !\\A
<PRIN1 42>  ; 42
<PRIN1 \"Hello, world!\">  ;  \"Hello, world!\"
<PRIN1 (1 2 3)>  ;  (1 2 3)
<PRIN1 <+ 1 2>>  ;  3"""@en ;
           skos:prefLabel "<PRIN1 value [channel]>"@en .


###  http://example.org/zilf/PRINC
zilf:PRINC rdf:type owl:NamedIndividual ,
                    skos:Concept ;
           skos:broader zilf:CoreFunctions ;
           skos:inScheme zilf:ZILF_Scheme ;
           skos:definition "MDL built-in function that returns the evaluated representation of value."@en ;
           skos:editorialNote "PRINC is just like PRIN1, except for STRING and CHARACTER where surrounding double quote (\") and initial !\\ is suppressed."@en ;
           skos:example """<PRINC !\\A>  ;  !\\A
<PRINC 42>  ; 42
<PRINC \"Hello, world!\">  ;  \"Hello, world!\"
<PRINC (1 2 3)>  ;  (1 2 3)
<PRINC <+ 1 2>>  ;  3"""@en ;
           skos:prefLabel "<PRINC value [channel]>"@en .


###  http://example.org/zilf/PRINT
zilf:PRINT rdf:type owl:NamedIndividual ,
                    skos:Concept ;
           skos:broader zilf:CoreFunctions ;
           skos:inScheme zilf:ZILF_Scheme ;
           rdfs:isDefinedBy """<PRINT !\\A>  ;  !\\A<space>
<PRINT 42>  ; 42<space>
<PRINT \"Hello, world!\">  ;  \"Hello, world!\"<space>
<PRINT (1 2 3)>  ;  (1 2 3)<space>
<PRINT <+ 1 2>>  ;  3<space>"""@en ;
           skos:definition "MDL built-in function that returns the evaluated representation of value."@en ;
           skos:editorialNote "PRINT is just like PRIN1, except that it first prints a CRLF, then the evaluated representation of value and lastly a space."@en ;
           skos:example """<PRINT !\\A>  ;  !\\A<space>
<PRINT 42>  ; 42<space>
<PRINT \"Hello, world!\">  ;  \"Hello, world!\"<space>
<PRINT (1 2 3)>  ;  (1 2 3)<space>
<PRINT <+ 1 2>>  ;  3<space>"""@en ;
           skos:prefLabel "<PRINT value [channel]>"@en .


###  http://example.org/zilf/PTABLE
zilf:PTABLE rdf:type owl:NamedIndividual ,
                     skos:Concept ;
            skos:broader zilf:CoreFunctions ;
            skos:inScheme zilf:ZILF_Scheme ;
            skos:definition "ZIL library function that defines a table containing the specified values and with the PURE flag (see TABLE about PURE and other flags)."@en ;
            skos:editorialNote "TABLE is a ZIL-specific structure that can be used both outside and inside ROUTINES."@en ;
            skos:example "<PTABLE 1 2 3 4>"@en ;
            skos:prefLabel "<PTABLE [(flags ...)] values ...>"@en .


###  http://example.org/zilf/PTSIZE
zilf:PTSIZE rdf:type owl:NamedIndividual ,
                     skos:Concept ;
            skos:broader zilf:ZCodeBuiltIns ;
            skos:inScheme zilf:ZILF_Scheme ;
            skos:definition "Z-code built-in function that gets the property size in bytes at property-address."@en ;
            skos:editorialNote "ZILF supports PTSIZE in all versions."@en ;
            skos:example """<OBJECT MYOBJECT (FOO 1 2 3)>
<PTSIZE <GETPT ,MYOBJECT ,P?FOO>>  ;  6"""@en ;
            skos:historyNote "Zapf syntax: PTSIZE, Inform syntax: get_prop_len"@en ;
            skos:prefLabel "<PTSIZE property-value>"@en .


###  http://example.org/zilf/PUSH
zilf:PUSH rdf:type owl:NamedIndividual ,
                   skos:Concept ;
          skos:broader zilf:ZCodeBuiltIns ;
          skos:inScheme zilf:ZILF_Scheme ;
          skos:definition "Z-code built-in function that pushes value on the game stack."@en ;
          skos:editorialNote "ZILF supports POP in all versions."@en ;
          skos:example "<PUSH 123>"@en ;
          skos:historyNote "Zapf syntax: PUT, Inform syntax: storew"@en ;
          skos:prefLabel "<PUSH value>"@en .


###  http://example.org/zilf/PUT
zilf:PUT rdf:type owl:NamedIndividual ,
                  skos:Concept ;
         skos:broader zilf:ZCodeBuiltIns ;
         skos:inScheme zilf:ZILF_Scheme ;
         skos:definition """Z-code built-in function that puts a 16-bit WORD value in the table at word position offset. Actual address is table-address+offset*2. Note that table can be a byte-address in dynamic memory. 

Also see BACK, GET, GETB, PUTB and REST."""@en ;
         skos:editorialNote "ZILF supports PUT in all versions."@en ;
         skos:example """<PUT ,MYTABLE 1 123>  ;  Stores 123 at position 1 in MYTABLE
<PUT 0 8 <BOR <GET 0 8> 2>>  ;  Sets bit 1 in Flags 2 in header (force monospace)"""@en ;
         skos:historyNote "Zapf syntax: PUT, Inform syntax: storew"@en ;
         skos:prefLabel "<PUT table offset value>"@en .


###  http://example.org/zilf/PUTB
zilf:PUTB rdf:type owl:NamedIndividual ,
                   skos:Concept ;
          skos:broader zilf:ZCodeBuiltIns ;
          skos:inScheme zilf:ZILF_Scheme ;
          skos:definition """Z-code built-in function that puts a byte value in the table at byte position offset. The actual address is table-address+offset. Note that table can be a byte-address in dynamic memory.

Also see BACK, GET, GETB, PUT and REST."""@en ;
          skos:editorialNote "ZILF supports PUTB in all versions."@en ;
          skos:example "<PUTB ,MYTABLE 1 !\\A>  ;  Stores character A at position 1 in MYTABLE"@en ;
          skos:historyNote "Zapf syntax: PUTB, Inform syntax: storeb"@en ;
          skos:prefLabel "<PUTB table offset value>"@en .


###  http://example.org/zilf/PUTP
zilf:PUTP rdf:type owl:NamedIndividual ,
                   skos:Concept ;
          skos:broader zilf:ZCodeBuiltIns ;
          skos:inScheme zilf:ZILF_Scheme ;
          skos:definition "Z-code built-in function that puts value into property on the object."@en ;
          skos:editorialNote "ZILF supports PUTP in all versions."@en ;
          skos:example """<OBJECT MYOBJ (MYPROP 123)>
<PUTP ,MYOBJ ,P?MYPROP 456>  ;  Stores 456 in property MYPROP on MYOBJ"""@en ;
          skos:historyNote "Zapf syntax: PUTP, Inform syntax: put_prop"@en ;
          skos:prefLabel "<PUTP object property value>"@en .


###  http://example.org/zilf/PUTREST
zilf:PUTREST rdf:type owl:NamedIndividual ,
                      skos:Concept ;
             skos:broader zilf:CoreFunctions ;
             skos:inScheme zilf:ZILF_Scheme ;
             skos:definition """MDL built-in function that replaces the REST of list with new-rest and returns list. In other words, list is assigned the first element of list and then all the elements from new-rest. 

Note that this actually changes the list."""@en ;
             skos:example """<PUTREST (1 2 3) (A B)>  ;  (1 A B)

<SET L1 [<SET L2 (1 2 3)>]>
<PUTREST .L2 (A B)>
.L1 ;  [(1 A B)]

<SET L1 [1 2 3]>
<SET L2 <PUTREST (!.L1) (A B)>>
.L1  ;  [1 2 3]
.L2  ;  (1 A B)

<SET L1 (1 2 3 4 5 6 7 8 9)>
<PUTREST <REST .L1 3> <REST .L1 7>>
.L1  ;  (1 2 3 4 8 9)"""@en ;
             skos:prefLabel "<PUTREST list new-rest>"@en .


###  http://example.org/zilf/ParserSystem
zilf:ParserSystem rdf:type owl:NamedIndividual ,
                           skos:Concept ;
                  skos:narrower zilf:ADJ-SYNONYM ,
                                zilf:BIT-SYNONYM ,
                                zilf:BUZZ ,
                                zilf:DIR-SYNONYM ,
                                zilf:PREP-SYNONYM ,
                                zilf:SYNONYM ,
                                zilf:SYNTAX ,
                                zilf:VERB-SYNONYM ;
                  skos:topConceptOf zilf:ZILF_Scheme ;
                  skos:prefLabel "Parser System"@en .


###  http://example.org/zilf/PropAdjective
zilf:PropAdjective rdf:type owl:NamedIndividual ,
                            skos:Concept ;
                   skos:broader zilf:ObjectProperties ;
                   skos:definition "A list of adjectives the parser accepts to identify a specific object." ;
                   skos:example "ADJECTIVE BRASS SMALL" ;
                   skos:prefLabel "ADJECTIVE"@en .


###  http://example.org/zilf/PropDesc
zilf:PropDesc rdf:type owl:NamedIndividual ,
                       skos:Concept ;
              skos:broader zilf:ObjectProperties ;
              skos:definition "A short string used to name the object in game output." ;
              skos:prefLabel "DESC"@en .


###  http://example.org/zilf/PropFlags
zilf:PropFlags rdf:type owl:NamedIndividual ,
                        skos:Concept ;
               skos:broader zilf:ObjectProperties ;
               skos:narrower zilf:BitOn ,
                             zilf:BitTake ;
               skos:definition "A collection of boolean bits (flags) that define the state or behavior of an object." ;
               skos:prefLabel "FLAGS"@en .


###  http://example.org/zilf/PropSynonym
zilf:PropSynonym rdf:type owl:NamedIndividual ,
                          skos:Concept ;
                 skos:broader zilf:ObjectProperties ;
                 skos:definition "A list of nouns the parser accepts for this object." ;
                 skos:prefLabel "SYNONYM"@en .


###  http://example.org/zilf/QUIT
zilf:QUIT rdf:type owl:NamedIndividual ,
                   skos:Concept ;
          skos:broader zilf:CoreFunctions ,
                       zilf:ZCodeBuiltIns ;
          skos:inScheme zilf:ZILF_Scheme ;
          skos:definition "MDL built-in function that exits ZILF (interpreter mode) and returns to the operating system with exit-code."@en ;
          skos:editorialNote "ZILF supports QUIT in all versions."@en ;
          skos:example "<QUIT>"@en ;
          skos:historyNote "Zapf syntax: QUIT, Inform syntax: quit"@en ;
          skos:prefLabel "<QUIT [exit-code]>"@en .


###  http://example.org/zilf/QUOTE
zilf:QUOTE rdf:type owl:NamedIndividual ,
                    skos:Concept ;
           skos:broader zilf:CoreFunctions ;
           skos:inScheme zilf:ZILF_Scheme ;
           skos:altLabel "'value  ;  \"Alternative syntax\""@en ;
           skos:definition "MDL built-in function that returns unevaluated value."@en ;
           skos:example """<SET F <QUOTE <+ 1 2>> ; Or <SET F '<+ 1 2>>
.F  ;  <+ 1 2>
<EVAL .F>  ;  3
'%<+ 1 2>  ;  3"""@en ;
           skos:prefLabel "<QUOTE value>"@en .


###  http://example.org/zilf/RANDOM
zilf:RANDOM rdf:type owl:NamedIndividual ,
                     skos:Concept ;
            skos:broader zilf:ZCodeBuiltIns ;
            skos:inScheme zilf:ZILF_Scheme ;
            skos:definition "Z-code built-in function that returns a random number between 1 and range. If range is negative the randomizer is reseeded with -range (absolute value of range)."@en ;
            skos:editorialNote "ZILF supports RANDOM in all versions."@en ;
            skos:example "<- <RANDOM 101> 1>  ;  Generates random number between 0-100"@en ;
            skos:historyNote "Zapf syntax: RANDOM, Inform syntax: random"@en ;
            skos:prefLabel "<RANDOM range>"@en .


###  http://example.org/zilf/REMOVE
zilf:REMOVE rdf:type owl:NamedIndividual ,
                     skos:Concept ;
            skos:broader zilf:ZCodeBuiltIns ;
            skos:inScheme zilf:ZILF_Scheme ;
            skos:definition "Z-code built-in function that removes object from parent. To reattach it to another object, see MOVE."@en ;
            skos:editorialNote "ZILF supports REMOVE in all versions."@en ;
            skos:example """<OBJECT ANIMAL>
<OBJECT CAT (LOC ANIMAL)>
<REMOVE ,CAT)  ;  Detach CAT from ANIMAL"""@en ;
            skos:historyNote "Zapf syntax: REMOVE, Inform syntax: remove_obj"@en ;
            skos:prefLabel "<REMOVE object>"@en .


###  http://example.org/zilf/RFALSE
zilf:RFALSE rdf:type owl:NamedIndividual ,
                     skos:Concept ;
            skos:broader zilf:ZCodeBuiltIns ;
            skos:inScheme zilf:ZILF_Scheme ;
            skos:definition "Z-code built-in function that  always exits routine and returns false (0). Note that this differs from RETURN that can both exit program blocks and routines."@en ;
            skos:editorialNote "ZILF supports RFALSE in all versions."@en ;
            skos:example "<RFALSE>"@en ;
            skos:historyNote "Zapf syntax: RFALSE, Inform syntax: rfalse"@en ;
            skos:prefLabel "<RFALSE>"@en .


###  http://example.org/zilf/RFATAL
zilf:RFATAL rdf:type owl:NamedIndividual ,
                     skos:Concept ;
            skos:broader zilf:ZCodeBuiltIns ;
            skos:inScheme zilf:ZILF_Scheme ;
            skos:definition "Z-code built-in function that always exits routine and returns FATAL-VALUE (2). Note that this differs from RETURN that can both exit program blocks and routines."@en ;
            skos:example "<RFATAL>"@en ;
            skos:prefLabel "<RFATAL>"@en .


###  http://example.org/zilf/ROOT
zilf:ROOT rdf:type owl:NamedIndividual ,
                   skos:Concept ;
          skos:broader zilf:CoreFunctions ;
          skos:inScheme zilf:ZILF_Scheme ;
          skos:definition "MDL built-in function that returns the OBLIST containing names of primitives (the same as <2 .OBLIST>)."@en ;
          skos:editorialNote "Initially contains all predefined SUBRs or FSUBRs, as well as OBLIST, DEFAULT, T, etc."@en ;
          skos:example "<ROOT>"@en ;
          skos:prefLabel "<ROOT>"@en .


###  http://example.org/zilf/ROUTINE
zilf:ROUTINE rdf:type owl:NamedIndividual ,
                      skos:Concept ;
             skos:broader zilf:CoreFunctions ;
             skos:inScheme zilf:ZILF_Scheme ;
             skos:definition "ZIL library function that is the central building block of a ZIL-program. Inside the ROUTINE it is only possible to use the reduced instruction set that can be executed on the Z-machine. It is the instructions inside the ROUTINEs that are compiled to the actual ZIP-program."@en ;
             skos:editorialNote """ROUTINE defines a program block with its own set of bindings. It is possible to specify an activation-atom to use as an argument to control the RETURN statement inside the ROUTINE. 

The arg-list is formatted the same way as FUNCTION, but the legal tokens is reduced to these:

Arguments: The required arguments for this ROUTINE. The arguments are bound to local variables inside this ROUTINE. 

\"OPT\": The optional arguments for this ROUTINE. The arguments are bound to local variables inside this ROUTINE and can be defined with a default value. \"OPTIONAL\" is an alias for \"OPT\".

\"AUX\": Followed by any number of ATOMs that becomes local variables inside this ROUTINE and can be defined with a default value. \"EXTRA\" is a alias for \"AUX\". 

\"NAME\": Followed by an ATOM that becomes the activation-atom for this ROUTINE. This is equivalent to naming the activation-atom  before the arg-list. \"ACT\" is an alias for \"NAME\". 

Default values for \"OPT\" and \"AUX\" are defined by a two-element LIST whose first element is the ATOM and the second element it is assigned to.

<ROUTINE TEST (\"AUX\" (X 1) (Y 2)) <+ .X .Y>>  Means that the local variables X and Y are initially assigned 1 and 2. After the arg-list follows the ZIL-instructions that makes up the body of the ROUTINE."""@en ;
             skos:example """;\"Move all child objects from object src to object dst\" 
    <ROUTINE MOVE-INVENTORY (SRC DST \"AUX\" X N) 
        <SET X <FIRST? .SRC>> 
        <REPEAT () 
            <COND (.X 
                <SET N <NEXT? .X>> 
                <MOVE .X .DST> 
                <SET X .N>) 
            (T <RETURN>)>>>"""@en ;
             skos:prefLabel "<ROUTINE name [activation-atom] arg-list body ...>"@en .


###  http://example.org/zilf/RSTACK
zilf:RSTACK rdf:type owl:NamedIndividual ,
                     skos:Concept ;
            skos:broader zilf:ZCodeBuiltIns ;
            skos:inScheme zilf:ZILF_Scheme ;
            skos:definition "Z-code built-in function that pops value from the game stack and returns that value."@en ;
            skos:editorialNote "ZILF supports RSTACK in all versions."@en ;
            skos:example """<PUSH 42>
<RSTACK>  ;  Returns 42"""@en ;
            skos:historyNote "Zapf syntax: RSTACK, Inform syntax: ret_popped"@en ;
            skos:prefLabel "<RSTACK>"@en .


###  http://example.org/zilf/RTRUE
zilf:RTRUE rdf:type owl:NamedIndividual ,
                    skos:Concept ;
           skos:broader zilf:ZCodeBuiltIns ;
           skos:inScheme zilf:ZILF_Scheme ;
           skos:definition "Z-code built-in function that always exits routine and returns true (1). Note that this differs from RETURN that can both exit program blocks and routines."@en ;
           skos:editorialNote "ZILF supports RTRUE in all versions."@en ;
           skos:example "<RTRUE>"@en ;
           skos:historyNote "Zapf syntax: RTRUE, Inform syntax: rtrue"@en ;
           skos:prefLabel "<RTRUE>"@en .


###  http://example.org/zilf/SAVE
zilf:SAVE rdf:type owl:NamedIndividual ,
                   skos:Concept ;
          skos:broader zilf:ZCodeBuiltIns ;
          skos:inScheme zilf:ZILF_Scheme ;
          skos:definition """Z-code built-in function that saves a game state that later can be restored. All questions about filename and path are asked by the interpreter. 

SAVE returns 0 if SAVE fails and 1 if it is successful. 

SAVE also can return 2. That means this is a continuation from a successful RESTORE.

See RESTORE on code example on SAVE and RESTORE.

See The Inform Designer’s Manual (ch. §42, p. 319) and The Z-machine Standards Document for a description about how to SAVE and RESTORE auxiliary files."""@en ;
          skos:editorialNote "ZILF supports SAVE in all versions."@en ;
          skos:example """;  Versions 1-4
<SAVE>

;  Version 5-
;  From Zork Zero
<ROUTINE SOFT-SAVE-DEFS ()
    <CLEAR 0>
    <SCREEN 0>
    <COND (<NOT <SAVE ,FKEY-TBL
                             ,FKEYS-STRTABLE-LEN
                             ,DEFS-NAME>>
                    <TELL \"Failed.\">)>
    <CLEAR 0>
    <SCREEN ,SOFT-WINDOW>
    <RFALSE>>

<ROUTINE SOFT-RESTORE-DEFS ()
    <CLEAR 0>
    <SCREEN 0>
    <COND (<NOT <RESTORE ,FKEY-TBL ,FKEYS-STRTABLE-LEN ,DEFS-NAME>>
                    <TELL \"Failed.\">)>
    <CLEAR 0>
    <SCREEN ,SOFT-WINDOW>
    <RFALSE>>"""@en ;
          skos:historyNote "Zapf syntax: SAVE, Inform syntax: save"@en ;
          skos:prefLabel """<SAVE>  ;  Versions 1-4, 
<SAVE [table] [bytes] [filename]>  ;  Versions 5-"""@en .


###  http://example.org/zilf/SCREEN
zilf:SCREEN rdf:type owl:NamedIndividual ,
                     skos:Concept ;
            skos:broader zilf:ZCodeBuiltIns ;
            skos:inScheme zilf:ZILF_Scheme ;
            skos:definition "Z-code built-in function that selects window-number for text output. Note that in versions 3-5 only the lower screen (window-number = 0) has text-buffering and word-wrap."@en ;
            skos:editorialNote "ZILF supports SCREEN in versions 3-."@en ;
            skos:example """<SPLIT 3>
<SCREEN 1>
<TELL \"West of House\">  ;  Split screen in 2 (upper screen is 3 rows) 
                                               ;  and write \"West of House\" in upper screen"""@en ;
            skos:historyNote "Zapf syntax: SCREEN, Inform syntax: set_window"@en ;
            skos:prefLabel "<SCREEN window-number>"@en .


###  http://example.org/zilf/SCROLL
zilf:SCROLL rdf:type owl:NamedIndividual ,
                     skos:Concept ;
            skos:broader zilf:ZCodeBuiltIns ;
            skos:inScheme zilf:ZILF_Scheme ;
            skos:definition "Z-code built-in function that scrolls window-number up (pixels is positive) or down (pixels is negative) by the number of supplied pixels. New lines are empty (background color)."@en ;
            skos:editorialNote "ZILF supports SCROLL in versions 6-."@en ;
            skos:example """;  From Arthur
<SETG GL-AUTHOR-SIZE <RT-COUNT-LINES ,K-DIROUT-TBL>>
<SET AY <* ,GL-AUTHOR-SIZE ,GL-FONT-Y>>
<SCROLL 0 .AY>"""@en ;
            skos:historyNote "Zapf syntax: SCROLL, Inform syntax: scroll_window"@en ;
            skos:prefLabel "<SCROLL window-number pixels>"@en .


###  http://example.org/zilf/SET
zilf:SET rdf:type owl:NamedIndividual ,
                  skos:Concept ;
         skos:broader zilf:CoreFunctions ,
                      zilf:ZCodeBuiltIns ;
         skos:inScheme zilf:ZILF_Scheme ;
         skos:definition """MDL built-in function that asigns a value to the local atom. It is possible to supply an environment for SET. See EVAL for more about the environment.

Z-code built-in function that stores value in local variable name."""@en ;
         skos:editorialNote "ZILF supports SET in all versions."@en ;
         skos:example """MDL: <PROG (X) <SET X 5> <RETURN .X>> ; Returns 5 after setting X.
Zapf: <SET MYVAR 42>  ;  Store 42 in local variable MYVAR"""@en ;
         skos:historyNote "Zapf syntax: SET, Inform syntax: store"@en ;
         skos:prefLabel """MDL: <SET atom value [environment]>
Zapf: <SET name value>"""@en .


###  http://example.org/zilf/SETG
zilf:SETG rdf:type owl:NamedIndividual ,
                   skos:Concept ;
          skos:broader zilf:CoreFunctions ;
          skos:definition "MDL built-in function that assigns a value to the global atom. If an atom is already assigned a value, it is changed."@en ;
          skos:example "<SETG MYVAR 42> ; Store 42 in global atom MYVAR"@en ;
          skos:prefLabel "<SETG atom value>"@en .


###  http://example.org/zilf/SETG20
zilf:SETG20 rdf:type owl:NamedIndividual ,
                     skos:Concept ;
            skos:broader zilf:CoreFunctions ;
            skos:inScheme zilf:ZILF_Scheme ;
            skos:definition "ZIL library function that assigs a value to the global atom. If an atom is already assigned a value, it is changed. SETG20 is an alias for SETG."@en ;
            skos:example "<SETG20 MYVAR 42> ; Store 42 in global atom MYVAR"@en ;
            skos:prefLabel "<SETG20 atom value>"@en .


###  http://example.org/zilf/SPNAME
zilf:SPNAME rdf:type owl:NamedIndividual ,
                     skos:Concept ;
            skos:broader zilf:CoreFunctions ;
            skos:inScheme zilf:ZILF_Scheme ;
            skos:definition "MDL built-in function for \"shared printed name\", which should return the same string of the atom's pname that is in its OBLIST (i.e. pointing to the same storage and therefore not able to change or modify)."@en ;
            skos:editorialNote "ZILF treats SPNAME as an alias to PNAME and returns a string copy of the atom’s pname."@en ;
            skos:example "<SPNAME atom>"@en ;
            skos:prefLabel "<SPNAME atom>"@en .


###  http://example.org/zilf/STRING
zilf:STRING rdf:type owl:NamedIndividual ,
                     skos:Concept ;
            skos:broader zilf:CoreFunctions ;
            skos:inScheme zilf:ZILF_Scheme ;
            skos:definition "MDL built-in function that returns a concatenated string of all values. values can be character or string."@en ;
            skos:editorialNote "A string is a block of contiguous bytes where each byte holds a character. See more about STRING  structure in The MDL Programming Language, Appendix 1."@en ;
            skos:example "<STRING !\\A <ASCII 66> \"CD\"> ; \"ABCD\""@en ;
            skos:prefLabel "<STRING values ...>"@en .


###  http://example.org/zilf/SYNONYM
zilf:SYNONYM rdf:type owl:NamedIndividual ,
                      skos:Concept ;
             skos:broader zilf:ParserSystem ;
             skos:inScheme zilf:ZILF_Scheme ;
             skos:definition "ZIL parser library function that creates one or more synonyms to the original verb, adjective, preposition or direction. Instead of  SYNONYM it is also possible to use VERB-SYNONYM, ADJ-SYNONYM, PREP-SYNONYM and DIR-SYNONYM for verbs, adjectives, prepositions and directions respectively, ZILF handles them all like aliases to SYNONYM."@en ;
             skos:editorialNote "Note that due to the way words, especially adjectives and nouns,  are stored in the vocabulary synonyms for adjectives only work in version 3 (ZIP) games."@en ;
             skos:example """<SYNONYM NORTH FORE>
<SYNONYM SOUTH AFT>
<SYNONYM WEST PORT>
<SYNONYM EAST STARBOARD>

<SYNTAX PUT OBJECT = V-INSERT>
<VERB-SYNONYM PUT SLIDE DIP SOAK>"""@en ;
             skos:prefLabel "<SYNONYM original synonyms ...>"@en .


###  http://example.org/zilf/SYNTAX
zilf:SYNTAX rdf:type owl:NamedIndividual ,
                     skos:Concept ;
            skos:broader zilf:ParserSystem ;
            skos:prefLabel "SYNTAX"@en .


###  http://example.org/zilf/TIME
zilf:TIME rdf:type owl:NamedIndividual ,
                   skos:Concept ;
          skos:broader zilf:CoreFunctions ;
          skos:inScheme zilf:ZILF_Scheme ;
          skos:definition "MDL built-in function that is used for measuring CPU execution time, typically used for debugging ZILCH."@en ;
          skos:editorialNote "ZILF ignores this and always returns 1, because modern IDE's offer different methods of debugging ZILCH."@en ;
          skos:example "<TIME>"@en ;
          skos:prefLabel "<TIME>"@en .


###  http://example.org/zilf/TOP
zilf:TOP rdf:type owl:NamedIndividual ,
                  skos:Concept ;
         skos:broader zilf:CoreFunctions ;
         skos:inScheme zilf:ZILF_Scheme ;
         skos:definition "MDL built-in function that returns array with all elements put back in  array. TOP only works on the structures VECTOR or STRING (arrays) and not on a LIST (a LIST is only pointing forward)."@en ;
         skos:editorialNote "The returned array is not a copy but pointing to the same array with another starting element. Also see BACK, NTH, PUT, REST and SUBSTRUC."@en ;
         skos:example """<SETG STRUCT1 [1 2 3 4 5]>  ;  STRUCT1 = [1 2 3 4 5]
<SETG STRUCT2 <REST ,STRUCT1 2>>  ;  STRUCT2 = [3 4 5]
<TOP ,STRUCT2>  ;  STRUCT2 = [1 2 3 4 5]"""@en ;
         skos:prefLabel "<TOP array>"@en .


###  http://example.org/zilf/VALUE
zilf:VALUE rdf:type owl:NamedIndividual ,
                    skos:Concept ;
           skos:broader zilf:CoreFunctions ;
           skos:inScheme zilf:ZILF_Scheme ;
           skos:definition "MDL built-in function that returns the value of an atom. If  the atom has an LVAL then the LVAL is returned, otherwise the GVAL of the atom is returned."@en ;
           skos:editorialNote "It is possible to supply an environment for VALUE. See EVAL for more about the environment."@en ;
           skos:example """<SETG X 3>
<SET X 4>
<VALUE X>  ;  4
<UNASSIGN X>
<VALUE X>  ;  3"""@en ;
           skos:prefLabel "<VALUE atom [environment]>"@en .


###  http://example.org/zilf/VERB-SYNONYM
zilf:VERB-SYNONYM rdf:type owl:NamedIndividual ,
                           skos:Concept ;
                  skos:broader zilf:ParserSystem ;
                  skos:inScheme zilf:ZILF_Scheme ;
                  skos:definition "ZIL parser library function that creates one or more synonyms to the original verb."@en ;
                  skos:editorialNote "ZILF treats VERB-SYNONYM as an alias to SYNONYM."@en ;
                  skos:example """<VERB-SYNONYM SAY TELL>
<VERB-SYNONYM GO MOVE>
<VERB-SYNONYM MAKE CREATE BUILD>
<VERB-SYNONYM GET OBTAIN ACQUIRE>"""@en ;
                  skos:prefLabel "<VERB-SYNONYM original synonyms ...>"@en .


###  http://example.org/zilf/ZCodeBuiltIns
zilf:ZCodeBuiltIns rdf:type owl:NamedIndividual ,
                            skos:Concept ;
                   skos:inScheme zilf:ZILF_Scheme ;
                   skos:narrower zilf:ERASE ,
                                 zilf:FCLEAR ,
                                 zilf:FONT ,
                                 zilf:FSET ,
                                 zilf:GET ,
                                 zilf:GETB ,
                                 zilf:GETP ,
                                 zilf:GETPT ,
                                 zilf:PICINF ,
                                 zilf:PICSET ,
                                 zilf:POP ,
                                 zilf:PTSIZE ,
                                 zilf:PUSH ,
                                 zilf:PUT ,
                                 zilf:PUTB ,
                                 zilf:PUTP ,
                                 zilf:QUIT ,
                                 zilf:RANDOM ,
                                 zilf:REMOVE ,
                                 zilf:RFALSE ,
                                 zilf:RFATAL ,
                                 zilf:RSTACK ,
                                 zilf:RTRUE ,
                                 zilf:SAVE ,
                                 zilf:SCREEN ,
                                 zilf:SCROLL ,
                                 zilf:SET ,
                                 <http://example.org/zilf/F?> ,
                                 <http://example.org/zilf/FIRST?> ,
                                 <http://example.org/zilf/FSET?> .


###  http://example.org/zilf/ZILF_Scheme
zilf:ZILF_Scheme rdf:type owl:NamedIndividual ,
                          skos:ConceptScheme ;
                 skos:hasTopConcept zilf:CoreFunctions ,
                                    zilf:ObjectSystem ,
                                    zilf:ParserSystem ;
                 skos:prefLabel "ZILF Reference Scheme"@en .


###  http://example.org/zilf/F?
<http://example.org/zilf/F?> rdf:type owl:NamedIndividual ,
                                      skos:Concept ;
                             skos:broader zilf:ZCodeBuiltIns ;
                             skos:inScheme zilf:ZILF_Scheme ;
                             skos:definition "Z-code built-in predicate that tests is expression evaluates to false."@en ;
                             skos:editorialNote "ZILF supports FONT in all versions."@en ;
                             skos:example """<F? <=? 1 1>>  ;  False
<F? <=? 1 2>>  ;  True"""@en ;
                             skos:prefLabel "<F? expression>"@en .


###  http://example.org/zilf/FIRST?
<http://example.org/zilf/FIRST?> rdf:type owl:NamedIndividual ,
                                          skos:Concept ;
                                 skos:broader zilf:ZCodeBuiltIns ;
                                 skos:inScheme zilf:ZILF_Scheme ;
                                 skos:definition "Z-code built-in function that returns the first object inside (contained) in the object. Returns 0 (false) if no object exists."@en ;
                                 skos:editorialNote "ZILF supports FIRST? in all versions."@en ;
                                 skos:example "<SET RM <FIRST? ,ROOMS>>  ;  Sets RM to first object in ROOMS. Also evaluates to true (all values not 0 is true)"@en ;
                                 skos:historyNote "Zapf syntax: FIRST?, Inform syntax: get_child"@en ;
                                 skos:prefLabel "<FIRST? object>"@en .


###  http://example.org/zilf/FSET?
<http://example.org/zilf/FSET?> rdf:type owl:NamedIndividual ,
                                         skos:Concept ;
                                skos:broader zilf:ZCodeBuiltIns ;
                                skos:inScheme zilf:ZILF_Scheme ;
                                skos:definition "Z-code built-in predicate that tests if the flag is set on the object."@en ;
                                skos:editorialNote "ZILF supports FSET? in all versions."@en ;
                                skos:example "<FSET? ,TRAP-DOOR ,OPENBIT>  ;  True if OPENBIT is set"@en ;
                                skos:historyNote "Zapf syntax: FSET?, Inform syntax: test_attr"@en ;
                                skos:prefLabel "<FSET? object flag>"@en .


###  http://example.org/zilf/OR?
<http://example.org/zilf/OR?> rdf:type owl:NamedIndividual ,
                                       skos:Concept ;
                              skos:broader zilf:CoreFunctions ;
                              skos:inScheme zilf:ZILF_Scheme ;
                              skos:definition "MDL built-in function that returns the same result as OR with the difference that all exressions are evaluated."@en ;
                              skos:editorialNote """<OR? <=? 1 2> <=? 1 1>>  ; True 
 <OR? <=? 1 1> <SET X 2>> ;  X is set to 2 because all expressions are evaluated"""@en ;
                              skos:prefLabel "<OR? Expressions ...>"@en .


###  http://example.org/zilf/VALID-TYPE?
<http://example.org/zilf/VALID-TYPE?> rdf:type owl:NamedIndividual ,
                                               skos:Concept ;
                                      skos:broader zilf:CoreFunctions ;
                                      skos:inScheme zilf:ZILF_Scheme ;
                                      skos:definition "MDL build-in function that returns the TYPE if the atom is a valid name of a TYPE (the atom name is in ALLTYPES), otherwise FALSE."@en ;
                                      skos:example """<VALID-TYPE? VECTOR>  ;  VECTOR
<VALID-TYPE? FOO>  ;  #FALSE
<NEWTYPE FOO FIX> 
<VALID-TYPE? FOO>  ;  FOO"""@en ;
                                      skos:prefLabel "<VALID-TYPE? atom>"@en .


###  Generated by the OWL API (version 4.5.29.2024-05-13T12:11:03Z) https://github.com/owlcs/owlapi
